@prefix cim: <http://iec.ch/TC57/CIM100#> .
@prefix rdfs: <http://www.w3.org/2000/01/rdf-schema#> .
@prefix rdf: <http://www.w3.org/1999/02/22-rdf-syntax-ns#> .
@prefix xsd: <http://www.w3.org/2001/XMLSchema#> .
@prefix profile: <http://example.com/cim/profile#> .

profile:sourceCardinality a rdf:Property ;
    rdfs:comment "Cardinality at the source end of an association." .

profile:targetCardinality a rdf:Property ;
    rdfs:comment "Cardinality at the target end of an association." .

cim:ACDCTerminal a rdfs:Class ;
    rdfs:label "ACDCTerminal" ;
    rdfs:comment "An electrical connection point (AC or DC) to a piece of conducting equipment. Terminals are connected at physical connection points called connectivity nodes." ;
    rdfs:subClassOf cim:IdentifiedObject .

cim:AcLineSegment a rdfs:Class ;
    rdfs:label "AcLineSegment" ;
    rdfs:comment "A wire or combination of wires, with consistent electrical characteristics, building a single electrical system, used to carry alternating current between points in the power system.\nFor symmetrical, transposed three phase lines, it is sufficient to use attributes of the line segment, which describe impedances and admittances for the entire length of the segment.  Additionally impedances can be computed by using length and associated per length impedances.\nThe BaseVoltage at the two ends of ACLineSegments in a Line shall have the same BaseVoltage.nominalVoltage. However, boundary lines may have slightly different BaseVoltage.nominalVoltages and variation is allowed. Larger voltage difference in general requires use of an equivalent branch." ;
    rdfs:subClassOf cim:Conductor .

cim:Accumulator a rdfs:Class ;
    rdfs:label "Accumulator" ;
    rdfs:comment "Accumulator represents an accumulated (counted) Measurement, e.g. an energy value." ;
    rdfs:subClassOf cim:Measurement .

cim:AccumulatorValue a rdfs:Class ;
    rdfs:label "AccumulatorValue" ;
    rdfs:comment "AccumulatorValue represents an accumulated (counted) MeasurementValue." ;
    rdfs:subClassOf cim:MeasurementValue .

cim:ActivePower a rdfs:Class ;
    rdfs:label "ActivePower" ;
    rdfs:comment "Product of RMS value of the voltage and the RMS value of the in-phase component of the current." .

cim:Agreement a rdfs:Class ;
    rdfs:label "Agreement" ;
    rdfs:comment "Formal agreement between two parties defining the terms and conditions for a set of services. The specifics of the services are, in turn, defined via one or more service agreements." ;
    rdfs:subClassOf cim:Document .

cim:Analog a rdfs:Class ;
    rdfs:label "Analog" ;
    rdfs:comment "Analog represents an analog Measurement." ;
    rdfs:subClassOf cim:Measurement .

cim:AnalogValue a rdfs:Class ;
    rdfs:label "AnalogValue" ;
    rdfs:comment "AnalogValue represents an analog MeasurementValue." ;
    rdfs:subClassOf cim:MeasurementValue .

cim:AngleDegrees a rdfs:Class ;
    rdfs:label "AngleDegrees" ;
    rdfs:comment "Measurement of angle in degrees." .

cim:AngleRadians a rdfs:Class ;
    rdfs:label "AngleRadians" ;
    rdfs:comment "Phase angle in radians." .

cim:ApparentPower a rdfs:Class ;
    rdfs:label "ApparentPower" ;
    rdfs:comment "Product of the RMS value of the voltage and the RMS value of the current." .

cim:Asset a rdfs:Class ;
    rdfs:label "Asset" ;
    rdfs:comment "Tangible resource of the utility, including power system equipment, various end devices, cabinets, buildings, etc. For electrical network equipment, the role of the asset is defined through PowerSystemResource and its subclasses, defined mainly in the Wires model (refer to IEC61970-301 and model package IEC61970::Wires). Asset description places emphasis on the physical characteristics of the equipment fulfilling that role." ;
    rdfs:subClassOf cim:IdentifiedObject .

cim:AssetContainer a rdfs:Class ;
    rdfs:label "AssetContainer" ;
    rdfs:comment "Asset that is aggregation of other assets such as conductors, transformers, switchgear, land, fences, buildings, equipment, vehicles, etc." ;
    rdfs:subClassOf cim:Asset .

cim:AssetFunction a rdfs:Class ;
    rdfs:label "AssetFunction" ;
    rdfs:comment "Function performed by an asset." ;
    rdfs:subClassOf cim:IdentifiedObject .

cim:AssetInfo a rdfs:Class ;
    rdfs:label "AssetInfo" ;
    rdfs:comment "Set of attributes of an asset, representing typical datasheet information of a physical device that can be instantiated and shared in different data exchange contexts:\n- as attributes of an asset instance (installed or in stock)\n- as attributes of an asset model (product by a manufacturer)\n- as attributes of a type asset (generic type of an asset as used in designs/extension planning)." ;
    rdfs:subClassOf cim:IdentifiedObject .

cim:AssetOrganisationRole a rdfs:Class ;
    rdfs:label "AssetOrganisationRole" ;
    rdfs:comment "Role an organisation plays with respect to asset." ;
    rdfs:subClassOf cim:OrganisationRole .

cim:AssetOwner a rdfs:Class ;
    rdfs:label "AssetOwner" ;
    rdfs:comment "Owner of the asset." ;
    rdfs:subClassOf cim:AssetOrganisationRole .

cim:AuxiliaryEquipment a rdfs:Class ;
    rdfs:label "AuxiliaryEquipment" ;
    rdfs:comment "AuxiliaryEquipment describe equipment that is not performing any primary functions but support for the equipment performing the primary function.\nAuxiliaryEquipment is attached to primary equipment via an association with Terminal." ;
    rdfs:subClassOf cim:Equipment .

cim:BaseVoltage a rdfs:Class ;
    rdfs:label "BaseVoltage" ;
    rdfs:comment "Defines a system base voltage which is referenced." ;
    rdfs:subClassOf cim:IdentifiedObject .

cim:BatteryControl a rdfs:Class ;
    rdfs:label "BatteryControl" ;
    rdfs:comment "\\[ZBEX\\] Describes behaviour specific to controlling batteries." ;
    rdfs:subClassOf cim:RegulatingControl .

cim:BatteryControlMode a rdfs:Class ;
    rdfs:label "BatteryControlMode" ;
    rdfs:comment "\\[ZBEX\\] Kind of battery control." .

cim:BatteryStateKind a rdfs:Class ;
    rdfs:label "BatteryStateKind" ;
    rdfs:comment "The state of the battery unit." .

cim:BatteryUnit a rdfs:Class ;
    rdfs:label "BatteryUnit" ;
    rdfs:comment "An electrochemical energy storage device." ;
    rdfs:subClassOf cim:PowerElectronicsUnit .

cim:Boolean a rdfs:Class ;
    rdfs:label "Boolean" ;
    rdfs:comment "A type with the value space \"true\" and \"false\"." .

cim:Breaker a rdfs:Class ;
    rdfs:label "Breaker" ;
    rdfs:comment "A mechanical switching device capable of making, carrying, and breaking currents under normal circuit conditions and also making, carrying for a specified time, and breaking currents under specified abnormal circuit conditions e.g.  those of short circuit." ;
    rdfs:subClassOf cim:ProtectedSwitch .

cim:BusbarSection a rdfs:Class ;
    rdfs:label "BusbarSection" ;
    rdfs:comment "A conductor, or group of conductors, with negligible impedance, that serve to connect other conducting equipment within a single substation. \nVoltage measurements are typically obtained from voltage transformers that are connected to busbar sections. A bus bar section may have many physical terminals but for analysis is modelled with exactly one logical terminal." ;
    rdfs:subClassOf cim:Connector .

cim:CableInfo a rdfs:Class ;
    rdfs:label "CableInfo" ;
    rdfs:comment "Cable data." ;
    rdfs:subClassOf cim:WireInfo .

cim:Circuit a rdfs:Class ;
    rdfs:label "Circuit" ;
    rdfs:comment "" ;
    rdfs:subClassOf cim:Line .

cim:Clamp a rdfs:Class ;
    rdfs:label "Clamp" ;
    rdfs:comment "A Clamp is a galvanic connection at a line segment where other equipment is connected. A Clamp does not cut the line segment. \nA Clamp is ConductingEquipment and has one Terminal with an associated ConnectivityNode. Any other ConductingEquipment can be connected to the Clamp ConnectivityNode." ;
    rdfs:subClassOf cim:ConductingEquipment .

cim:Conductance a rdfs:Class ;
    rdfs:label "Conductance" ;
    rdfs:comment "Factor by which voltage must be multiplied to give corresponding power lost from a circuit. Real part of admittance." .

cim:ConductancePerLength a rdfs:Class ;
    rdfs:label "ConductancePerLength" ;
    rdfs:comment "Real part of admittance per unit of length." .

cim:ConductingEquipment a rdfs:Class ;
    rdfs:label "ConductingEquipment" ;
    rdfs:comment "The parts of the AC power system that are designed to carry current or that are conductively connected through terminals." ;
    rdfs:subClassOf cim:Equipment .

cim:Conductor a rdfs:Class ;
    rdfs:label "Conductor" ;
    rdfs:comment "Combination of conducting material with consistent electrical characteristics, building a single electrical system, used to carry current between points in the power system." ;
    rdfs:subClassOf cim:ConductingEquipment .

cim:ConnectivityNode a rdfs:Class ;
    rdfs:label "ConnectivityNode" ;
    rdfs:comment "Connectivity nodes are points where terminals of AC conducting equipment are connected together with zero impedance." ;
    rdfs:subClassOf cim:IdentifiedObject .

cim:ConnectivityNodeContainer a rdfs:Class ;
    rdfs:label "ConnectivityNodeContainer" ;
    rdfs:comment "A base class for all objects that may contain connectivity nodes or topological nodes." ;
    rdfs:subClassOf cim:PowerSystemResource .

cim:Connector a rdfs:Class ;
    rdfs:label "Connector" ;
    rdfs:comment "A conductor, or group of conductors, with negligible impedance, that serve to connect other conducting equipment within a single substation and are modelled with a single logical terminal." ;
    rdfs:subClassOf cim:ConductingEquipment .

cim:ContactDetails a rdfs:Class ;
    rdfs:label "ContactDetails" ;
    rdfs:comment "\\[ZBEX\\] The details required to contact a person or company.\"" .

cim:ContactMethodType a rdfs:Class ;
    rdfs:label "ContactMethodType" ;
    rdfs:comment "\\[ZBEX\\] The method to use to make contact with a person or company." .

cim:Control a rdfs:Class ;
    rdfs:label "Control" ;
    rdfs:comment "Control is used for supervisory/device control. It represents control outputs that are used to change the state in a process, e.g. close or open breaker, a set point value or a raise lower command." ;
    rdfs:subClassOf cim:IOPoint .

cim:ControlledAppliance a rdfs:Class ;
    rdfs:label "ControlledAppliance" ;
    rdfs:comment "Appliance controlled with a PAN device control." .

cim:CurrentFlow a rdfs:Class ;
    rdfs:label "CurrentFlow" ;
    rdfs:comment "Electrical current with sign convention: positive flow is out of the conducting equipment into the connectivity node. Can be both AC and DC." .

cim:CurrentRelay a rdfs:Class ;
    rdfs:label "CurrentRelay" ;
    rdfs:comment "A device that checks current flow values in any direction or designated direction." ;
    rdfs:subClassOf cim:ProtectionRelayFunction .

cim:CurrentTransformer a rdfs:Class ;
    rdfs:label "CurrentTransformer" ;
    rdfs:comment "Instrument transformer used to measure electrical qualities of the circuit that is being protected and/or monitored. Typically used as current transducer for the purpose of metering or protection. A typical secondary current rating would be 5A." ;
    rdfs:subClassOf cim:Sensor .

cim:CurrentTransformerInfo a rdfs:Class ;
    rdfs:label "CurrentTransformerInfo" ;
    rdfs:comment "Properties of current transformer asset." ;
    rdfs:subClassOf cim:AssetInfo .

cim:Curve a rdfs:Class ;
    rdfs:label "Curve" ;
    rdfs:comment "A multi-purpose curve or functional relationship between an independent variable (X-axis) and dependent (Y-axis) variables." ;
    rdfs:subClassOf cim:IdentifiedObject .

cim:CurveData a rdfs:Class ;
    rdfs:label "CurveData" ;
    rdfs:comment "Multi-purpose data points for defining a curve. The use of this generic class is discouraged if a more specific class can be used to specify the X and Y axis values along with their specific data types." .

cim:Customer a rdfs:Class ;
    rdfs:label "Customer" ;
    rdfs:comment "Organisation receiving services from service supplier." ;
    rdfs:subClassOf cim:OrganisationRole .

cim:CustomerAgreement a rdfs:Class ;
    rdfs:label "CustomerAgreement" ;
    rdfs:comment "Agreement between the customer and the service supplier to pay for service at a specific service location. It records certain billing information about the type of service provided at the service location and is used during charge creation to determine the type of service." ;
    rdfs:subClassOf cim:Agreement .

cim:CustomerKind a rdfs:Class ;
    rdfs:label "CustomerKind" ;
    rdfs:comment "Kind of customer." .

cim:Cut a rdfs:Class ;
    rdfs:label "Cut" ;
    rdfs:comment "A cut separates a line segment into two parts. The cut appears as a switch inserted between these two parts and connects them together. As the cut is normally open there is no galvanic connection between the two line segment parts. But it is possible to close the cut to get galvanic connection.\nThe cut terminals are oriented towards the line segment terminals with the same sequence number. Hence the cut terminal with sequence number equal to 1 is oriented to the line segment's terminal with sequence number equal to 1.\nThe cut terminals also act as connection points for jumpers and other equipment, e.g. a mobile generator. To enable this, connectivity nodes are placed at the cut terminals. Once the connectivity nodes are in place any conducting equipment can be connected at them." ;
    rdfs:subClassOf cim:Switch .

cim:DateTime a rdfs:Class ;
    rdfs:label "DateTime" ;
    rdfs:comment "Date and time as \"yyyy-mm-ddThh:mm:ss.sss\", which conforms with ISO 8601. UTC time zone is specified as \"yyyy-mm-ddThh:mm:ss.sssZ\". A local timezone relative UTC is specified as \"yyyy-mm-ddThh:mm:ss.sss-hh:mm\". The second component (shown here as \"ss.sss\") could have any number of digits in its fractional part to allow any kind of precision beyond seconds." .

cim:DateTimeInterval a rdfs:Class ;
    rdfs:label "DateTimeInterval" ;
    rdfs:comment "Interval between two date and time points, where the interval includes the start time but excludes end time." .

cim:Diagram a rdfs:Class ;
    rdfs:label "Diagram" ;
    rdfs:comment "The diagram being exchanged. The coordinate system is a standard Cartesian coordinate system and the orientation attribute defines the orientation. The initial view related attributes can be used to specify an initial view with the x,y coordinates of the diagonal points." ;
    rdfs:subClassOf cim:IdentifiedObject .

cim:DiagramObject a rdfs:Class ;
    rdfs:label "DiagramObject" ;
    rdfs:comment "An object that defines one or more points in a given space. This object can be associated with anything that specializes IdentifiedObject. For single line diagrams such objects typically include such items as analog values, breakers, disconnectors, power transformers, and transmission lines." ;
    rdfs:subClassOf cim:IdentifiedObject .

cim:DiagramObjectPoint a rdfs:Class ;
    rdfs:label "DiagramObjectPoint" ;
    rdfs:comment "A point in a given space defined by 3 coordinates and associated to a diagram object.  The coordinates may be positive or negative as the origin does not have to be in the corner of a diagram." .

cim:DiagramStyle a rdfs:Class ;
    rdfs:label "DiagramStyle" ;
    rdfs:comment "The diagram style refers to a style used by the originating system for a diagram.  A diagram style describes information such as schematic, geographic, etc." .

cim:DirectionalCurrentRelay a rdfs:Class ;
    rdfs:label "DirectionalCurrentRelay" ;
    rdfs:comment "[ZBEX] A Directional Current Relay is a type of protective relay used in electrical power systems to detect the\ndirection of current flow and operate only when the current exceeds a certain threshold in a specified direction." ;
    rdfs:subClassOf cim:ProtectionRelayFunction .

cim:Disconnector a rdfs:Class ;
    rdfs:label "Disconnector" ;
    rdfs:comment "A manually operated or motor operated mechanical switching device used for changing the connections in a circuit, or for isolating a circuit or equipment from a source of power. It is required to open or close circuits when negligible current is broken or made." ;
    rdfs:subClassOf cim:Switch .

cim:Discrete a rdfs:Class ;
    rdfs:label "Discrete" ;
    rdfs:comment "Discrete represents a discrete Measurement, i.e. a Measurement representing discrete values, e.g. a Breaker position." ;
    rdfs:subClassOf cim:Measurement .

cim:DiscreteValue a rdfs:Class ;
    rdfs:label "DiscreteValue" ;
    rdfs:comment "DiscreteValue represents a discrete MeasurementValue." ;
    rdfs:subClassOf cim:MeasurementValue .

cim:DistanceRelay a rdfs:Class ;
    rdfs:label "DistanceRelay" ;
    rdfs:comment "\\[ZBEX\\] This extension is in-line with the CIM working group for replacing the `protection` package, can be replaced when the working group outcome is merged into the CIM model. <br/> A protective device used in power systems that measures the impedance of a transmission line to determine the distance to a fault, and initiates circuit breaker tripping to isolate the faulty section and safeguard the power system." ;
    rdfs:subClassOf cim:ProtectionRelayFunction .

cim:Document a rdfs:Class ;
    rdfs:label "Document" ;
    rdfs:comment "Parent class for different groupings of information collected and managed as a part of a business process. It will frequently contain references to other objects, such as assets, people and power system resources." ;
    rdfs:subClassOf cim:IdentifiedObject .

cim:EarthFaultCompensator a rdfs:Class ;
    rdfs:label "EarthFaultCompensator" ;
    rdfs:comment "A conducting equipment used to represent a connection to ground which is typically used to compensate earth faults. An earth fault compensator device modelled with a single terminal implies a second terminal solidly connected to ground. If two terminals are modelled, the ground is not assumed and normal connection rules apply." ;
    rdfs:subClassOf cim:ConductingEquipment .

cim:ElectronicAddress a rdfs:Class ;
    rdfs:label "ElectronicAddress" ;
    rdfs:comment "Electronic address information." .

cim:EndDevice a rdfs:Class ;
    rdfs:label "EndDevice" ;
    rdfs:comment "Asset container that performs one or more end device functions. One type of end device is a meter which can perform metering, load management, connect/disconnect, accounting functions, etc. Some end devices, such as ones monitoring and controlling air conditioners, refrigerators, pool pumps may be connected to a meter. All end devices may have communication capability defined by the associated communication function(s). An end device may be owned by a consumer, a service provider, utility or otherwise.\nThere may be a related end device function that identifies a sensor or control point within a metering application or communications systems (e.g., water, gas, electricity).\nSome devices may use an optical port that conforms to the ANSI C12.18 standard for communications." ;
    rdfs:subClassOf cim:AssetContainer .

cim:EndDeviceFunction a rdfs:Class ;
    rdfs:label "EndDeviceFunction" ;
    rdfs:comment "Function performed by an end device such as a meter, communication equipment, controllers, etc." ;
    rdfs:subClassOf cim:AssetFunction .

cim:EndDeviceFunctionKind a rdfs:Class ;
    rdfs:label "EndDeviceFunctionKind" ;
    rdfs:comment "Kind of end device function." .

cim:EnergyConnection a rdfs:Class ;
    rdfs:label "EnergyConnection" ;
    rdfs:comment "A connection of energy generation or consumption on the power system model." ;
    rdfs:subClassOf cim:ConductingEquipment .

cim:EnergyConsumer a rdfs:Class ;
    rdfs:label "EnergyConsumer" ;
    rdfs:comment "Generic user of energy - a  point of consumption on the power system model.\nEnergyConsumer.pfixed, .qfixed, .pfixedPct and .qfixedPct have meaning only if there is no LoadResponseCharacteristic associated with EnergyConsumer or if LoadResponseCharacteristic.exponentModel is set to False." ;
    rdfs:subClassOf cim:EnergyConnection .

cim:EnergyConsumerPhase a rdfs:Class ;
    rdfs:label "EnergyConsumerPhase" ;
    rdfs:comment "A single phase of an energy consumer." ;
    rdfs:subClassOf cim:PowerSystemResource .

cim:EnergySource a rdfs:Class ;
    rdfs:label "EnergySource" ;
    rdfs:comment "A generic equivalent for an energy supplier on a transmission or distribution voltage level." ;
    rdfs:subClassOf cim:EnergyConnection .

cim:EnergySourcePhase a rdfs:Class ;
    rdfs:label "EnergySourcePhase" ;
    rdfs:comment "Represents the single phase information of an unbalanced energy source." ;
    rdfs:subClassOf cim:PowerSystemResource .

cim:Equipment a rdfs:Class ;
    rdfs:label "Equipment" ;
    rdfs:comment "The parts of a power system that are physical devices, electronic or mechanical." ;
    rdfs:subClassOf cim:PowerSystemResource .

cim:EquipmentContainer a rdfs:Class ;
    rdfs:label "EquipmentContainer" ;
    rdfs:comment "A modelling construct to provide a root class for containing equipment." ;
    rdfs:subClassOf cim:ConnectivityNodeContainer .

cim:EquivalentBranch a rdfs:Class ;
    rdfs:label "EquivalentBranch" ;
    rdfs:comment "The class represents equivalent branches. In cases where a transformer phase shift is modelled and the EquivalentBranch is spanning the same nodes, the impedance quantities for the EquivalentBranch shall consider the needed phase shift." ;
    rdfs:subClassOf cim:EquivalentEquipment .

cim:EquivalentEquipment a rdfs:Class ;
    rdfs:label "EquivalentEquipment" ;
    rdfs:comment "The class represents equivalent objects that are the result of a network reduction. The class is the base for equivalent objects of different types." ;
    rdfs:subClassOf cim:ConductingEquipment .

cim:EvChargingUnit a rdfs:Class ;
    rdfs:label "EvChargingUnit" ;
    rdfs:comment "\\[ZBEX\\] An electric vehicle charging station." ;
    rdfs:subClassOf cim:PowerElectronicsUnit .

cim:FaultIndicator a rdfs:Class ;
    rdfs:label "FaultIndicator" ;
    rdfs:comment "A FaultIndicator is typically only an indicator (which may or may not be remotely monitored), and not a piece of equipment that actually initiates a protection event. It is used for FLISR (Fault Location, Isolation and Restoration) purposes, assisting with the dispatch of crews to \"most likely\" part of the network (i.e. assists with determining circuit section where the fault most likely happened)." ;
    rdfs:subClassOf cim:AuxiliaryEquipment .

cim:Feeder a rdfs:Class ;
    rdfs:label "Feeder" ;
    rdfs:comment "A collection of equipment for organizational purposes, used for grouping distribution resources.\nThe organization a feeder does not necessarily reflect connectivity or current operation state." ;
    rdfs:subClassOf cim:EquipmentContainer .

cim:Float a rdfs:Class ;
    rdfs:label "Float" ;
    rdfs:comment "A floating point number. The range is unspecified and not limited." .

cim:Frequency a rdfs:Class ;
    rdfs:label "Frequency" ;
    rdfs:comment "Cycles per second." .

cim:Fuse a rdfs:Class ;
    rdfs:label "Fuse" ;
    rdfs:comment "An overcurrent protective device with a circuit opening fusible part that is heated and severed by the passage of overcurrent through it. A fuse is considered a switching device because it breaks current." ;
    rdfs:subClassOf cim:Switch .

cim:GeographicalRegion a rdfs:Class ;
    rdfs:label "GeographicalRegion" ;
    rdfs:comment "A geographical region of a power system network model." ;
    rdfs:subClassOf cim:IdentifiedObject .

cim:Ground a rdfs:Class ;
    rdfs:label "Ground" ;
    rdfs:comment "A point where the system is grounded used for connecting conducting equipment to ground. The power system model can have any number of grounds." ;
    rdfs:subClassOf cim:ConductingEquipment .

cim:GroundDisconnector a rdfs:Class ;
    rdfs:label "GroundDisconnector" ;
    rdfs:comment "A manually operated or motor operated mechanical switching device used for isolating a circuit or equipment from ground." ;
    rdfs:subClassOf cim:Switch .

cim:GroundingImpedance a rdfs:Class ;
    rdfs:label "GroundingImpedance" ;
    rdfs:comment "A fixed impedance device used for grounding." ;
    rdfs:subClassOf cim:EarthFaultCompensator .

cim:IOPoint a rdfs:Class ;
    rdfs:label "IOPoint" ;
    rdfs:comment "The class describe a measurement or control value. The purpose is to enable having attributes and associations common for measurement and control." ;
    rdfs:subClassOf cim:IdentifiedObject .

cim:IdentifiedObject a rdfs:Class ;
    rdfs:label "IdentifiedObject" ;
    rdfs:comment "This is a root class to provide common identification for all classes needing identification and naming attributes." .

cim:Impedance a rdfs:Class ;
    rdfs:label "Impedance" ;
    rdfs:comment "Ratio of voltage to current." .

cim:Integer a rdfs:Class ;
    rdfs:label "Integer" ;
    rdfs:comment "An integer number. The range is unspecified and not limited." .

cim:Jumper a rdfs:Class ;
    rdfs:label "Jumper" ;
    rdfs:comment "A short section of conductor with negligible impedance which can be manually removed and replaced if the circuit is de-energized. Note that zero-impedance branches can potentially be modelled by other equipment types." ;
    rdfs:subClassOf cim:Switch .

cim:Junction a rdfs:Class ;
    rdfs:label "Junction" ;
    rdfs:comment "A point where one or more conducting equipments are connected with zero resistance." ;
    rdfs:subClassOf cim:Connector .

cim:KiloActivePower a rdfs:Class ;
    rdfs:label "KiloActivePower" ;
    rdfs:comment "Active power in kilowatts." .

cim:Length a rdfs:Class ;
    rdfs:label "Length" ;
    rdfs:comment "Unit of length. It shall be a positive value or zero." .

cim:Line a rdfs:Class ;
    rdfs:label "Line" ;
    rdfs:comment "Contains equipment beyond a substation belonging to a power transmission line." ;
    rdfs:subClassOf cim:EquipmentContainer .

cim:LinearShuntCompensator a rdfs:Class ;
    rdfs:label "LinearShuntCompensator" ;
    rdfs:comment "A linear shunt compensator has banks or sections with equal admittance values." ;
    rdfs:subClassOf cim:ShuntCompensator .

cim:LoadBreakSwitch a rdfs:Class ;
    rdfs:label "LoadBreakSwitch" ;
    rdfs:comment "A mechanical switching device capable of making, carrying, and breaking currents under normal operating conditions." ;
    rdfs:subClassOf cim:ProtectedSwitch .

cim:Location a rdfs:Class ;
    rdfs:label "Location" ;
    rdfs:comment "The place, scene, or point of something where someone or something has been, is, and/or will be at a given moment in time. It can be defined with one or more position points (coordinates) in a given coordinate system." ;
    rdfs:subClassOf cim:IdentifiedObject .

cim:Loop a rdfs:Class ;
    rdfs:label "Loop" ;
    rdfs:comment "\\[ZBEX\\] Sub-transmission circuits are usually arranged in loops so that a single line failure does not cut off service to many customers for more than a short time." ;
    rdfs:subClassOf cim:IdentifiedObject .

cim:LvFeeder a rdfs:Class ;
    rdfs:label "LvFeeder" ;
    rdfs:comment "\\[ZBEX\\] A branch of LV network starting at a distribution substation and continuing until the end of the LV network." ;
    rdfs:subClassOf cim:EquipmentContainer .

cim:Measurement a rdfs:Class ;
    rdfs:label "Measurement" ;
    rdfs:comment "A Measurement represents any measured, calculated or non-measured non-calculated quantity. Any piece of equipment may contain Measurements, e.g. a substation may have temperature measurements and door open indications, a transformer may have oil temperature and tank pressure measurements, a bay may contain a number of power flow measurements and a Breaker may contain a switch status measurement. \nThe PSR - Measurement association is intended to capture this use of Measurement and is included in the naming hierarchy based on EquipmentContainer. The naming hierarchy typically has Measurements as leaves, e.g. Substation-VoltageLevel-Bay-Switch-Measurement.\nSome Measurements represent quantities related to a particular sensor location in the network, e.g. a voltage transformer (VT) or potential transformer (PT) at a busbar or a current transformer (CT) at the bar between a breaker and an isolator. The sensing position is not captured in the PSR - Measurement association. Instead it is captured by the Measurement - Terminal association that is used to define the sensing location in the network topology. The location is defined by the connection of the Terminal to ConductingEquipment. \nIf both a Terminal and PSR are associated, and the PSR is of type ConductingEquipment, the associated Terminal should belong to that ConductingEquipment instance.\nWhen the sensor location is needed both Measurement-PSR and Measurement-Terminal are used. The Measurement-Terminal association is never used alone." ;
    rdfs:subClassOf cim:IdentifiedObject .

cim:MeasurementValue a rdfs:Class ;
    rdfs:label "MeasurementValue" ;
    rdfs:comment "The current state for a measurement. A state value is an instance of a measurement from a specific source. Measurements can be associated with many state values, each representing a different source for the measurement." .

cim:Meter a rdfs:Class ;
    rdfs:label "Meter" ;
    rdfs:comment "Physical asset that performs the metering role of the usage point. Used for measuring consumption and detection of events." ;
    rdfs:subClassOf cim:EndDevice .

cim:Name a rdfs:Class ;
    rdfs:label "Name" ;
    rdfs:comment "The Name class provides the means to define any number of human readable  names for an object. A name is <b>not</b> to be used for defining inter-object relationships. For inter-object relationships instead use the object identification 'mRID'." .

cim:NameType a rdfs:Class ;
    rdfs:label "NameType" ;
    rdfs:comment "Type of name. Possible values for attribute 'name' are implementation dependent but standard profiles may specify types. An enterprise may have multiple IT systems each having its own local name for the same object, e.g. a planning system may have different names from an EMS. An object may also have different names within the same IT system, e.g. localName as defined in CIM version 14. The definition from CIM14 is:\nThe localName is a human readable name of the object. It is a free text name local to a node in a naming hierarchy similar to a file directory structure. A power system related naming hierarchy may be: Substation, VoltageLevel, Equipment etc. Children of the same parent in such a hierarchy have names that typically are unique among them." .

cim:NoLoadTest a rdfs:Class ;
    rdfs:label "NoLoadTest" ;
    rdfs:comment "No-load test results determine core admittance parameters. They include exciting current and core loss measurements from applying voltage to one winding. The excitation may be positive sequence or zero sequence. The test may be repeated at different voltages to measure saturation." ;
    rdfs:subClassOf cim:TransformerTest .

cim:OpenCircuitTest a rdfs:Class ;
    rdfs:label "OpenCircuitTest" ;
    rdfs:comment "Open-circuit test results verify winding turn ratios and phase shifts. They include induced voltage and phase shift measurements on open-circuit windings, with voltage applied to the energised end. For three-phase windings, the excitation can be a positive sequence (the default) or a zero sequence." ;
    rdfs:subClassOf cim:TransformerTest .

cim:OperationalRestriction a rdfs:Class ;
    rdfs:label "OperationalRestriction" ;
    rdfs:comment "A document that can be associated with equipment to describe any sort of restrictions compared with the original manufacturer's specification or with the usual operational practice e.g. temporary maximum loadings, maximum switching current, do not operate if bus couplers are open, etc.\nIn the UK, for example, if a breaker or switch ever mal-operates, this is reported centrally and utilities use their asset systems to identify all the installed devices of the same manufacturer's type. They then apply operational restrictions in the operational systems to warn operators of potential problems. After appropriate inspection and maintenance, the operational restrictions may be removed." ;
    rdfs:subClassOf cim:Document .

cim:Organisation a rdfs:Class ;
    rdfs:label "Organisation" ;
    rdfs:comment "Organisation that might have roles as utility, contractor, supplier, manufacturer, customer, etc." ;
    rdfs:subClassOf cim:IdentifiedObject .

cim:OrganisationRole a rdfs:Class ;
    rdfs:label "OrganisationRole" ;
    rdfs:comment "Identifies a way in which an organisation may participate in the utility enterprise (e.g., customer, manufacturer, etc)." ;
    rdfs:subClassOf cim:IdentifiedObject .

cim:OrientationKind a rdfs:Class ;
    rdfs:label "OrientationKind" ;
    rdfs:comment "The orientation of the coordinate system with respect to top, left, and the coordinate number system." .

cim:OverheadWireInfo a rdfs:Class ;
    rdfs:label "OverheadWireInfo" ;
    rdfs:comment "Overhead wire data." ;
    rdfs:subClassOf cim:WireInfo .

cim:PU a rdfs:Class ;
    rdfs:label "PU" ;
    rdfs:comment "Per Unit - a positive or negative value referred to a defined base. Values typically range from -10 to +10." .

cim:PanDemandResponseFunction a rdfs:Class ;
    rdfs:label "PanDemandResponseFunction" ;
    rdfs:comment "\\[ZBEX\\] PAN function that an end device supports, distinguished by 'kind'." ;
    rdfs:subClassOf cim:EndDeviceFunction .

cim:PerCent a rdfs:Class ;
    rdfs:label "PerCent" ;
    rdfs:comment "Percentage on a defined base.   For example, specify as 100 to indicate at the defined base." .

cim:PerLengthImpedance a rdfs:Class ;
    rdfs:label "PerLengthImpedance" ;
    rdfs:comment "Common type for per-length impedance electrical catalogues." ;
    rdfs:subClassOf cim:PerLengthLineParameter .

cim:PerLengthLineParameter a rdfs:Class ;
    rdfs:label "PerLengthLineParameter" ;
    rdfs:comment "Common type for per-length electrical catalogues describing line parameters." ;
    rdfs:subClassOf cim:IdentifiedObject .

cim:PerLengthPhaseImpedance a rdfs:Class ;
    rdfs:label "PerLengthPhaseImpedance" ;
    rdfs:comment "Impedance and admittance parameters per unit length for n-wire unbalanced lines, in matrix form." ;
    rdfs:subClassOf cim:PerLengthImpedance .

cim:PerLengthSequenceImpedance a rdfs:Class ;
    rdfs:label "PerLengthSequenceImpedance" ;
    rdfs:comment "Sequence impedance and admittance parameters per unit length, for transposed lines of 1, 2, or 3 phases. For 1-phase lines, define x=x0=xself. For 2-phase lines, define x=xs-xm and x0=xs+xm." ;
    rdfs:subClassOf cim:PerLengthImpedance .

cim:PetersenCoil a rdfs:Class ;
    rdfs:label "PetersenCoil" ;
    rdfs:comment "A variable impedance device normally used to offset line charging during single line faults in an ungrounded section of network." ;
    rdfs:subClassOf cim:EarthFaultCompensator .

cim:PhaseCode a rdfs:Class ;
    rdfs:label "PhaseCode" ;
    rdfs:comment "An unordered enumeration of phase identifiers.  Allows designation of phases for both transmission and distribution equipment, circuits and loads.   The enumeration, by itself, does not describe how the phases are connected together or connected to ground.  Ground is not explicitly denoted as a phase.\nResidential and small commercial loads are often served from single-phase, or split-phase, secondary circuits. For the example of s12N, phases 1 and 2 refer to hot wires that are 180 degrees out of phase, while N refers to the neutral wire. Through single-phase transformer connections, these secondary circuits may be served from one or two of the primary phases A, B, and C. For three-phase loads, use the A, B, C phase codes instead of s12N.\nThe integer values are from IEC 61968-9 to support revenue metering applications." .

cim:PhaseImpedanceData a rdfs:Class ;
    rdfs:label "PhaseImpedanceData" ;
    rdfs:comment "Impedance and conductance matrix element values. \nThe diagonal elements are described by the elements having the same toPhase and fromPhase value and the off diagonal elements have different toPhase and fromPhase values.  The matrix can also be stored in symmetric lower triangular format using the row and column attributes, which map to ACLineSegmentPhase.sequenceNumber." .

cim:PhaseShuntConnectionKind a rdfs:Class ;
    rdfs:label "PhaseShuntConnectionKind" ;
    rdfs:comment "The configuration of phase connections for a single terminal device such as a load or capacitor." .

cim:PhotoVoltaicUnit a rdfs:Class ;
    rdfs:label "PhotoVoltaicUnit" ;
    rdfs:comment "A photovoltaic device or an aggregation of such devices." ;
    rdfs:subClassOf cim:PowerElectronicsUnit .

cim:PolarizingQuantityType a rdfs:Class ;
    rdfs:label "PolarizingQuantityType" ;
    rdfs:comment "[ZBEX] Defines the type of polarizing quantity used by the directional relay. This informs how the relay\ndetermines the reference voltage from the Voltage transformers associated with its parent ProtectionEquipment." .

cim:Pole a rdfs:Class ;
    rdfs:label "Pole" ;
    rdfs:comment "Pole asset." ;
    rdfs:subClassOf cim:Structure .

cim:PositionPoint a rdfs:Class ;
    rdfs:label "PositionPoint" ;
    rdfs:comment "Set of spatial coordinates that determine a point, defined in the coordinate system specified in 'Location.CoordinateSystem'. Use a single position point instance to describe a point-oriented location. Use a sequence of position points to describe a line-oriented object (physical location of non-point oriented objects like cables or lines), or area of an object (like a substation or a geographical zone - in this case, have first and last position point with the same values)." .

cim:PotentialTransformer a rdfs:Class ;
    rdfs:label "PotentialTransformer" ;
    rdfs:comment "Instrument transformer (also known as Voltage Transformer) used to measure electrical qualities of the circuit that is being protected and/or monitored. Typically used as voltage transducer for the purpose of metering, protection, or sometimes auxiliary substation supply. A typical secondary voltage rating would be 120V." ;
    rdfs:subClassOf cim:Sensor .

cim:PotentialTransformerInfo a rdfs:Class ;
    rdfs:label "PotentialTransformerInfo" ;
    rdfs:comment "Properties of potential transformer asset." ;
    rdfs:subClassOf cim:AssetInfo .

cim:PotentialTransformerKind a rdfs:Class ;
    rdfs:label "PotentialTransformerKind" ;
    rdfs:comment "The construction kind of the potential transformer." .

cim:PowerDirectionKind a rdfs:Class ;
    rdfs:label "PowerDirectionKind" ;
    rdfs:comment "\\[ZBEX\\] This extension is in-line with the CIM working group for replacing the `protection` package, can be replaced when the working group outcome is merged into the CIM model. <br/> The flow of power direction used by a ProtectionEquipment." .

cim:PowerElectronicsConnection a rdfs:Class ;
    rdfs:label "PowerElectronicsConnection" ;
    rdfs:comment "A connection to the AC network for energy production or consumption that uses power electronics rather than rotating machines." ;
    rdfs:subClassOf cim:RegulatingCondEq .

cim:PowerElectronicsConnectionPhase a rdfs:Class ;
    rdfs:label "PowerElectronicsConnectionPhase" ;
    rdfs:comment "A single phase of a power electronics connection." ;
    rdfs:subClassOf cim:PowerSystemResource .

cim:PowerElectronicsUnit a rdfs:Class ;
    rdfs:label "PowerElectronicsUnit" ;
    rdfs:comment "A generating unit or battery or aggregation that connects to the AC network using power electronics rather than rotating machines." ;
    rdfs:subClassOf cim:Equipment .

cim:PowerElectronicsWindUnit a rdfs:Class ;
    rdfs:label "PowerElectronicsWindUnit" ;
    rdfs:comment "A wind generating unit that connects to the AC network with power electronics rather than rotating machines or an aggregation of such units." ;
    rdfs:subClassOf cim:PowerElectronicsUnit .

cim:PowerSystemResource a rdfs:Class ;
    rdfs:label "PowerSystemResource" ;
    rdfs:comment "A power system resource (PSR) can be an item of equipment such as a switch, an equipment container containing many individual items of equipment such as a substation, or an organisational entity such as sub-control area. Power system resources can have measurements associated." ;
    rdfs:subClassOf cim:IdentifiedObject .

cim:PowerTransformer a rdfs:Class ;
    rdfs:label "PowerTransformer" ;
    rdfs:comment "An electrical device consisting of  two or more coupled windings, with or without a magnetic core, for introducing mutual coupling between electric circuits. Transformers can be used to control voltage and phase shift (active power flow).\nA power transformer may be composed of separate transformer tanks that need not be identical.\nA power transformer can be modelled with or without tanks and is intended for use in both balanced and unbalanced representations.   A power transformer typically has two terminals, but may have one (grounding), three or more terminals.\nThe inherited association ConductingEquipment.BaseVoltage should not be used.  The association from TransformerEnd to BaseVoltage should be used instead." ;
    rdfs:subClassOf cim:ConductingEquipment .

cim:PowerTransformerEnd a rdfs:Class ;
    rdfs:label "PowerTransformerEnd" ;
    rdfs:comment "A PowerTransformerEnd is associated with each Terminal of a PowerTransformer.\nThe impedance values r, r0, x, and x0 of a PowerTransformerEnd represents a star equivalent as follows.\n1) for a two Terminal PowerTransformer the high voltage (TransformerEnd.endNumber=1) PowerTransformerEnd has non zero values on r, r0, x, and x0 while the low voltage (TransformerEnd.endNumber=2) PowerTransformerEnd has zero values for r, r0, x, and x0.  Parameters are always provided, even if the PowerTransformerEnds have the same rated voltage.  In this case, the parameters are provided at the PowerTransformerEnd which has TransformerEnd.endNumber equal to 1.\n2) for a three Terminal PowerTransformer the three PowerTransformerEnds represent a star equivalent with each leg in the star represented by r, r0, x, and x0 values.\n3) For a three Terminal transformer each PowerTransformerEnd shall have g, g0, b and b0 values corresponding to the no load losses distributed on the three PowerTransformerEnds. The total no load loss shunt impedances may also be placed at one of the PowerTransformerEnds, preferably the end numbered 1, having the shunt values on end 1.  This is the preferred way.\n4) for a PowerTransformer with more than three Terminals the PowerTransformerEnd impedance values cannot be used. Instead use the TransformerMeshImpedance or split the transformer into multiple PowerTransformers.\nEach PowerTransformerEnd must be contained by a PowerTransformer. Because a PowerTransformerEnd (or any other object) can not be contained by more than one parent, a PowerTransformerEnd can not have an association to an EquipmentContainer (Substation, VoltageLevel, etc)." ;
    rdfs:subClassOf cim:TransformerEnd .

cim:PowerTransformerInfo a rdfs:Class ;
    rdfs:label "PowerTransformerInfo" ;
    rdfs:comment "Set of power transformer data, from an equipment library." ;
    rdfs:subClassOf cim:AssetInfo .

cim:PricingStructure a rdfs:Class ;
    rdfs:label "PricingStructure" ;
    rdfs:comment "Grouping of pricing components and prices used in the creation of customer charges and the eligibility criteria under which these terms may be offered to a customer. The reasons for grouping include state, customer classification, site characteristics, classification (i.e. fee price structure, deposit price structure, electric service price structure, etc.) and accounting requirements." ;
    rdfs:subClassOf cim:Document .

cim:ProtectedSwitch a rdfs:Class ;
    rdfs:label "ProtectedSwitch" ;
    rdfs:comment "A ProtectedSwitch is a switching device that can be operated by ProtectionEquipment." ;
    rdfs:subClassOf cim:Switch .

cim:ProtectionKind a rdfs:Class ;
    rdfs:label "ProtectionKind" ;
    rdfs:comment "\\[ZBEX\\] This extension is in-line with the CIM working group for replacing the `protection` package, can be replaced when the working group outcome is merged into the CIM model. <br/> The kind of protection being provided by this protection equipment." .

cim:ProtectionRelayFunction a rdfs:Class ;
    rdfs:label "ProtectionRelayFunction" ;
    rdfs:comment "\\[ZBEX\\] This extension is in-line with the CIM working group for replacing the `protection` package, can be replaced when the working group outcome is merged into the CIM model. <br/> A function that a relay implements to protect equipment." ;
    rdfs:subClassOf cim:PowerSystemResource .

cim:ProtectionRelayScheme a rdfs:Class ;
    rdfs:label "ProtectionRelayScheme" ;
    rdfs:comment "\\[ZBEX\\] This extension is in-line with the CIM working group for replacing the `protection` package, can be replaced when the working group outcome is merged into the CIM model. <br/> A scheme that a group of relay functions implement. For example, typically schemes are primary and secondary, or main and failsafe." ;
    rdfs:subClassOf cim:IdentifiedObject .

cim:ProtectionRelaySystem a rdfs:Class ;
    rdfs:label "ProtectionRelaySystem" ;
    rdfs:comment "\\[ZBEX\\] This extension is in-line with the CIM working group for replacing the `protection` package, can be replaced when the working group outcome is merged into the CIM model. <br/> A relay system for controlling ProtectedSwitches." ;
    rdfs:subClassOf cim:Equipment .

cim:Ratio a rdfs:Class ;
    rdfs:label "Ratio" ;
    rdfs:comment "Fraction specified explicitly with a numerator and denominator, which can be used to calculate the quotient." .

cim:RatioTapChanger a rdfs:Class ;
    rdfs:label "RatioTapChanger" ;
    rdfs:comment "A tap changer that changes the voltage ratio impacting the voltage magnitude but not the phase angle across the transformer.\n\nAngle sign convention (general): Positive value indicates a positive phase shift from the winding where the tap is located to the other winding (for a two-winding transformer)." ;
    rdfs:subClassOf cim:TapChanger .

cim:Reactance a rdfs:Class ;
    rdfs:label "Reactance" ;
    rdfs:comment "Reactance (imaginary part of impedance), at rated frequency." .

cim:ReactancePerLength a rdfs:Class ;
    rdfs:label "ReactancePerLength" ;
    rdfs:comment "Reactance (imaginary part of impedance) per unit of length, at rated frequency." .

cim:ReactiveCapabilityCurve a rdfs:Class ;
    rdfs:label "ReactiveCapabilityCurve" ;
    rdfs:comment "Reactive power rating envelope versus the synchronous machine's active power, in both the generating and motoring modes. For each active power value there is a corresponding high and low reactive power limit value. Typically there will be a separate curve for each coolant condition, such as hydrogen pressure. The Y1 axis values represent reactive minimum and the Y2 axis values represent reactive maximum." ;
    rdfs:subClassOf cim:Curve .

cim:ReactivePower a rdfs:Class ;
    rdfs:label "ReactivePower" ;
    rdfs:comment "Product of RMS value of the voltage and the RMS value of the quadrature component of the current." .

cim:RealEnergy a rdfs:Class ;
    rdfs:label "RealEnergy" ;
    rdfs:comment "Real electrical energy." .

cim:Recloser a rdfs:Class ;
    rdfs:label "Recloser" ;
    rdfs:comment "Pole-mounted fault interrupter with built-in phase and ground relays, current transformer (CT), and supplemental controls." ;
    rdfs:subClassOf cim:ProtectedSwitch .

cim:RegulatingCondEq a rdfs:Class ;
    rdfs:label "RegulatingCondEq" ;
    rdfs:comment "A type of conducting equipment that can regulate a quantity (i.e. voltage or flow) at a specific point in the network." ;
    rdfs:subClassOf cim:EnergyConnection .

cim:RegulatingControl a rdfs:Class ;
    rdfs:label "RegulatingControl" ;
    rdfs:comment "Specifies a set of equipment that works together to control a power system quantity such as voltage or flow. \nRemote bus voltage control is possible by specifying the controlled terminal located at some place remote from the controlling equipment.\nThe specified terminal shall be associated with the connectivity node of the controlled point.  The most specific subtype of RegulatingControl shall be used in case such equipment participate in the control, e.g. TapChangerControl for tap changers.\nFor flow control, load sign convention is used, i.e. positive sign means flow out from a TopologicalNode (bus) into the conducting equipment.\nThe attribute minAllowedTargetValue and maxAllowedTargetValue are required in the following cases:\n- For a power generating module operated in power factor control mode to specify maximum and minimum power factor values;\n- Whenever it is necessary to have an off center target voltage for the tap changer regulator. For instance, due to long cables to off shore wind farms and the need to have a simpler setup at the off shore transformer platform, the voltage is controlled from the land at the connection point for the off shore wind farm. Since there usually is a voltage rise along the cable, there is typical and overvoltage of up 3-4 kV compared to the on shore station. Thus in normal operation the tap changer on the on shore station is operated with a target set point, which is in the lower parts of the dead band.\nThe attributes minAllowedTargetValue and maxAllowedTargetValue are not related to the attribute targetDeadband and thus they are not treated as an alternative of the targetDeadband. They are needed due to limitations in the local substation controller. The attribute targetDeadband is used to prevent the power flow from move the tap position in circles (hunting) that is to be used regardless of the attributes minAllowedTargetValue and maxAllowedTargetValue." ;
    rdfs:subClassOf cim:PowerSystemResource .

cim:RegulatingControlModeKind a rdfs:Class ;
    rdfs:label "RegulatingControlModeKind" ;
    rdfs:comment "The kind of regulation model.   For example regulating voltage, reactive power, active power, etc." .

cim:RelayInfo a rdfs:Class ;
    rdfs:label "RelayInfo" ;
    rdfs:comment "\\[ZBEX\\] Relay Datasheet Information." ;
    rdfs:subClassOf cim:AssetInfo .

cim:RelaySetting a rdfs:Class ;
    rdfs:label "RelaySetting" ;
    rdfs:comment "\\[ZBEX\\] This extension is in-line with the CIM working group for replacing the `protection` package, can be replaced when the working group outcome is merged into the CIM model. <br/> The threshold settings for a given relay." .

cim:RemoteControl a rdfs:Class ;
    rdfs:label "RemoteControl" ;
    rdfs:comment "Remote controls are outputs that are sent by the remote unit to actuators in the process." ;
    rdfs:subClassOf cim:RemotePoint .

cim:RemotePoint a rdfs:Class ;
    rdfs:label "RemotePoint" ;
    rdfs:comment "For an RTU, remote points correspond to telemetered values or control outputs. Other units (e.g. control centres) usually also contain calculated values." ;
    rdfs:subClassOf cim:IdentifiedObject .

cim:RemoteSource a rdfs:Class ;
    rdfs:label "RemoteSource" ;
    rdfs:comment "Remote sources are state variables that are telemetered or calculated within the remote unit." ;
    rdfs:subClassOf cim:RemotePoint .

cim:Resistance a rdfs:Class ;
    rdfs:label "Resistance" ;
    rdfs:comment "Resistance (real part of impedance)." .

cim:ResistancePerLength a rdfs:Class ;
    rdfs:label "ResistancePerLength" ;
    rdfs:comment "Resistance (real part of impedance) per unit of length." .

cim:RotatingMachine a rdfs:Class ;
    rdfs:label "RotatingMachine" ;
    rdfs:comment "A rotating machine which may be used as a generator or motor." ;
    rdfs:subClassOf cim:RegulatingCondEq .

cim:SVCControlMode a rdfs:Class ;
    rdfs:label "SVCControlMode" ;
    rdfs:comment "Static VAr Compensator control mode." .

cim:Seconds a rdfs:Class ;
    rdfs:label "Seconds" ;
    rdfs:comment "Time, in seconds." .

cim:Sensor a rdfs:Class ;
    rdfs:label "Sensor" ;
    rdfs:comment "This class describe devices that transform a measured quantity into signals that can be presented at displays, used in control or be recorded." ;
    rdfs:subClassOf cim:AuxiliaryEquipment .

cim:SeriesCompensator a rdfs:Class ;
    rdfs:label "SeriesCompensator" ;
    rdfs:comment "A Series Compensator is a series capacitor or reactor or an AC transmission line without charging susceptance.  It is a two terminal device." ;
    rdfs:subClassOf cim:ConductingEquipment .

cim:ShortCircuitTest a rdfs:Class ;
    rdfs:label "ShortCircuitTest" ;
    rdfs:comment "Short-circuit test results determine mesh impedance parameters. They include load losses and leakage impedances. For three-phase windings, the excitation can be a positive sequence (the default) or a zero sequence. There shall be at least one grounded winding." ;
    rdfs:subClassOf cim:TransformerTest .

cim:ShuntCompensator a rdfs:Class ;
    rdfs:label "ShuntCompensator" ;
    rdfs:comment "A shunt capacitor or reactor or switchable bank of shunt capacitors or reactors. A section of a shunt compensator is an individual capacitor or reactor.  A negative value for reactivePerSection indicates that the compensator is a reactor. ShuntCompensator is a single terminal device.  Ground is implied." ;
    rdfs:subClassOf cim:RegulatingCondEq .

cim:ShuntCompensatorInfo a rdfs:Class ;
    rdfs:label "ShuntCompensatorInfo" ;
    rdfs:comment "Properties of shunt capacitor, shunt reactor or switchable bank of shunt capacitor or reactor assets." ;
    rdfs:subClassOf cim:AssetInfo .

cim:SinglePhaseKind a rdfs:Class ;
    rdfs:label "SinglePhaseKind" ;
    rdfs:comment "Enumeration of single phase identifiers. Allows designation of single phases for both transmission and distribution equipment, circuits and loads." .

cim:Site a rdfs:Class ;
    rdfs:label "Site" ;
    rdfs:comment "\\[ZBEX\\] A collection of equipment for organizational purposes, used for grouping distribution resources located at a site." ;
    rdfs:subClassOf cim:EquipmentContainer .

cim:StaticVarCompensator a rdfs:Class ;
    rdfs:label "StaticVarCompensator" ;
    rdfs:comment "A facility for providing variable and controllable shunt reactive power. The SVC typically consists of a step-down transformer, filter, thyristor-controlled reactor, and thyristor-switched capacitor arms.\n\nThe SVC may operate in fixed MVar output mode or in voltage control mode. When in voltage control mode, the output of the SVC will be proportional to the deviation of voltage at the controlled bus from the voltage setpoint.  The SVC characteristic slope defines the proportion.  If the voltage at the controlled bus is equal to the voltage setpoint, the SVC MVar output is zero." ;
    rdfs:subClassOf cim:RegulatingCondEq .

cim:StreetAddress a rdfs:Class ;
    rdfs:label "StreetAddress" ;
    rdfs:comment "General purpose street and postal address information." .

cim:StreetDetail a rdfs:Class ;
    rdfs:label "StreetDetail" ;
    rdfs:comment "Street details, in the context of address." .

cim:Streetlight a rdfs:Class ;
    rdfs:label "Streetlight" ;
    rdfs:comment "Streetlight asset." ;
    rdfs:subClassOf cim:Asset .

cim:StreetlightLampKind a rdfs:Class ;
    rdfs:label "StreetlightLampKind" ;
    rdfs:comment "Kind of lamp for the streetlight." .

cim:String a rdfs:Class ;
    rdfs:label "String" ;
    rdfs:comment "A string consisting of a sequence of characters. The character encoding is UTF-8. The string length is unspecified and unlimited." .

cim:Structure a rdfs:Class ;
    rdfs:label "Structure" ;
    rdfs:comment "Construction holding assets such as conductors, transformers, switchgear, etc. Where applicable, number of conductors can be derived from the number of associated wire spacing instances." ;
    rdfs:subClassOf cim:AssetContainer .

cim:SubGeographicalRegion a rdfs:Class ;
    rdfs:label "SubGeographicalRegion" ;
    rdfs:comment "A subset of a geographical region of a power system network model." ;
    rdfs:subClassOf cim:IdentifiedObject .

cim:Substation a rdfs:Class ;
    rdfs:label "Substation" ;
    rdfs:comment "A collection of equipment for purposes other than generation or utilization, through which electric energy in bulk is passed for the purposes of switching or modifying its characteristics." ;
    rdfs:subClassOf cim:EquipmentContainer .

cim:Susceptance a rdfs:Class ;
    rdfs:label "Susceptance" ;
    rdfs:comment "Imaginary part of admittance." .

cim:SusceptancePerLength a rdfs:Class ;
    rdfs:label "SusceptancePerLength" ;
    rdfs:comment "Imaginary part of admittance per unit of length." .

cim:Switch a rdfs:Class ;
    rdfs:label "Switch" ;
    rdfs:comment "A generic device designed to close, or open, or both, one or more electric circuits.  All switches are two terminal devices including grounding switches. The ACDCTerminal.connected at the two sides of the switch shall not be considered for assessing switch connectivity, i.e. only Switch.open, .normalOpen and .locked are relevant." ;
    rdfs:subClassOf cim:ConductingEquipment .

cim:SwitchInfo a rdfs:Class ;
    rdfs:label "SwitchInfo" ;
    rdfs:comment "<was Switch data.>\nSwitch datasheet information." ;
    rdfs:subClassOf cim:AssetInfo .

cim:SynchronousMachine a rdfs:Class ;
    rdfs:label "SynchronousMachine" ;
    rdfs:comment "An electromechanical device that operates with shaft rotating synchronously with the network. It is a single machine operating either as a generator or synchronous condenser or pump." ;
    rdfs:subClassOf cim:RotatingMachine .

cim:SynchronousMachineKind a rdfs:Class ;
    rdfs:label "SynchronousMachineKind" ;
    rdfs:comment "Synchronous machine type." .

cim:TapChanger a rdfs:Class ;
    rdfs:label "TapChanger" ;
    rdfs:comment "Mechanism for changing transformer winding tap positions." ;
    rdfs:subClassOf cim:PowerSystemResource .

cim:TapChangerControl a rdfs:Class ;
    rdfs:label "TapChangerControl" ;
    rdfs:comment "Describes behaviour specific to tap changers, e.g. how the voltage at the end of a line varies with the load level and compensation of the voltage drop by tap adjustment." ;
    rdfs:subClassOf cim:RegulatingControl .

cim:Tariff a rdfs:Class ;
    rdfs:label "Tariff" ;
    rdfs:comment "Document, approved by the responsible regulatory agency, listing the terms and conditions, including a schedule of prices, under which utility services will be provided. It has a unique number within the state or province. For rate schedules it is frequently allocated by the affiliated Public utilities commission (PUC)." ;
    rdfs:subClassOf cim:Document .

cim:TelephoneNumber a rdfs:Class ;
    rdfs:label "TelephoneNumber" ;
    rdfs:comment "Telephone number." .

cim:Temperature a rdfs:Class ;
    rdfs:label "Temperature" ;
    rdfs:comment "Value of temperature in degrees Celsius." .

cim:Terminal a rdfs:Class ;
    rdfs:label "Terminal" ;
    rdfs:comment "An AC electrical connection point to a piece of conducting equipment. Terminals are connected at physical connection points called connectivity nodes." ;
    rdfs:subClassOf cim:ACDCTerminal .

cim:TownDetail a rdfs:Class ;
    rdfs:label "TownDetail" ;
    rdfs:comment "Town details, in the context of address." .

cim:TransformerConstructionKind a rdfs:Class ;
    rdfs:label "TransformerConstructionKind" ;
    rdfs:comment "Kind of transformer construction." .

cim:TransformerCoolingType a rdfs:Class ;
    rdfs:label "TransformerCoolingType" ;
    rdfs:comment "\\[ZBEX\\] Transformer cooling types." .

cim:TransformerEnd a rdfs:Class ;
    rdfs:label "TransformerEnd" ;
    rdfs:comment "A conducting connection point of a power transformer. It corresponds to a physical transformer winding terminal.  In earlier CIM versions, the TransformerWinding class served a similar purpose, but this class is more flexible because it associates to terminal but is not a specialization of ConductingEquipment." ;
    rdfs:subClassOf cim:IdentifiedObject .

cim:TransformerEndInfo a rdfs:Class ;
    rdfs:label "TransformerEndInfo" ;
    rdfs:comment "Transformer end data." ;
    rdfs:subClassOf cim:AssetInfo .

cim:TransformerEndRatedS a rdfs:Class ;
    rdfs:label "TransformerEndRatedS" ;
    rdfs:comment "\\[ZBEX\\] Normal apparent power rating for a PowerTransformerEnd based on their cooling types." .

cim:TransformerFunctionKind a rdfs:Class ;
    rdfs:label "TransformerFunctionKind" ;
    rdfs:comment "Function of a transformer." .

cim:TransformerStarImpedance a rdfs:Class ;
    rdfs:label "TransformerStarImpedance" ;
    rdfs:comment "Transformer star impedance (Pi-model) that accurately reflects impedance for transformers with 2 or 3 windings. For transformers with 4 or more windings, TransformerMeshImpedance class shall be used.\nFor transmission networks use PowerTransformerEnd impedances (r, r0, x, x0, b, b0, g and g0)." ;
    rdfs:subClassOf cim:IdentifiedObject .

cim:TransformerTankInfo a rdfs:Class ;
    rdfs:label "TransformerTankInfo" ;
    rdfs:comment "Set of transformer tank data, from an equipment library." ;
    rdfs:subClassOf cim:AssetInfo .

cim:TransformerTest a rdfs:Class ;
    rdfs:label "TransformerTest" ;
    rdfs:comment "Test result for transformer ends, such as short-circuit, open-circuit (excitation) or no-load test." ;
    rdfs:subClassOf cim:IdentifiedObject .

cim:UnitSymbol a rdfs:Class ;
    rdfs:label "UnitSymbol" ;
    rdfs:comment "The derived units defined for usage in the CIM. In some cases, the derived unit is equal to an SI unit. Whenever possible, the standard derived symbol is used instead of the formula for the derived unit. For example, the unit symbol Farad is defined as \"F\" instead of \"CPerV\". In cases where a standard symbol does not exist for a derived unit, the formula for the unit is used as the unit symbol. For example, density does not have a standard symbol and so it is represented as \"kgPerm3\". With the exception of the \"kg\", which is an SI unit, the unit symbols do not contain multipliers and therefore represent the base derived unit to which a multiplier can be applied as a whole. \nEvery unit symbol is treated as an unparseable text as if it were a single-letter symbol. The meaning of each unit symbol is defined by the accompanying descriptive text and not by the text contents of the unit symbol.\nTo allow the widest possible range of serializations without requiring special character handling, several substitutions are made which deviate from the format described in IEC 80000-1. The division symbol \"/\" is replaced by the letters \"Per\". Exponents are written in plain text after the unit as \"m3\" instead of being formatted as \"m\" with a superscript of 3  or introducing a symbol as in \"m^3\". The degree symbol \"\" is replaced with the letters \"deg\". Any clarification of the meaning for a substitution is included in the description for the unit symbol.\nNon-SI units are included in list of unit symbols to allow sources of data to be correctly labelled with their non-SI units (for example, a GPS sensor that is reporting numbers that represent feet instead of meters). This allows software to use the unit symbol information correctly convert and scale the raw data of those sources into SI-based units. \nThe integer values are used for harmonization with IEC 61850." .

cim:UsagePoint a rdfs:Class ;
    rdfs:label "UsagePoint" ;
    rdfs:comment "Logical or physical point in the network to which readings or events may be attributed. Used at the place where a physical or virtual meter may be located; however, it is not required that a meter be present." ;
    rdfs:subClassOf cim:IdentifiedObject .

cim:VectorGroup a rdfs:Class ;
    rdfs:label "VectorGroup" ;
    rdfs:comment "\\[ZBEX\\] Vector group of the transformer for protective relaying, e.g., Dyn1. For unbalanced transformers, this may not be simply determined from the constituent winding connections and phase angle displacements.\nThe vectorGroup string consists of the following components in the order listed: high voltage winding connection, mid voltage winding connection (for three winding transformers), phase displacement clock number from 0 to 11, low voltage winding connection phase displacement clock number from 0 to 11.\nThe winding connections are D (delta), Y (wye), YN (wye with neutral), Z (zigzag), ZN (zigzag with neutral), A (auto transformer). Upper case means the high voltage, lower case mid or low. The high voltage winding always has clock position 0 and is not included in the vector group string.\nSome examples:\n                YNy0 (two winding wye to wye with no phase displacement),\n                YNd11 (two winding wye to delta with 330 degrees phase displacement),\n                YNyn0d5 (three winding transformer wye with neutral high voltage, wye with neutral mid\n                        voltage and no phase displacement, delta low voltage with 150 degrees displacement).\n\nPhase displacement is defined as the angular difference between the phasors representing the voltages between the neutral point (real or imaginary) and the corresponding terminals of two windings, a positive sequence voltage system being applied to the high-voltage terminals, following each other in alphabetical sequence if they are lettered, or in numerical sequence if they are numbered: the phasors are assumed to rotate in a counter-clockwise sense.\n" .

cim:Voltage a rdfs:Class ;
    rdfs:label "Voltage" ;
    rdfs:comment "Electrical voltage, can be both AC and DC." .

cim:VoltageRelay a rdfs:Class ;
    rdfs:label "VoltageRelay" ;
    rdfs:comment "[ZBEX] This extension is in-line with the CIM working group for replacing the `protection` package, can be replaced when the working group outcome is merged into the CIM model. <br/> A device that detects when the voltage in an AC circuit reaches a preset voltage. There are two basic types of voltage relay operation: overvoltage relay for overvoltage detection and undervoltage relay for undervoltage detection.\n" ;
    rdfs:subClassOf cim:ProtectionRelayFunction .

cim:WindingConnection a rdfs:Class ;
    rdfs:label "WindingConnection" ;
    rdfs:comment "Winding connection type." .

cim:WireInfo a rdfs:Class ;
    rdfs:label "WireInfo" ;
    rdfs:comment "Wire data that can be specified per line segment phase, or for the line segment as a whole in case its phases all have the same wire characteristics." ;
    rdfs:subClassOf cim:AssetInfo .

cim:WireMaterialKind a rdfs:Class ;
    rdfs:label "WireMaterialKind" ;
    rdfs:comment "Kind of wire material." .

cim:ACDCTerminal.Measurement a rdf:Property ;
    rdfs:label "ACDCTerminal.Measurement" ;
    rdfs:comment "One or more measurements may be associated with a terminal in the network. Measurements associated with this terminal defining  where the measurement is placed in the network topology.  It may be used, for instance, to capture the sensor position, such as a voltage transformer (PT) at a busbar or a current transformer (CT) at the bar between a breaker and an isolator." ;
    rdfs:domain cim:ACDCTerminal ;
    rdfs:range cim:Measurement ;
    profile:sourceCardinality "0..1" ;
    profile:targetCardinality "0..*" .

cim:AcLineSegment.Clamp a rdf:Property ;
    rdfs:label "AcLineSegment.Clamp" ;
    rdfs:comment "The line segment to which the clamp is connected. The clamps connected to the line segment." ;
    rdfs:domain cim:AcLineSegment ;
    rdfs:range cim:Clamp ;
    profile:sourceCardinality "0..1" ;
    profile:targetCardinality "0..*" .

cim:AcLineSegment.Cut a rdf:Property ;
    rdfs:label "AcLineSegment.Cut" ;
    rdfs:comment "The line segment to which the cut is applied. Cuts applied to the line segment." ;
    rdfs:domain cim:AcLineSegment ;
    rdfs:range cim:Cut ;
    profile:sourceCardinality "0..1" ;
    profile:targetCardinality "0..*" .

cim:AcLineSegment.PerLengthImpedance a rdf:Property ;
    rdfs:label "AcLineSegment.PerLengthImpedance" ;
    rdfs:comment "Per-length impedance of this line segment." ;
    rdfs:domain cim:AcLineSegment ;
    rdfs:range cim:PerLengthImpedance ;
    profile:targetCardinality "0..1" .

cim:AccumulatorValue.Accumulator a rdf:Property ;
    rdfs:label "AccumulatorValue.Accumulator" ;
    rdfs:comment "Measurement to which this value is connected." ;
    rdfs:domain cim:AccumulatorValue ;
    rdfs:range cim:Accumulator ;
    profile:targetCardinality "0..1" .

cim:AccumulatorValue.value a rdf:Property ;
    rdfs:label "value" ;
    rdfs:comment "The value to supervise. The value is positive." ;
    rdfs:domain cim:AccumulatorValue ;
    rdfs:range xsd:int .

cim:ActivePower.value a rdf:Property ;
    rdfs:label "value" ;
    rdfs:comment "watts (W)" ;
    rdfs:domain cim:ActivePower ;
    rdfs:range xsd:int .

cim:Agreement.validityInterval a rdf:Property ;
    rdfs:label "validityInterval" ;
    rdfs:comment "Date and time interval this agreement is valid (from going into effect to termination)." ;
    rdfs:domain cim:Agreement ;
    rdfs:range cim:DateTimeInterval .

cim:Analog.positiveFlowIn a rdf:Property ;
    rdfs:label "positiveFlowIn" ;
    rdfs:comment "If true then this measurement is an active power, reactive power or current with the convention that a positive value measured at the Terminal means power is flowing into the related PowerSystemResource." ;
    rdfs:domain cim:Analog ;
    rdfs:range xsd:boolean .

cim:AnalogValue.Analog a rdf:Property ;
    rdfs:label "AnalogValue.Analog" ;
    rdfs:comment "Measurement to which this value is connected." ;
    rdfs:domain cim:AnalogValue ;
    rdfs:range cim:Analog ;
    profile:targetCardinality "0..1" .

cim:AnalogValue.value a rdf:Property ;
    rdfs:label "value" ;
    rdfs:comment "The value to supervise." ;
    rdfs:domain cim:AnalogValue ;
    rdfs:range xsd:double .

cim:AngleDegrees.value a rdf:Property ;
    rdfs:label "value" ;
    rdfs:comment "degrees (deg)" ;
    rdfs:domain cim:AngleDegrees ;
    rdfs:range xsd:double .

cim:AngleRadians.value a rdf:Property ;
    rdfs:label "value" ;
    rdfs:comment "radians (rad)" ;
    rdfs:domain cim:AngleRadians ;
    rdfs:range xsd:double .

cim:ApparentPower.value a rdf:Property ;
    rdfs:label "value" ;
    rdfs:comment "volt amperes (VA)" ;
    rdfs:domain cim:ApparentPower ;
    rdfs:range xsd:int .

cim:Asset.AssetOrganisationRole a rdf:Property ;
    rdfs:label "Asset.AssetOrganisationRole" ;
    rdfs:comment "All roles an organisation plays for this asset." ;
    rdfs:domain cim:Asset ;
    rdfs:range cim:AssetOrganisationRole ;
    profile:targetCardinality "0..*" .

cim:Asset.Location a rdf:Property ;
    rdfs:label "Asset.Location" ;
    rdfs:comment "Location of this asset." ;
    rdfs:domain cim:Asset ;
    rdfs:range cim:Location ;
    profile:targetCardinality "0..1" .

cim:Asset.PowerSystemResource a rdf:Property ;
    rdfs:label "Asset.PowerSystemResource" ;
    rdfs:comment "All power system resources used to electrically model this asset. For example, transformer asset is electrically modelled with a transformer and its windings and tap changer." ;
    rdfs:domain cim:Asset ;
    rdfs:range cim:PowerSystemResource ;
    profile:targetCardinality "0..*" .

cim:AuxiliaryEquipment.Terminal a rdf:Property ;
    rdfs:label "AuxiliaryEquipment.Terminal" ;
    rdfs:comment "The Terminal at the equipment where the AuxiliaryEquipment is attached." ;
    rdfs:domain cim:AuxiliaryEquipment ;
    rdfs:range cim:Terminal ;
    profile:targetCardinality "0..1" .

cim:BaseVoltage.nominalVoltage a rdf:Property ;
    rdfs:label "nominalVoltage" ;
    rdfs:comment "The power system resource's base voltage.  Shall be a positive value and not zero." ;
    rdfs:domain cim:BaseVoltage ;
    rdfs:range cim:Voltage .

cim:BatteryControl.chargingRate a rdf:Property ;
    rdfs:label "chargingRate" ;
    rdfs:comment "\\[ZBEX\\] Charging rate (input power) in percentage of maxP. (Unit - Percent)" ;
    rdfs:domain cim:BatteryControl ;
    rdfs:range cim:PerCent .

cim:BatteryControl.controlMode a rdf:Property ;
    rdfs:label "controlMode" ;
    rdfs:comment "\\[ZBEX\\] Mode of operation for the dispatch (charging/discharging) function of BatteryControl." ;
    rdfs:domain cim:BatteryControl ;
    rdfs:range cim:BatteryControlMode .

cim:BatteryControl.dischargingRate a rdf:Property ;
    rdfs:label "dischargingRate" ;
    rdfs:comment "\\[ZBEX\\] Discharge rate (output power) in percentage of maxP. (Unit - Percent)" ;
    rdfs:domain cim:BatteryControl ;
    rdfs:range cim:PerCent .

cim:BatteryControl.reservePercent a rdf:Property ;
    rdfs:label "reservePercent" ;
    rdfs:comment "\\[ZBEX\\] Percentage of the rated storage capacity that should be reserved during normal operations. This reserve acts as a safeguard, preventing the energy level from dropping below this threshold under standard conditions. The field must be set to a non-negative value between 0 and 1. (Unit - Percent)" ;
    rdfs:domain cim:BatteryControl ;
    rdfs:range cim:PerCent .

cim:BatteryControlMode.UNKNOWN a rdf:Property ;
    rdfs:label "UNKNOWN" ;
    rdfs:comment "\\[ZBEX\\] Unknown control mode." ;
    rdfs:domain cim:BatteryControlMode ;
    rdfs:range xsd:string .

cim:BatteryControlMode.currentPeakShaveCharge a rdf:Property ;
    rdfs:label "currentPeakShaveCharge" ;
    rdfs:comment "\\[ZBEX\\] This mode initiates charging when the current (in Amps) at a monitored element falls below a specified threshold (minAllowedTargetValue). Similar to peakShaveCharge, this mode aims to manage demand effectively, but it operates based on current levels rather than power, providing finer control in systems where current management is prioritized." ;
    rdfs:domain cim:BatteryControlMode ;
    rdfs:range xsd:string .

cim:BatteryControlMode.currentPeakShaveDischarge a rdf:Property ;
    rdfs:label "currentPeakShaveDischarge" ;
    rdfs:comment "\\[ZBEX\\] This mode directs the BatteryUnit to discharge as needed to maintain the current (in amps) at a monitored element below a specified target. Similar to peakShaveDischarge, this mode aims to reduce demand peaks, focusing specifically on current levels to manage capacity and enhance system stability where current control is essential." ;
    rdfs:domain cim:BatteryControlMode ;
    rdfs:range xsd:string .

cim:BatteryControlMode.following a rdf:Property ;
    rdfs:label "following" ;
    rdfs:comment "\\[ZBEX\\] The control is triggered by time and resets the targetValue property to the present monitored element power." ;
    rdfs:domain cim:BatteryControlMode ;
    rdfs:range xsd:string .

cim:BatteryControlMode.peakShaveCharge a rdf:Property ;
    rdfs:label "peakShaveCharge" ;
    rdfs:comment "\\[ZBEX\\] This mode directs the BatteryUnit to initiate charging when the power level at a monitored element falls below a specified threshold (minAllowedTargetValue). This mode supports demand leveling by charging the BatteryUnit during low-demand periods, optimizing overall power management." ;
    rdfs:domain cim:BatteryControlMode ;
    rdfs:range xsd:string .

cim:BatteryControlMode.peakShaveDischarge a rdf:Property ;
    rdfs:label "peakShaveDischarge" ;
    rdfs:comment "\\[ZBEX\\] This mode directs the BatteryUnit to discharge as needed to maintain the power level of the monitored element within a defined range (specified by targetDeadband) or to keep it at or below the value specified by maxAllowedTargetValue. This mode helps prevent power spikes by discharging the BatteryUnit to manage peak demand effectively." ;
    rdfs:domain cim:BatteryControlMode ;
    rdfs:range xsd:string .

cim:BatteryControlMode.profile a rdf:Property ;
    rdfs:label "profile" ;
    rdfs:comment "\\[ZBEX\\] In this mode both discharging and charging precisely follow a per-unit curve." ;
    rdfs:domain cim:BatteryControlMode ;
    rdfs:range xsd:string .

cim:BatteryControlMode.schedule a rdf:Property ;
    rdfs:label "schedule" ;
    rdfs:comment "\\[ZBEX\\] In Schedule mode, a trapezoidal-shaped discharge schedule is specified through Tup (up ramp duration), TFlat (at duration), and Tdn (down ramp duration) properties." ;
    rdfs:domain cim:BatteryControlMode ;
    rdfs:range xsd:string .

cim:BatteryControlMode.support a rdf:Property ;
    rdfs:label "support" ;
    rdfs:comment "\\[ZBEX\\] This is essentially the opposite of peakShave modes. The fleet is dispatched to keep the power in the monitored terminal at or above targetValue." ;
    rdfs:domain cim:BatteryControlMode ;
    rdfs:range xsd:string .

cim:BatteryControlMode.time a rdf:Property ;
    rdfs:label "time" ;
    rdfs:comment "\\[ZBEX\\] In Time mode all storage elements are set to discharge when in the course of simulation the time of day passes the specified hour of day by the TimeDisChargeTrigger property (hour is a decimal value, e.g., 10.5 = 1030)" ;
    rdfs:domain cim:BatteryControlMode ;
    rdfs:range xsd:string .

cim:BatteryStateKind.UNKNOWN a rdf:Property ;
    rdfs:label "UNKNOWN" ;
    rdfs:comment "Battery state is unknown." ;
    rdfs:domain cim:BatteryStateKind ;
    rdfs:range xsd:string .

cim:BatteryStateKind.charging a rdf:Property ;
    rdfs:label "charging" ;
    rdfs:comment "Stored energy is increasing." ;
    rdfs:domain cim:BatteryStateKind ;
    rdfs:range xsd:string .

cim:BatteryStateKind.discharging a rdf:Property ;
    rdfs:label "discharging" ;
    rdfs:comment "Stored energy is decreasing." ;
    rdfs:domain cim:BatteryStateKind ;
    rdfs:range xsd:string .

cim:BatteryStateKind.empty a rdf:Property ;
    rdfs:label "empty" ;
    rdfs:comment "Unable to discharge, and not charging." ;
    rdfs:domain cim:BatteryStateKind ;
    rdfs:range xsd:string .

cim:BatteryStateKind.full a rdf:Property ;
    rdfs:label "full" ;
    rdfs:comment "Unable to charge, and not discharging." ;
    rdfs:domain cim:BatteryStateKind ;
    rdfs:range xsd:string .

cim:BatteryStateKind.waiting a rdf:Property ;
    rdfs:label "waiting" ;
    rdfs:comment "Neither charging nor discharging, but able to do so." ;
    rdfs:domain cim:BatteryStateKind ;
    rdfs:range xsd:string .

cim:BatteryUnit.BatteryControl a rdf:Property ;
    rdfs:label "BatteryUnit.BatteryControl" ;
    rdfs:comment "All controls present on this battery." ;
    rdfs:domain cim:BatteryUnit ;
    rdfs:range cim:BatteryControl ;
    profile:targetCardinality "0..*" .

cim:BatteryUnit.batteryState a rdf:Property ;
    rdfs:label "batteryState" ;
    rdfs:comment "The current state of the battery (charging, full, etc.)." ;
    rdfs:domain cim:BatteryUnit ;
    rdfs:range cim:BatteryStateKind .

cim:BatteryUnit.ratedE a rdf:Property ;
    rdfs:label "ratedE" ;
    rdfs:comment "Full energy storage capacity of the battery. The attribute shall be a positive value." ;
    rdfs:domain cim:BatteryUnit ;
    rdfs:range cim:RealEnergy .

cim:BatteryUnit.storedE a rdf:Property ;
    rdfs:label "storedE" ;
    rdfs:comment "Amount of energy currently stored. The attribute shall be a positive value or zero and lower than BatteryUnit.ratedE." ;
    rdfs:domain cim:BatteryUnit ;
    rdfs:range cim:RealEnergy .

cim:Breaker.inTransitTime a rdf:Property ;
    rdfs:label "inTransitTime" ;
    rdfs:comment "The transition time from open to close in seconds." ;
    rdfs:domain cim:Breaker ;
    rdfs:range cim:Seconds .

cim:Circuit.Loop a rdf:Property ;
    rdfs:label "Circuit.Loop" ;
    rdfs:comment "Sub-transmission circuits that form part of this loop. The loop containing this circuit." ;
    rdfs:domain cim:Circuit ;
    rdfs:range cim:Loop ;
    profile:sourceCardinality "0..*" ;
    profile:targetCardinality "0..1" .

cim:Circuit.Substation a rdf:Property ;
    rdfs:label "Circuit.Substation" ;
    rdfs:comment "Simplification of the CIM association via Bay to Substation Simplification of the CIM association via Bay to Circuit" ;
    rdfs:domain cim:Circuit ;
    rdfs:range cim:Substation ;
    profile:sourceCardinality "0..*" ;
    profile:targetCardinality "0..*" .

cim:Circuit.Terminal a rdf:Property ;
    rdfs:label "Circuit.Terminal" ;
    rdfs:comment "Circuit.Terminal" ;
    rdfs:domain cim:Circuit ;
    rdfs:range cim:Terminal ;
    profile:targetCardinality "0..*" .

cim:Clamp.AcLineSegment a rdf:Property ;
    rdfs:label "Clamp.AcLineSegment" ;
    rdfs:comment "The clamps connected to the line segment. The line segment to which the clamp is connected." ;
    rdfs:domain cim:Clamp ;
    rdfs:range cim:AcLineSegment ;
    profile:sourceCardinality "0..*" ;
    profile:targetCardinality "0..1" .

cim:Clamp.lengthFromTerminal1 a rdf:Property ;
    rdfs:label "lengthFromTerminal1" ;
    rdfs:comment "The length to the place where the clamp is located starting from side one of the line segment, i.e. the line segment terminal with sequence number equal to 1." ;
    rdfs:domain cim:Clamp ;
    rdfs:range cim:Length .

cim:Conductance.value a rdf:Property ;
    rdfs:label "value" ;
    rdfs:comment "siemens (S)" ;
    rdfs:domain cim:Conductance ;
    rdfs:range xsd:double .

cim:ConductancePerLength.value a rdf:Property ;
    rdfs:label "value" ;
    rdfs:comment "siemens per meter (SPerm)" ;
    rdfs:domain cim:ConductancePerLength ;
    rdfs:range xsd:double .

cim:ConductingEquipment.BaseVoltage a rdf:Property ;
    rdfs:label "ConductingEquipment.BaseVoltage" ;
    rdfs:comment "Base voltage of this conducting equipment.  Use only when there is no voltage level container used and only one base voltage applies.  For example, not used for transformers." ;
    rdfs:domain cim:ConductingEquipment ;
    rdfs:range cim:BaseVoltage ;
    profile:targetCardinality "0..1" .

cim:ConductingEquipment.Terminal a rdf:Property ;
    rdfs:label "ConductingEquipment.Terminal" ;
    rdfs:comment "The conducting equipment of the terminal.  Conducting equipment have  terminals that may be connected to other conducting equipment terminals via connectivity nodes or topological nodes. Conducting equipment have terminals that may be connected to other conducting equipment terminals via connectivity nodes or topological nodes." ;
    rdfs:domain cim:ConductingEquipment ;
    rdfs:range cim:Terminal ;
    profile:sourceCardinality "0..1" ;
    profile:targetCardinality "0..*" .

cim:Conductor.WireInfo a rdf:Property ;
    rdfs:label "Conductor.WireInfo" ;
    rdfs:comment "The conductor that uses this wire information. Wire characteristics applied to this conductor." ;
    rdfs:domain cim:Conductor ;
    rdfs:range cim:WireInfo ;
    profile:sourceCardinality "0..1" ;
    profile:targetCardinality "0..*" .

cim:Conductor.designRating a rdf:Property ;
    rdfs:label "designRating" ;
    rdfs:comment "\\[ZBEX\\] The current rating in Amperes at the specified design temperature that can be used without the conductor breaching physical network design limits." ;
    rdfs:domain cim:Conductor ;
    rdfs:range cim:CurrentFlow .

cim:Conductor.designTemperature a rdf:Property ;
    rdfs:label "designTemperature" ;
    rdfs:comment "\\[ZBEX\\] The temperature in degrees Celsius for the network design of this conductor. Values are limited to integers." ;
    rdfs:domain cim:Conductor ;
    rdfs:range cim:Temperature .

cim:Conductor.length a rdf:Property ;
    rdfs:label "length" ;
    rdfs:comment "Segment length for calculating line section capabilities." ;
    rdfs:domain cim:Conductor ;
    rdfs:range cim:Length .

cim:ConnectivityNode.Terminal a rdf:Property ;
    rdfs:label "ConnectivityNode.Terminal" ;
    rdfs:comment "The connectivity node to which this terminal connects with zero impedance. Terminals interconnected with zero impedance at a this connectivity node." ;
    rdfs:domain cim:ConnectivityNode ;
    rdfs:range cim:Terminal ;
    profile:sourceCardinality "0..1" ;
    profile:targetCardinality "0..*" .

cim:ContactDetails.ElectronicAddress a rdf:Property ;
    rdfs:label "ContactDetails.ElectronicAddress" ;
    rdfs:comment "\\[ZBEX\\] Electronic addresses." ;
    rdfs:domain cim:ContactDetails ;
    rdfs:range cim:ElectronicAddress ;
    profile:targetCardinality "0..1" .

cim:ContactDetails.StreetAddress a rdf:Property ;
    rdfs:label "ContactDetails.StreetAddress" ;
    rdfs:comment "\\[ZBEX\\] Contact address, potentially different than 'streetAddress' (e.g., another city)." ;
    rdfs:domain cim:ContactDetails ;
    rdfs:range cim:StreetAddress ;
    profile:targetCardinality "0..*" .

cim:ContactDetails.TelephoneNumber a rdf:Property ;
    rdfs:label "ContactDetails.TelephoneNumber" ;
    rdfs:comment "\\[ZBEX\\] Phone numbers." ;
    rdfs:domain cim:ContactDetails ;
    rdfs:range cim:TelephoneNumber ;
    profile:targetCardinality "0..*" .

cim:ContactDetails.businessName a rdf:Property ;
    rdfs:label "businessName" ;
    rdfs:comment "\\[ZBEX\\] The business name of this contact." ;
    rdfs:domain cim:ContactDetails ;
    rdfs:range xsd:string .

cim:ContactDetails.contactType a rdf:Property ;
    rdfs:label "contactType" ;
    rdfs:comment "\\[ZBEX\\] The type of contact, e.g Account Owner." ;
    rdfs:domain cim:ContactDetails ;
    rdfs:range xsd:string .

cim:ContactDetails.firstName a rdf:Property ;
    rdfs:label "firstName" ;
    rdfs:comment "\\[ZBEX\\] First name of the contact." ;
    rdfs:domain cim:ContactDetails ;
    rdfs:range xsd:string .

cim:ContactDetails.id a rdf:Property ;
    rdfs:label "id" ;
    rdfs:comment "\\[ZBEX\\] The identifier for this contact, could be autogenerated." ;
    rdfs:domain cim:ContactDetails ;
    rdfs:range xsd:string .

cim:ContactDetails.isPrimary a rdf:Property ;
    rdfs:label "isPrimary" ;
    rdfs:comment "\\[ZBEX\\] Whether this contact is a primary contact." ;
    rdfs:domain cim:ContactDetails ;
    rdfs:range xsd:boolean .

cim:ContactDetails.lastName a rdf:Property ;
    rdfs:label "lastName" ;
    rdfs:comment "\\[ZBEX\\] Last name of the contact." ;
    rdfs:domain cim:ContactDetails ;
    rdfs:range xsd:string .

cim:ContactDetails.preferredContactMethod a rdf:Property ;
    rdfs:label "preferredContactMethod" ;
    rdfs:comment "\\[ZBEX\\] The preferred contact method for this contact." ;
    rdfs:domain cim:ContactDetails ;
    rdfs:range cim:ContactMethodType .

cim:ContactMethodType.CALL a rdf:Property ;
    rdfs:label "CALL" ;
    rdfs:comment "\\[ZBEX\\] Contact by call using the primary phone number." ;
    rdfs:domain cim:ContactMethodType ;
    rdfs:range xsd:string .

cim:ContactMethodType.EMAIL a rdf:Property ;
    rdfs:label "EMAIL" ;
    rdfs:comment "\\[ZBEX\\] Contact via email using the primary address." ;
    rdfs:domain cim:ContactMethodType ;
    rdfs:range xsd:string .

cim:ContactMethodType.LETTER a rdf:Property ;
    rdfs:label "LETTER" ;
    rdfs:comment "\\[ZBEX\\] Letter by post to the contact address is the method of contact." ;
    rdfs:domain cim:ContactMethodType ;
    rdfs:range xsd:string .

cim:ContactMethodType.UNKNOWN a rdf:Property ;
    rdfs:label "UNKNOWN" ;
    rdfs:comment "\\[ZBEX\\] Unknown contact method type." ;
    rdfs:domain cim:ContactMethodType ;
    rdfs:range xsd:string .

cim:Control.PowerSystemResource a rdf:Property ;
    rdfs:label "Control.PowerSystemResource" ;
    rdfs:comment "The controller outputs used to actually govern a regulating device, e.g. the magnetization of a synchronous machine or capacitor bank breaker actuator. Regulating device governed by this control output." ;
    rdfs:domain cim:Control ;
    rdfs:range cim:PowerSystemResource ;
    profile:sourceCardinality "0..*" ;
    profile:targetCardinality "0..1" .

cim:Control.RemoteControl a rdf:Property ;
    rdfs:label "Control.RemoteControl" ;
    rdfs:comment "The Control for the RemoteControl point. The remote point controlling the physical actuator." ;
    rdfs:domain cim:Control ;
    rdfs:range cim:RemoteControl ;
    profile:sourceCardinality "0..1" ;
    profile:targetCardinality "0..1" .

cim:ControlledAppliance.isElectricVehicle a rdf:Property ;
    rdfs:label "isElectricVehicle" ;
    rdfs:comment "True if the appliance is an electric vehicle." ;
    rdfs:domain cim:ControlledAppliance ;
    rdfs:range xsd:boolean .

cim:ControlledAppliance.isExteriorLighting a rdf:Property ;
    rdfs:label "isExteriorLighting" ;
    rdfs:comment "True if the appliance is exterior lighting." ;
    rdfs:domain cim:ControlledAppliance ;
    rdfs:range xsd:boolean .

cim:ControlledAppliance.isGenerationSystem a rdf:Property ;
    rdfs:label "isGenerationSystem" ;
    rdfs:comment "True if the appliance is a generation system." ;
    rdfs:domain cim:ControlledAppliance ;
    rdfs:range xsd:boolean .

cim:ControlledAppliance.isHvacCompressorOrFurnace a rdf:Property ;
    rdfs:label "isHvacCompressorOrFurnace" ;
    rdfs:comment "True if the appliance is HVAC compressor or furnace." ;
    rdfs:domain cim:ControlledAppliance ;
    rdfs:range xsd:boolean .

cim:ControlledAppliance.isInteriorLighting a rdf:Property ;
    rdfs:label "isInteriorLighting" ;
    rdfs:comment "True if the appliance is interior lighting." ;
    rdfs:domain cim:ControlledAppliance ;
    rdfs:range xsd:boolean .

cim:ControlledAppliance.isIrrigationPump a rdf:Property ;
    rdfs:label "isIrrigationPump" ;
    rdfs:comment "True if the appliance is an irrigation pump." ;
    rdfs:domain cim:ControlledAppliance ;
    rdfs:range xsd:boolean .

cim:ControlledAppliance.isManagedCommercialIndustrialLoad a rdf:Property ;
    rdfs:label "isManagedCommercialIndustrialLoad" ;
    rdfs:comment "True if the appliance is managed commercial or industrial load." ;
    rdfs:domain cim:ControlledAppliance ;
    rdfs:range xsd:boolean .

cim:ControlledAppliance.isPoolPumpSpaJacuzzi a rdf:Property ;
    rdfs:label "isPoolPumpSpaJacuzzi" ;
    rdfs:comment "True if the appliance is a pool, pump, spa or jacuzzi." ;
    rdfs:domain cim:ControlledAppliance ;
    rdfs:range xsd:boolean .

cim:ControlledAppliance.isSimpleMiscLoad a rdf:Property ;
    rdfs:label "isSimpleMiscLoad" ;
    rdfs:comment "True if the appliance is a simple miscellaneous load." ;
    rdfs:domain cim:ControlledAppliance ;
    rdfs:range xsd:boolean .

cim:ControlledAppliance.isSmartAppliance a rdf:Property ;
    rdfs:label "isSmartAppliance" ;
    rdfs:comment "True if the appliance is a smart appliance." ;
    rdfs:domain cim:ControlledAppliance ;
    rdfs:range xsd:boolean .

cim:ControlledAppliance.isStripAndBaseboardHeater a rdf:Property ;
    rdfs:label "isStripAndBaseboardHeater" ;
    rdfs:comment "True if the appliance is a strip or baseboard heater." ;
    rdfs:domain cim:ControlledAppliance ;
    rdfs:range xsd:boolean .

cim:ControlledAppliance.isWaterHeater a rdf:Property ;
    rdfs:label "isWaterHeater" ;
    rdfs:comment "True if the appliance is a water heater." ;
    rdfs:domain cim:ControlledAppliance ;
    rdfs:range xsd:boolean .

cim:CurrentFlow.value a rdf:Property ;
    rdfs:label "value" ;
    rdfs:comment "amperes (A)" ;
    rdfs:domain cim:CurrentFlow ;
    rdfs:range xsd:double .

cim:CurrentRelay.currentLimit1 a rdf:Property ;
    rdfs:label "currentLimit1" ;
    rdfs:comment "Current limit number one 1 for inverse time pickup." ;
    rdfs:domain cim:CurrentRelay ;
    rdfs:range cim:CurrentFlow .

cim:CurrentRelay.inverseTimeFlag a rdf:Property ;
    rdfs:label "inverseTimeFlag" ;
    rdfs:comment "Set true if the current relay has inverse time characteristic." ;
    rdfs:domain cim:CurrentRelay ;
    rdfs:range xsd:boolean .

cim:CurrentRelay.timeDelay1 a rdf:Property ;
    rdfs:label "timeDelay1" ;
    rdfs:comment "Inverse time delay number 1 for current limit number 1." ;
    rdfs:domain cim:CurrentRelay ;
    rdfs:range cim:Seconds .

cim:CurrentTransformer.coreBurden a rdf:Property ;
    rdfs:label "coreBurden" ;
    rdfs:comment "Power burden of the CT core." ;
    rdfs:domain cim:CurrentTransformer ;
    rdfs:range cim:ActivePower .

cim:CurrentTransformerInfo.accuracyClass a rdf:Property ;
    rdfs:label "accuracyClass" ;
    rdfs:comment "CT accuracy classification." ;
    rdfs:domain cim:CurrentTransformerInfo ;
    rdfs:range xsd:string .

cim:CurrentTransformerInfo.accuracyLimit a rdf:Property ;
    rdfs:label "accuracyLimit" ;
    rdfs:comment "Accuracy limit." ;
    rdfs:domain cim:CurrentTransformerInfo ;
    rdfs:range cim:CurrentFlow .

cim:CurrentTransformerInfo.coreCount a rdf:Property ;
    rdfs:label "coreCount" ;
    rdfs:comment "Number of cores." ;
    rdfs:domain cim:CurrentTransformerInfo ;
    rdfs:range xsd:int .

cim:CurrentTransformerInfo.ctClass a rdf:Property ;
    rdfs:label "ctClass" ;
    rdfs:comment "" ;
    rdfs:domain cim:CurrentTransformerInfo ;
    rdfs:range xsd:string .

cim:CurrentTransformerInfo.kneePointVoltage a rdf:Property ;
    rdfs:label "kneePointVoltage" ;
    rdfs:comment "Maximum voltage across the secondary terminals where the CT still displays linear characteristicts." ;
    rdfs:domain cim:CurrentTransformerInfo ;
    rdfs:range cim:Voltage .

cim:CurrentTransformerInfo.maxRatio a rdf:Property ;
    rdfs:label "maxRatio" ;
    rdfs:comment "Maximum ratio between the primary and secondary current." ;
    rdfs:domain cim:CurrentTransformerInfo ;
    rdfs:range cim:Ratio .

cim:CurrentTransformerInfo.nominalRatio a rdf:Property ;
    rdfs:label "nominalRatio" ;
    rdfs:comment "Nominal ratio between the primary and secondary current; i.e. 100:5." ;
    rdfs:domain cim:CurrentTransformerInfo ;
    rdfs:range cim:Ratio .

cim:CurrentTransformerInfo.primaryRatio a rdf:Property ;
    rdfs:label "primaryRatio" ;
    rdfs:comment "Ratio for the primary winding tap changer." ;
    rdfs:domain cim:CurrentTransformerInfo ;
    rdfs:range cim:Ratio .

cim:CurrentTransformerInfo.ratedCurrent a rdf:Property ;
    rdfs:label "ratedCurrent" ;
    rdfs:comment "Rated current on the primary side." ;
    rdfs:domain cim:CurrentTransformerInfo ;
    rdfs:range cim:CurrentFlow .

cim:CurrentTransformerInfo.secondaryFlsRating a rdf:Property ;
    rdfs:label "secondaryFlsRating" ;
    rdfs:comment "Full load secondary (FLS) rating for secondary winding." ;
    rdfs:domain cim:CurrentTransformerInfo ;
    rdfs:range cim:CurrentFlow .

cim:CurrentTransformerInfo.secondaryRatio a rdf:Property ;
    rdfs:label "secondaryRatio" ;
    rdfs:comment "Ratio for the secondary winding tap changer." ;
    rdfs:domain cim:CurrentTransformerInfo ;
    rdfs:range cim:Ratio .

cim:CurrentTransformerInfo.usage a rdf:Property ;
    rdfs:label "usage" ;
    rdfs:comment "Usage: eg. metering, protection, etc." ;
    rdfs:domain cim:CurrentTransformerInfo ;
    rdfs:range xsd:string .

cim:Curve.CurveData a rdf:Property ;
    rdfs:label "Curve.CurveData" ;
    rdfs:comment "The point data values that define this curve." ;
    rdfs:domain cim:Curve ;
    rdfs:range cim:CurveData ;
    profile:targetCardinality "0..*" .

cim:CurveData.xvalue a rdf:Property ;
    rdfs:label "xvalue" ;
    rdfs:comment "The data value of the X-axis variable, depending on the X-axis units." ;
    rdfs:domain cim:CurveData ;
    rdfs:range xsd:double .

cim:CurveData.y1value a rdf:Property ;
    rdfs:label "y1value" ;
    rdfs:comment "The data value of the first Y-axis variable, depending on the Y-axis units." ;
    rdfs:domain cim:CurveData ;
    rdfs:range xsd:double .

cim:CurveData.y2value a rdf:Property ;
    rdfs:label "y2value" ;
    rdfs:comment "The data value of the second Y-axis variable (if present), depending on the Y-axis units." ;
    rdfs:domain cim:CurveData ;
    rdfs:range xsd:double .

cim:CurveData.y3value a rdf:Property ;
    rdfs:label "y3value" ;
    rdfs:comment "The data value of the third Y-axis variable (if present), depending on the Y-axis units." ;
    rdfs:domain cim:CurveData ;
    rdfs:range xsd:double .

cim:Customer.CustomerAgreement a rdf:Property ;
    rdfs:label "Customer.CustomerAgreement" ;
    rdfs:comment "Customer for this agreement. All agreements of this customer." ;
    rdfs:domain cim:Customer ;
    rdfs:range cim:CustomerAgreement ;
    profile:sourceCardinality "0..1" ;
    profile:targetCardinality "0..*" .

cim:Customer.kind a rdf:Property ;
    rdfs:label "kind" ;
    rdfs:comment "Kind of customer." ;
    rdfs:domain cim:Customer ;
    rdfs:range cim:CustomerKind .

cim:Customer.numEndDevices a rdf:Property ;
    rdfs:label "numEndDevices" ;
    rdfs:comment "Count of the EndDevice's that are associated with this Customer." ;
    rdfs:domain cim:Customer ;
    rdfs:range xsd:int .

cim:Customer.specialNeed a rdf:Property ;
    rdfs:label "specialNeed" ;
    rdfs:comment "True if customer organisation has special service needs such as life support, hospitals, etc." ;
    rdfs:domain cim:Customer ;
    rdfs:range xsd:string .

cim:CustomerAgreement.Customer a rdf:Property ;
    rdfs:label "CustomerAgreement.Customer" ;
    rdfs:comment "All agreements of this customer. Customer for this agreement." ;
    rdfs:domain cim:CustomerAgreement ;
    rdfs:range cim:Customer ;
    profile:sourceCardinality "0..*" ;
    profile:targetCardinality "0..1" .

cim:CustomerAgreement.PricingStructure a rdf:Property ;
    rdfs:label "CustomerAgreement.PricingStructure" ;
    rdfs:comment "All pricing structures applicable to this customer agreement." ;
    rdfs:domain cim:CustomerAgreement ;
    rdfs:range cim:PricingStructure ;
    profile:targetCardinality "0..*" .

cim:CustomerKind.UNKNOWN a rdf:Property ;
    rdfs:label "UNKNOWN" ;
    rdfs:comment "" ;
    rdfs:domain cim:CustomerKind ;
    rdfs:range xsd:string .

cim:CustomerKind.commercialIndustrial a rdf:Property ;
    rdfs:label "commercialIndustrial" ;
    rdfs:comment "Commercial industrial customer." ;
    rdfs:domain cim:CustomerKind ;
    rdfs:range xsd:string .

cim:CustomerKind.energyServiceScheduler a rdf:Property ;
    rdfs:label "energyServiceScheduler" ;
    rdfs:comment "Customer as energy service scheduler." ;
    rdfs:domain cim:CustomerKind ;
    rdfs:range xsd:string .

cim:CustomerKind.energyServiceSupplier a rdf:Property ;
    rdfs:label "energyServiceSupplier" ;
    rdfs:comment "Customer as energy service supplier." ;
    rdfs:domain cim:CustomerKind ;
    rdfs:range xsd:string .

cim:CustomerKind.enterprise a rdf:Property ;
    rdfs:label "enterprise" ;
    rdfs:comment "" ;
    rdfs:domain cim:CustomerKind ;
    rdfs:range xsd:string .

cim:CustomerKind.internalUse a rdf:Property ;
    rdfs:label "internalUse" ;
    rdfs:comment "Internal use customer." ;
    rdfs:domain cim:CustomerKind ;
    rdfs:range xsd:string .

cim:CustomerKind.other a rdf:Property ;
    rdfs:label "other" ;
    rdfs:comment "Other kind of customer." ;
    rdfs:domain cim:CustomerKind ;
    rdfs:range xsd:string .

cim:CustomerKind.pumpingLoad a rdf:Property ;
    rdfs:label "pumpingLoad" ;
    rdfs:comment "Pumping load customer." ;
    rdfs:domain cim:CustomerKind ;
    rdfs:range xsd:string .

cim:CustomerKind.regionalOperator a rdf:Property ;
    rdfs:label "regionalOperator" ;
    rdfs:comment "" ;
    rdfs:domain cim:CustomerKind ;
    rdfs:range xsd:string .

cim:CustomerKind.residential a rdf:Property ;
    rdfs:label "residential" ;
    rdfs:comment "Residential customer." ;
    rdfs:domain cim:CustomerKind ;
    rdfs:range xsd:string .

cim:CustomerKind.residentialAndCommercial a rdf:Property ;
    rdfs:label "residentialAndCommercial" ;
    rdfs:comment "Residential and commercial customer." ;
    rdfs:domain cim:CustomerKind ;
    rdfs:range xsd:string .

cim:CustomerKind.residentialAndStreetlight a rdf:Property ;
    rdfs:label "residentialAndStreetlight" ;
    rdfs:comment "Residential and streetlight customer." ;
    rdfs:domain cim:CustomerKind ;
    rdfs:range xsd:string .

cim:CustomerKind.residentialFarmService a rdf:Property ;
    rdfs:label "residentialFarmService" ;
    rdfs:comment "Residential farm service customer." ;
    rdfs:domain cim:CustomerKind ;
    rdfs:range xsd:string .

cim:CustomerKind.residentialStreetlightOthers a rdf:Property ;
    rdfs:label "residentialStreetlightOthers" ;
    rdfs:comment "Residential streetlight or other related customer." ;
    rdfs:domain cim:CustomerKind ;
    rdfs:range xsd:string .

cim:CustomerKind.subsidiary a rdf:Property ;
    rdfs:label "subsidiary" ;
    rdfs:comment "" ;
    rdfs:domain cim:CustomerKind ;
    rdfs:range xsd:string .

cim:CustomerKind.windMachine a rdf:Property ;
    rdfs:label "windMachine" ;
    rdfs:comment "Wind machine customer." ;
    rdfs:domain cim:CustomerKind ;
    rdfs:range xsd:string .

cim:Cut.AcLineSegment a rdf:Property ;
    rdfs:label "Cut.AcLineSegment" ;
    rdfs:comment "Cuts applied to the line segment. The line segment to which the cut is applied." ;
    rdfs:domain cim:Cut ;
    rdfs:range cim:AcLineSegment ;
    profile:sourceCardinality "0..*" ;
    profile:targetCardinality "0..1" .

cim:Cut.lengthFromTerminal1 a rdf:Property ;
    rdfs:label "lengthFromTerminal1" ;
    rdfs:comment "The length to the place where the cut is located starting from side one of the cut line segment, i.e. the line segment Terminal with sequenceNumber equal to 1." ;
    rdfs:domain cim:Cut ;
    rdfs:range cim:Length .

cim:DateTimeInterval.end a rdf:Property ;
    rdfs:label "end" ;
    rdfs:comment "End date and time of this interval.  The end date and time where the interval is defined up to, but excluded." ;
    rdfs:domain cim:DateTimeInterval ;
    rdfs:range cim:DateTime .

cim:DateTimeInterval.start a rdf:Property ;
    rdfs:label "start" ;
    rdfs:comment "Start date and time of this interval.  The start date and time is included in the defined interval." ;
    rdfs:domain cim:DateTimeInterval ;
    rdfs:range cim:DateTime .

cim:Diagram.DiagramObject a rdf:Property ;
    rdfs:label "Diagram.DiagramObject" ;
    rdfs:comment "A diagram object is part of a diagram. A diagram is made up of multiple diagram objects." ;
    rdfs:domain cim:Diagram ;
    rdfs:range cim:DiagramObject ;
    profile:sourceCardinality "0..1" ;
    profile:targetCardinality "0..*" .

cim:Diagram.diagramStyle a rdf:Property ;
    rdfs:label "diagramStyle" ;
    rdfs:comment "A Diagram may have a DiagramStyle." ;
    rdfs:domain cim:Diagram ;
    rdfs:range cim:DiagramStyle .

cim:Diagram.orientation a rdf:Property ;
    rdfs:label "orientation" ;
    rdfs:comment "Coordinate system orientation of the diagram. A positive orientation gives standard right-hand orientation, with negative orientation indicating a left-hand orientation. For 2D diagrams, a positive orientation will result in X values increasing from left to right and Y values increasing from bottom to top. A negative orientation gives the left-hand orientation (favoured by computer graphics displays) with X values increasing from left to right and Y values increasing from top to bottom." ;
    rdfs:domain cim:Diagram ;
    rdfs:range cim:OrientationKind .

cim:DiagramObject.Diagram a rdf:Property ;
    rdfs:label "DiagramObject.Diagram" ;
    rdfs:comment "A diagram is made up of multiple diagram objects. A diagram object is part of a diagram." ;
    rdfs:domain cim:DiagramObject ;
    rdfs:range cim:Diagram ;
    profile:sourceCardinality "0..*" ;
    profile:targetCardinality "0..1" .

cim:DiagramObject.DiagramObjectPoint a rdf:Property ;
    rdfs:label "DiagramObject.DiagramObjectPoint" ;
    rdfs:comment "A diagram object can have 0 or more points to reflect its layout position, routing (for polylines) or boundary (for polygons)." ;
    rdfs:domain cim:DiagramObject ;
    rdfs:range cim:DiagramObjectPoint ;
    profile:targetCardinality "0..*" .

cim:DiagramObject.IdentifiedObject a rdf:Property ;
    rdfs:label "DiagramObject.IdentifiedObject" ;
    rdfs:comment "The domain object to which this diagram object is associated." ;
    rdfs:domain cim:DiagramObject ;
    rdfs:range cim:IdentifiedObject ;
    profile:targetCardinality "0..1" .

cim:DiagramObject.diagramObjectStyle a rdf:Property ;
    rdfs:label "diagramObjectStyle" ;
    rdfs:comment "A diagram object has a style associated that provides a reference for the style used in the originating system." ;
    rdfs:domain cim:DiagramObject ;
    rdfs:range xsd:string .

cim:DiagramObject.rotation a rdf:Property ;
    rdfs:label "rotation" ;
    rdfs:comment "Sets the angle of rotation of the diagram object.  Zero degrees is pointing to the top of the diagram.  Rotation is clockwise.  DiagramObject.rotation=0 has the following meaning: The connection point of an element which has one terminal is pointing to the top side of the diagram. The connection point \"From side\" of an element which has more than one terminal is pointing to the top side of the diagram.\nDiagramObject.rotation=90 has the following meaning: The connection point of an element which has one terminal is pointing to the right hand side of the diagram. The connection point \"From side\" of an element which has more than one terminal is pointing to the right hand side of the diagram." ;
    rdfs:domain cim:DiagramObject ;
    rdfs:range cim:AngleDegrees .

cim:DiagramObjectPoint.xPosition a rdf:Property ;
    rdfs:label "xPosition" ;
    rdfs:comment "The X coordinate of this point." ;
    rdfs:domain cim:DiagramObjectPoint ;
    rdfs:range xsd:double .

cim:DiagramObjectPoint.yPosition a rdf:Property ;
    rdfs:label "yPosition" ;
    rdfs:comment "" ;
    rdfs:domain cim:DiagramObjectPoint ;
    rdfs:range xsd:double .

cim:DiagramStyle.GEOGRAPHIC a rdf:Property ;
    rdfs:label "GEOGRAPHIC" ;
    rdfs:comment "The diagram should be styled as a geographic view." ;
    rdfs:domain cim:DiagramStyle ;
    rdfs:range xsd:string .

cim:DiagramStyle.SCHEMATIC a rdf:Property ;
    rdfs:label "SCHEMATIC" ;
    rdfs:comment "The diagram should be styled as a schematic view." ;
    rdfs:domain cim:DiagramStyle ;
    rdfs:range xsd:string .

cim:DirectionalCurrentRelay.currentLimit1 a rdf:Property ;
    rdfs:label "currentLimit1" ;
    rdfs:comment "\\[ZBEX\\] Current limit number 1 for inverse time pickup in amperes." ;
    rdfs:domain cim:DirectionalCurrentRelay ;
    rdfs:range cim:CurrentFlow .

cim:DirectionalCurrentRelay.directionalCharacteristicAngle a rdf:Property ;
    rdfs:label "directionalCharacteristicAngle" ;
    rdfs:comment "\\[ZBEX\\] The characteristic angle (in degrees) that defines the boundary between the operate and restrain regions of the directional element, relative to the polarizing quantity. Often referred to as Maximum Torque Angle (MTA) or Relay Characteristic Angle (RCA)." ;
    rdfs:domain cim:DirectionalCurrentRelay ;
    rdfs:range cim:AngleDegrees .

cim:DirectionalCurrentRelay.inverseTimeFlag a rdf:Property ;
    rdfs:label "inverseTimeFlag" ;
    rdfs:comment "\\[ZBEX\\] Set true if the current relay has inverse time characteristic." ;
    rdfs:domain cim:DirectionalCurrentRelay ;
    rdfs:range xsd:boolean .

cim:DirectionalCurrentRelay.minimumPickupCurrent a rdf:Property ;
    rdfs:label "minimumPickupCurrent" ;
    rdfs:comment "\\[ZBEX\\] The minimum current magnitude required for the directional element to operate reliably and determine direction. This might be different from the main pickupCurrent for the overcurrent function." ;
    rdfs:domain cim:DirectionalCurrentRelay ;
    rdfs:range cim:CurrentFlow .

cim:DirectionalCurrentRelay.polarizingQuantityType a rdf:Property ;
    rdfs:label "polarizingQuantityType" ;
    rdfs:comment "\\[ZBEX\\] Specifies the type of voltage to be used for polarization. This guides the selection/derivation of voltage from the VTs." ;
    rdfs:domain cim:DirectionalCurrentRelay ;
    rdfs:range cim:PolarizingQuantityType .

cim:DirectionalCurrentRelay.relayElementPhase a rdf:Property ;
    rdfs:label "relayElementPhase" ;
    rdfs:comment "\\[ZBEX\\] The phase associated with this directional relay element. This helps in selecting the correct 'self-phase' or other phase-derived." ;
    rdfs:domain cim:DirectionalCurrentRelay ;
    rdfs:range cim:PhaseCode .

cim:DirectionalCurrentRelay.timeDelay1 a rdf:Property ;
    rdfs:label "timeDelay1" ;
    rdfs:comment "\\[ZBEX\\] Inverse time delay number 1 for current limit number 1 in seconds." ;
    rdfs:domain cim:DirectionalCurrentRelay ;
    rdfs:range cim:Seconds .

cim:DiscreteValue.Discrete a rdf:Property ;
    rdfs:label "DiscreteValue.Discrete" ;
    rdfs:comment "Measurement to which this value is connected." ;
    rdfs:domain cim:DiscreteValue ;
    rdfs:range cim:Discrete ;
    profile:targetCardinality "0..1" .

cim:DiscreteValue.value a rdf:Property ;
    rdfs:label "value" ;
    rdfs:comment "The value to supervise." ;
    rdfs:domain cim:DiscreteValue ;
    rdfs:range xsd:int .

cim:DistanceRelay.backwardBlind a rdf:Property ;
    rdfs:label "backwardBlind" ;
    rdfs:comment "\\[ZBEX\\] The reverse blind impedance (in ohms) that defines the area to be blinded in the opposite direction of the power flow." ;
    rdfs:domain cim:DistanceRelay ;
    rdfs:range cim:Impedance .

cim:DistanceRelay.backwardReach a rdf:Property ;
    rdfs:label "backwardReach" ;
    rdfs:comment "\\[ZBEX\\] The reverse reach impedance (in ohms) that determines the maximum distance along the transmission line in the opposite direction of power flow for which the relay will provide protection." ;
    rdfs:domain cim:DistanceRelay ;
    rdfs:range cim:Impedance .

cim:DistanceRelay.backwardReactance a rdf:Property ;
    rdfs:label "backwardReactance" ;
    rdfs:comment "\\[ZBEX\\] The reverse reactance (in ohms) that determines the maximum distance along the transmission line in the opposite direction of power flow for which the relay will provide protection." ;
    rdfs:domain cim:DistanceRelay ;
    rdfs:range cim:Reactance .

cim:DistanceRelay.forwardBlind a rdf:Property ;
    rdfs:label "forwardBlind" ;
    rdfs:comment "\\[ZBEX\\] The forward blind impedance (in ohms) that defines the area to be blinded in the opposite direction of the power flow." ;
    rdfs:domain cim:DistanceRelay ;
    rdfs:range cim:Impedance .

cim:DistanceRelay.forwardReach a rdf:Property ;
    rdfs:label "forwardReach" ;
    rdfs:comment "\\[ZBEX\\] The forward reach impedance (in ohms) that determines the maximum distance along the transmission line in the opposite direction of power flow for which the relay will provide protection." ;
    rdfs:domain cim:DistanceRelay ;
    rdfs:range cim:Impedance .

cim:DistanceRelay.forwardReactance a rdf:Property ;
    rdfs:label "forwardReactance" ;
    rdfs:comment "\\[ZBEX\\] The forward reactance (in ohms) that determines the maximum distance along the transmission line in the opposite direction of power flow for which the relay will provide protection." ;
    rdfs:domain cim:DistanceRelay ;
    rdfs:range cim:Reactance .

cim:DistanceRelay.operationPhaseAngle1 a rdf:Property ;
    rdfs:label "operationPhaseAngle1" ;
    rdfs:comment "\\[ZBEX\\] The phase angle (in degrees) between voltage and current during normal operating conditions for zone 1 relay." ;
    rdfs:domain cim:DistanceRelay ;
    rdfs:range cim:AngleDegrees .

cim:DistanceRelay.operationPhaseAngle2 a rdf:Property ;
    rdfs:label "operationPhaseAngle2" ;
    rdfs:comment "\\[ZBEX\\] The phase angle (in degrees) between voltage and current during normal operating conditions for zone 2 relay." ;
    rdfs:domain cim:DistanceRelay ;
    rdfs:range cim:AngleDegrees .

cim:DistanceRelay.operationPhaseAngle3 a rdf:Property ;
    rdfs:label "operationPhaseAngle3" ;
    rdfs:comment "\\[ZBEX\\] The phase angle (in degrees) between voltage and current during normal operating conditions for zone 3 relay." ;
    rdfs:domain cim:DistanceRelay ;
    rdfs:range cim:AngleDegrees .

cim:Document.authorName a rdf:Property ;
    rdfs:label "authorName" ;
    rdfs:comment "Name of the author of this document." ;
    rdfs:domain cim:Document ;
    rdfs:range xsd:string .

cim:Document.comment a rdf:Property ;
    rdfs:label "comment" ;
    rdfs:comment "Free text comment." ;
    rdfs:domain cim:Document ;
    rdfs:range xsd:string .

cim:Document.createdDateTime a rdf:Property ;
    rdfs:label "createdDateTime" ;
    rdfs:comment "Date and time that this document was created." ;
    rdfs:domain cim:Document ;
    rdfs:range cim:DateTime .

cim:Document.status a rdf:Property ;
    rdfs:label "status" ;
    rdfs:comment "Status of subject matter (e.g., Agreement, Work) this document represents. For status of the document itself, use 'docStatus' attribute." ;
    rdfs:domain cim:Document ;
    rdfs:range cim:Status .

cim:Document.title a rdf:Property ;
    rdfs:label "title" ;
    rdfs:comment "Document title." ;
    rdfs:domain cim:Document ;
    rdfs:range xsd:string .

cim:Document.type a rdf:Property ;
    rdfs:label "type" ;
    rdfs:comment "Utility-specific classification of this document, according to its corporate standards, practices, and existing IT systems (e.g., for management of assets, maintenance, work, outage, customers, etc.)." ;
    rdfs:domain cim:Document ;
    rdfs:range xsd:string .

cim:EarthFaultCompensator.r a rdf:Property ;
    rdfs:label "r" ;
    rdfs:comment "Nominal resistance of device in ohms." ;
    rdfs:domain cim:EarthFaultCompensator ;
    rdfs:range cim:Resistance .

cim:ElectronicAddress.description a rdf:Property ;
    rdfs:label "description" ;
    rdfs:comment "[ZBEX] A description for this email, e.g: work, personal." ;
    rdfs:domain cim:ElectronicAddress ;
    rdfs:range xsd:string .

cim:ElectronicAddress.email1 a rdf:Property ;
    rdfs:label "email1" ;
    rdfs:comment "Primary email address." ;
    rdfs:domain cim:ElectronicAddress ;
    rdfs:range xsd:string .

cim:ElectronicAddress.isPrimary a rdf:Property ;
    rdfs:label "isPrimary" ;
    rdfs:comment "[ZBEX] Whether this email is the primary email address." ;
    rdfs:domain cim:ElectronicAddress ;
    rdfs:range xsd:boolean .

cim:EndDevice.Customer a rdf:Property ;
    rdfs:label "EndDevice.Customer" ;
    rdfs:comment "Customer owning this end device." ;
    rdfs:domain cim:EndDevice ;
    rdfs:range cim:Customer ;
    profile:targetCardinality "0..1" .

cim:EndDevice.EndDeviceFunction a rdf:Property ;
    rdfs:label "EndDevice.EndDeviceFunction" ;
    rdfs:comment "All end device functions this end device performs." ;
    rdfs:domain cim:EndDevice ;
    rdfs:range cim:EndDeviceFunction ;
    profile:targetCardinality "0..*" .

cim:EndDevice.Location a rdf:Property ;
    rdfs:label "EndDevice.Location" ;
    rdfs:comment "Service location whose service delivery is measured by this end device." ;
    rdfs:domain cim:EndDevice ;
    rdfs:range cim:Location ;
    profile:targetCardinality "All end devices that measure the service delivered to this service location." .

cim:EndDevice.UsagePoint a rdf:Property ;
    rdfs:label "EndDevice.UsagePoint" ;
    rdfs:comment "All end devices at this usage point. Usage point to which this end device belongs." ;
    rdfs:domain cim:EndDevice ;
    rdfs:range cim:UsagePoint ;
    profile:sourceCardinality "0..*" ;
    profile:targetCardinality "0..*" .

cim:EndDeviceFunction.enabled a rdf:Property ;
    rdfs:label "enabled" ;
    rdfs:comment "True if the function is enabled." ;
    rdfs:domain cim:EndDeviceFunction ;
    rdfs:range xsd:boolean .

cim:EndDeviceFunctionKind.UNKNOWN a rdf:Property ;
    rdfs:label "UNKNOWN" ;
    rdfs:comment "Unknown function kind." ;
    rdfs:domain cim:EndDeviceFunctionKind ;
    rdfs:range xsd:string .

cim:EndDeviceFunctionKind.autonomousDst a rdf:Property ;
    rdfs:label "autonomousDst" ;
    rdfs:comment "Autonomous application of daylight saving time (DST)." ;
    rdfs:domain cim:EndDeviceFunctionKind ;
    rdfs:range xsd:string .

cim:EndDeviceFunctionKind.demandResponse a rdf:Property ;
    rdfs:label "demandResponse" ;
    rdfs:comment "Demand response functions." ;
    rdfs:domain cim:EndDeviceFunctionKind ;
    rdfs:range xsd:string .

cim:EndDeviceFunctionKind.electricMetering a rdf:Property ;
    rdfs:label "electricMetering" ;
    rdfs:comment "Electricity metering." ;
    rdfs:domain cim:EndDeviceFunctionKind ;
    rdfs:range xsd:string .

cim:EndDeviceFunctionKind.metrology a rdf:Property ;
    rdfs:label "metrology" ;
    rdfs:comment "Presentation of metered values to a user or another system (always a function of a meter, but might not be supported by a load control unit)." ;
    rdfs:domain cim:EndDeviceFunctionKind ;
    rdfs:range xsd:string .

cim:EndDeviceFunctionKind.onRequestRead a rdf:Property ;
    rdfs:label "onRequestRead" ;
    rdfs:comment "On-request reads." ;
    rdfs:domain cim:EndDeviceFunctionKind ;
    rdfs:range xsd:string .

cim:EndDeviceFunctionKind.outageHistory a rdf:Property ;
    rdfs:label "outageHistory" ;
    rdfs:comment "Reporting historical power interruption data." ;
    rdfs:domain cim:EndDeviceFunctionKind ;
    rdfs:range xsd:string .

cim:EndDeviceFunctionKind.relaysProgramming a rdf:Property ;
    rdfs:label "relaysProgramming" ;
    rdfs:comment "Support for one or more relays that may be programmable in the meter (and tied to TOU, time pulse, load control or other functions)." ;
    rdfs:domain cim:EndDeviceFunctionKind ;
    rdfs:range xsd:string .

cim:EndDeviceFunctionKind.reverseFlow a rdf:Property ;
    rdfs:label "reverseFlow" ;
    rdfs:comment "Detection and monitoring of reverse flow." ;
    rdfs:domain cim:EndDeviceFunctionKind ;
    rdfs:range xsd:string .

cim:EnergyConsumer.EnergyConsumerPhase a rdf:Property ;
    rdfs:label "EnergyConsumer.EnergyConsumerPhase" ;
    rdfs:comment "The energy consumer to which this phase belongs. The individual phase models for this energy consumer." ;
    rdfs:domain cim:EnergyConsumer ;
    rdfs:range cim:EnergyConsumerPhase ;
    profile:sourceCardinality "0..1" ;
    profile:targetCardinality "0..*" .

cim:EnergyConsumer.customerCount a rdf:Property ;
    rdfs:label "customerCount" ;
    rdfs:comment "Number of individual customers represented by this demand." ;
    rdfs:domain cim:EnergyConsumer ;
    rdfs:range xsd:int .

cim:EnergyConsumer.grounded a rdf:Property ;
    rdfs:label "grounded" ;
    rdfs:comment "Used for Yn and Zn connections. True if the neutral is solidly grounded." ;
    rdfs:domain cim:EnergyConsumer ;
    rdfs:range xsd:boolean .

cim:EnergyConsumer.p a rdf:Property ;
    rdfs:label "p" ;
    rdfs:comment "Active power of the load. Load sign convention is used, i.e. positive sign means flow out from a node.\nFor voltage dependent loads the value is at rated voltage.\nStarting value for a steady state solution." ;
    rdfs:domain cim:EnergyConsumer ;
    rdfs:range cim:ActivePower .

cim:EnergyConsumer.pfixed a rdf:Property ;
    rdfs:label "pfixed" ;
    rdfs:comment "Active power of the load that is a fixed quantity and does not vary as load group value varies. Load sign convention is used, i.e. positive sign means flow out from a node." ;
    rdfs:domain cim:EnergyConsumer ;
    rdfs:range cim:ActivePower .

cim:EnergyConsumer.phaseConnection a rdf:Property ;
    rdfs:label "phaseConnection" ;
    rdfs:comment "The type of phase connection, such as wye or delta." ;
    rdfs:domain cim:EnergyConsumer ;
    rdfs:range cim:PhaseShuntConnectionKind .

cim:EnergyConsumer.q a rdf:Property ;
    rdfs:label "q" ;
    rdfs:comment "Reactive power of the load. Load sign convention is used, i.e. positive sign means flow out from a node.\nFor voltage dependent loads the value is at rated voltage.\nStarting value for a steady state solution." ;
    rdfs:domain cim:EnergyConsumer ;
    rdfs:range cim:ReactivePower .

cim:EnergyConsumer.qfixed a rdf:Property ;
    rdfs:label "qfixed" ;
    rdfs:comment "Reactive power of the load that is a fixed quantity and does not vary as load group value varies. Load sign convention is used, i.e. positive sign means flow out from a node." ;
    rdfs:domain cim:EnergyConsumer ;
    rdfs:range cim:ReactivePower .

cim:EnergyConsumerPhase.EnergyConsumer a rdf:Property ;
    rdfs:label "EnergyConsumerPhase.EnergyConsumer" ;
    rdfs:comment "The individual phase models for this energy consumer. The energy consumer to which this phase belongs." ;
    rdfs:domain cim:EnergyConsumerPhase ;
    rdfs:range cim:EnergyConsumer ;
    profile:sourceCardinality "0..*" ;
    profile:targetCardinality "0..1" .

cim:EnergyConsumerPhase.p a rdf:Property ;
    rdfs:label "p" ;
    rdfs:comment "Active power of the load. Load sign convention is used, i.e. positive sign means flow out from a node.\nFor voltage dependent loads the value is at rated voltage.\nStarting value for a steady state solution." ;
    rdfs:domain cim:EnergyConsumerPhase ;
    rdfs:range cim:ActivePower .

cim:EnergyConsumerPhase.pfixed a rdf:Property ;
    rdfs:label "pfixed" ;
    rdfs:comment "Active power of the load that is a fixed quantity. Load sign convention is used, i.e. positive sign means flow out from a node." ;
    rdfs:domain cim:EnergyConsumerPhase ;
    rdfs:range cim:ActivePower .

cim:EnergyConsumerPhase.phase a rdf:Property ;
    rdfs:label "phase" ;
    rdfs:comment "Phase of this energy consumer component.   If the energy consumer is wye connected, the connection is from the indicated phase to the central ground or neutral point.  If the energy consumer is delta connected, the phase indicates an energy consumer connected from the indicated phase to the next logical non-neutral phase." ;
    rdfs:domain cim:EnergyConsumerPhase ;
    rdfs:range cim:SinglePhaseKind .

cim:EnergyConsumerPhase.q a rdf:Property ;
    rdfs:label "q" ;
    rdfs:comment "Reactive power of the load. Load sign convention is used, i.e. positive sign means flow out from a node.\nFor voltage dependent loads the value is at rated voltage.\nStarting value for a steady state solution." ;
    rdfs:domain cim:EnergyConsumerPhase ;
    rdfs:range cim:ReactivePower .

cim:EnergyConsumerPhase.qfixed a rdf:Property ;
    rdfs:label "qfixed" ;
    rdfs:comment "Reactive power of the load that is a fixed quantity. Load sign convention is used, i.e. positive sign means flow out from a node." ;
    rdfs:domain cim:EnergyConsumerPhase ;
    rdfs:range cim:ReactivePower .

cim:EnergySource.EnergySourcePhase a rdf:Property ;
    rdfs:label "EnergySource.EnergySourcePhase" ;
    rdfs:comment "The energy sourceto which the phase belongs. The individual phase information of the energy source." ;
    rdfs:domain cim:EnergySource ;
    rdfs:range cim:EnergySourcePhase ;
    profile:sourceCardinality "0..1" ;
    profile:targetCardinality "0..*" .

cim:EnergySource.activePower a rdf:Property ;
    rdfs:label "activePower" ;
    rdfs:comment "High voltage source active injection. Load sign convention is used, i.e. positive sign means flow out from a node.\nStarting value for steady state solutions." ;
    rdfs:domain cim:EnergySource ;
    rdfs:range cim:ActivePower .

cim:EnergySource.isExternalGrid a rdf:Property ;
    rdfs:label "isExternalGrid" ;
    rdfs:comment "True if this energy source represents the higher-level power grid connection to an external grid that normally is modelled as the slack bus for power flow calculations." ;
    rdfs:domain cim:EnergySource ;
    rdfs:range xsd:boolean .

cim:EnergySource.pMax a rdf:Property ;
    rdfs:label "pMax" ;
    rdfs:comment "This is the maximum active power that can be produced by the source. Load sign convention is used, i.e. positive sign means flow out from a TopologicalNode (bus) into the conducting equipment." ;
    rdfs:domain cim:EnergySource ;
    rdfs:range cim:ActivePower .

cim:EnergySource.pMin a rdf:Property ;
    rdfs:label "pMin" ;
    rdfs:comment "This is the minimum active power that can be produced by the source. Load sign convention is used, i.e. positive sign means flow out from a TopologicalNode (bus) into the conducting equipment." ;
    rdfs:domain cim:EnergySource ;
    rdfs:range cim:ActivePower .

cim:EnergySource.r a rdf:Property ;
    rdfs:label "r" ;
    rdfs:comment "Positive sequence Thevenin resistance." ;
    rdfs:domain cim:EnergySource ;
    rdfs:range cim:Resistance .

cim:EnergySource.r0 a rdf:Property ;
    rdfs:label "r0" ;
    rdfs:comment "Zero sequence Thevenin resistance." ;
    rdfs:domain cim:EnergySource ;
    rdfs:range cim:Resistance .

cim:EnergySource.r0_max a rdf:Property ;
    rdfs:label "r0_max" ;
    rdfs:comment "Maximum zero sequence Thevenin resistance." ;
    rdfs:domain cim:EnergySource ;
    rdfs:range cim:Resistance .

cim:EnergySource.r0_min a rdf:Property ;
    rdfs:label "r0_min" ;
    rdfs:comment "Minimum zero sequence Thevenin resistance." ;
    rdfs:domain cim:EnergySource ;
    rdfs:range cim:Resistance .

cim:EnergySource.r_max a rdf:Property ;
    rdfs:label "r_max" ;
    rdfs:comment "Maximum positive sequence Thevenin resistance." ;
    rdfs:domain cim:EnergySource ;
    rdfs:range cim:Resistance .

cim:EnergySource.r_min a rdf:Property ;
    rdfs:label "r_min" ;
    rdfs:comment "Minimum positive sequence Thevenin resistance." ;
    rdfs:domain cim:EnergySource ;
    rdfs:range cim:Resistance .

cim:EnergySource.reactivePower a rdf:Property ;
    rdfs:label "reactivePower" ;
    rdfs:comment "High voltage source reactive injection. Load sign convention is used, i.e. positive sign means flow out from a node.\nStarting value for steady state solutions." ;
    rdfs:domain cim:EnergySource ;
    rdfs:range cim:ReactivePower .

cim:EnergySource.rn a rdf:Property ;
    rdfs:label "rn" ;
    rdfs:comment "Negative sequence Thevenin resistance." ;
    rdfs:domain cim:EnergySource ;
    rdfs:range cim:Resistance .

cim:EnergySource.rn_max a rdf:Property ;
    rdfs:label "rn_max" ;
    rdfs:comment "Maximum negative sequence Thevenin resistance." ;
    rdfs:domain cim:EnergySource ;
    rdfs:range cim:Resistance .

cim:EnergySource.rn_min a rdf:Property ;
    rdfs:label "rn_min" ;
    rdfs:comment "Minimum negative sequence Thevenin resistance" ;
    rdfs:domain cim:EnergySource ;
    rdfs:range cim:Resistance .

cim:EnergySource.voltageAngle a rdf:Property ;
    rdfs:label "voltageAngle" ;
    rdfs:comment "Phase angle of a-phase open circuit used when voltage characteristics need to be imposed at the node associated with the terminal of the energy source, such as when voltages and angles from the transmission level are used as input to the distribution network. The attribute shall be a positive value or zero." ;
    rdfs:domain cim:EnergySource ;
    rdfs:range cim:AngleRadians .

cim:EnergySource.voltageMagnitude a rdf:Property ;
    rdfs:label "voltageMagnitude" ;
    rdfs:comment "Phase-to-phase open circuit voltage magnitude used when voltage characteristics need to be imposed at the node associated with the terminal of the energy source, such as when voltages and angles from the transmission level are used as input to the distribution network. The attribute shall be a positive value or zero." ;
    rdfs:domain cim:EnergySource ;
    rdfs:range cim:Voltage .

cim:EnergySource.x a rdf:Property ;
    rdfs:label "x" ;
    rdfs:comment "Positive sequence Thevenin reactance." ;
    rdfs:domain cim:EnergySource ;
    rdfs:range cim:Reactance .

cim:EnergySource.x0 a rdf:Property ;
    rdfs:label "x0" ;
    rdfs:comment "Zero sequence Thevenin reactance." ;
    rdfs:domain cim:EnergySource ;
    rdfs:range cim:Reactance .

cim:EnergySource.x0_max a rdf:Property ;
    rdfs:label "x0_max" ;
    rdfs:comment "Maximum zero sequence Thevenin reactance." ;
    rdfs:domain cim:EnergySource ;
    rdfs:range cim:Reactance .

cim:EnergySource.x0_min a rdf:Property ;
    rdfs:label "x0_min" ;
    rdfs:comment "Minimum zero sequence Thevenin reactance." ;
    rdfs:domain cim:EnergySource ;
    rdfs:range cim:Reactance .

cim:EnergySource.x_max a rdf:Property ;
    rdfs:label "x_max" ;
    rdfs:comment "Maximum positive sequence Thevenin reactance." ;
    rdfs:domain cim:EnergySource ;
    rdfs:range cim:Reactance .

cim:EnergySource.x_min a rdf:Property ;
    rdfs:label "x_min" ;
    rdfs:comment "Minimum positive sequence Thevenin reactance." ;
    rdfs:domain cim:EnergySource ;
    rdfs:range cim:Reactance .

cim:EnergySource.xn a rdf:Property ;
    rdfs:label "xn" ;
    rdfs:comment "Negative sequence Thevenin reactance." ;
    rdfs:domain cim:EnergySource ;
    rdfs:range cim:Reactance .

cim:EnergySource.xn_max a rdf:Property ;
    rdfs:label "xn_max" ;
    rdfs:comment "Maximum negative sequence Thevenin reactance." ;
    rdfs:domain cim:EnergySource ;
    rdfs:range cim:Reactance .

cim:EnergySource.xn_min a rdf:Property ;
    rdfs:label "xn_min" ;
    rdfs:comment "Minimum negative sequence Thevenin reactance." ;
    rdfs:domain cim:EnergySource ;
    rdfs:range cim:Reactance .

cim:EnergySourcePhase.EnergySource a rdf:Property ;
    rdfs:label "EnergySourcePhase.EnergySource" ;
    rdfs:comment "The individual phase information of the energy source. The energy sourceto which the phase belongs." ;
    rdfs:domain cim:EnergySourcePhase ;
    rdfs:range cim:EnergySource ;
    profile:sourceCardinality "0..*" ;
    profile:targetCardinality "0..1" .

cim:EnergySourcePhase.phase a rdf:Property ;
    rdfs:label "phase" ;
    rdfs:comment "Phase of this energy source component.   If the energy source wye connected, the connection is from the indicated phase to the central ground or neutral point.  If the energy source is delta connected, the phase indicates an energy source connected from the indicated phase to the next logical non-neutral phase." ;
    rdfs:domain cim:EnergySourcePhase ;
    rdfs:range cim:SinglePhaseKind .

cim:Equipment.EquipmentContainer a rdf:Property ;
    rdfs:label "Equipment.EquipmentContainer" ;
    rdfs:comment "Contained equipment. Container of this equipment." ;
    rdfs:domain cim:Equipment ;
    rdfs:range cim:EquipmentContainer ;
    profile:sourceCardinality "0..*" ;
    profile:targetCardinality "0..1" .

cim:Equipment.EquipmentContainer a rdf:Property ;
    rdfs:label "Equipment.EquipmentContainer" ;
    rdfs:comment "Contained equipment. Container of this equipment if the equipment belongs to the current network state" ;
    rdfs:domain cim:Equipment ;
    rdfs:range cim:EquipmentContainer ;
    profile:sourceCardinality "0..*" ;
    profile:targetCardinality "0..1" .

cim:Equipment.OperationalRestriction a rdf:Property ;
    rdfs:label "Equipment.OperationalRestriction" ;
    rdfs:comment "All equipments to which this restriction applies. All operational restrictions for this equipment." ;
    rdfs:domain cim:Equipment ;
    rdfs:range cim:OperationalRestriction ;
    profile:sourceCardinality "0..*" ;
    profile:targetCardinality "0..*" .

cim:Equipment.UsagePoint a rdf:Property ;
    rdfs:label "Equipment.UsagePoint" ;
    rdfs:comment "All equipment connecting this usage point to the electrical grid. All usage points connected to the electrical grid through this equipment." ;
    rdfs:domain cim:Equipment ;
    rdfs:range cim:UsagePoint ;
    profile:sourceCardinality "0..*" ;
    profile:targetCardinality "0..*" .

cim:Equipment.commissionedDate a rdf:Property ;
    rdfs:label "commissionedDate" ;
    rdfs:comment "The date this equipment was commissioned into service." ;
    rdfs:domain cim:Equipment ;
    rdfs:range cim:Datetime .

cim:Equipment.inService a rdf:Property ;
    rdfs:label "inService" ;
    rdfs:comment "Specifies the availability of the equipment. True means the equipment is available for topology processing, which determines if the equipment is energized or not. False means that the equipment is treated by network applications as if it is not in the model." ;
    rdfs:domain cim:Equipment ;
    rdfs:range xsd:boolean .

cim:Equipment.normallyInService a rdf:Property ;
    rdfs:label "normallyInService" ;
    rdfs:comment "" ;
    rdfs:domain cim:Equipment ;
    rdfs:range xsd:boolean .

cim:EquipmentContainer.Equipment a rdf:Property ;
    rdfs:label "EquipmentContainer.Equipment" ;
    rdfs:comment "Container of this equipment. Contained equipment." ;
    rdfs:domain cim:EquipmentContainer ;
    rdfs:range cim:Equipment ;
    profile:sourceCardinality "0..1" ;
    profile:targetCardinality "0..*" .

cim:EquipmentContainer.Equipment a rdf:Property ;
    rdfs:label "EquipmentContainer.Equipment" ;
    rdfs:comment "Container of this equipment. Contained equipment relative to the current state of the network." ;
    rdfs:domain cim:EquipmentContainer ;
    rdfs:range cim:Equipment ;
    profile:sourceCardinality "0..1" ;
    profile:targetCardinality "0..*" .

cim:EquivalentBranch.negativeR12 a rdf:Property ;
    rdfs:label "negativeR12" ;
    rdfs:comment "Negative sequence series resistance from terminal sequence  1 to terminal sequence 2. Used for short circuit data exchange according to IEC 60909.\nEquivalentBranch is a result of network reduction prior to the data exchange." ;
    rdfs:domain cim:EquivalentBranch ;
    rdfs:range cim:Resistance .

cim:EquivalentBranch.negativeR21 a rdf:Property ;
    rdfs:label "negativeR21" ;
    rdfs:comment "Negative sequence series resistance from terminal sequence 2 to terminal sequence 1. Used for short circuit data exchange according to IEC 60909.\nEquivalentBranch is a result of network reduction prior to the data exchange." ;
    rdfs:domain cim:EquivalentBranch ;
    rdfs:range cim:Resistance .

cim:EquivalentBranch.negativeX12 a rdf:Property ;
    rdfs:label "negativeX12" ;
    rdfs:comment "Negative sequence series reactance from terminal sequence  1 to terminal sequence 2. Used for short circuit data exchange according to IEC 60909.\nUsage : EquivalentBranch is a result of network reduction prior to the data exchange." ;
    rdfs:domain cim:EquivalentBranch ;
    rdfs:range cim:Reactance .

cim:EquivalentBranch.negativeX21 a rdf:Property ;
    rdfs:label "negativeX21" ;
    rdfs:comment "Negative sequence series reactance from terminal sequence 2 to terminal sequence 1. Used for short circuit data exchange according to IEC 60909.\nUsage: EquivalentBranch is a result of network reduction prior to the data exchange." ;
    rdfs:domain cim:EquivalentBranch ;
    rdfs:range cim:Reactance .

cim:EquivalentBranch.positiveR12 a rdf:Property ;
    rdfs:label "positiveR12" ;
    rdfs:comment "Positive sequence series resistance from terminal sequence  1 to terminal sequence 2 . Used for short circuit data exchange according to IEC 60909. \nEquivalentBranch is a result of network reduction prior to the data exchange." ;
    rdfs:domain cim:EquivalentBranch ;
    rdfs:range cim:Resistance .

cim:EquivalentBranch.positiveR21 a rdf:Property ;
    rdfs:label "positiveR21" ;
    rdfs:comment "Positive sequence series resistance from terminal sequence 2 to terminal sequence 1. Used for short circuit data exchange according to IEC 60909.\nEquivalentBranch is a result of network reduction prior to the data exchange." ;
    rdfs:domain cim:EquivalentBranch ;
    rdfs:range cim:Resistance .

cim:EquivalentBranch.positiveX12 a rdf:Property ;
    rdfs:label "positiveX12" ;
    rdfs:comment "Positive sequence series reactance from terminal sequence  1 to terminal sequence 2. Used for short circuit data exchange according to IEC 60909.\nUsage : EquivalentBranch is a result of network reduction prior to the data exchange." ;
    rdfs:domain cim:EquivalentBranch ;
    rdfs:range cim:Reactance .

cim:EquivalentBranch.positiveX21 a rdf:Property ;
    rdfs:label "positiveX21" ;
    rdfs:comment "Positive sequence series reactance from terminal sequence 2 to terminal sequence 1. Used for short circuit data exchange according to IEC 60909.\nUsage : EquivalentBranch is a result of network reduction prior to the data exchange." ;
    rdfs:domain cim:EquivalentBranch ;
    rdfs:range cim:Reactance .

cim:EquivalentBranch.r a rdf:Property ;
    rdfs:label "r" ;
    rdfs:comment "Positive sequence series resistance of the reduced branch." ;
    rdfs:domain cim:EquivalentBranch ;
    rdfs:range cim:Resistance .

cim:EquivalentBranch.r21 a rdf:Property ;
    rdfs:label "r21" ;
    rdfs:comment "Resistance from terminal sequence 2 to terminal sequence 1 .Used for steady state power flow. This attribute is optional and represent unbalanced network such as off-nominal phase shifter. If only EquivalentBranch.r is given, then EquivalentBranch.r21 is assumed equal to EquivalentBranch.r.\nUsage rule : EquivalentBranch is a result of network reduction prior to the data exchange." ;
    rdfs:domain cim:EquivalentBranch ;
    rdfs:range cim:Resistance .

cim:EquivalentBranch.x a rdf:Property ;
    rdfs:label "x" ;
    rdfs:comment "Positive sequence series reactance of the reduced branch." ;
    rdfs:domain cim:EquivalentBranch ;
    rdfs:range cim:Reactance .

cim:EquivalentBranch.x21 a rdf:Property ;
    rdfs:label "x21" ;
    rdfs:comment "Reactance from terminal sequence 2 to terminal sequence 1. Used for steady state power flow. This attribute is optional and represents an unbalanced network such as off-nominal phase shifter. If only EquivalentBranch.x is given, then EquivalentBranch.x21 is assumed equal to EquivalentBranch.x.\nUsage rule: EquivalentBranch is a result of network reduction prior to the data exchange." ;
    rdfs:domain cim:EquivalentBranch ;
    rdfs:range cim:Reactance .

cim:EquivalentBranch.zeroR12 a rdf:Property ;
    rdfs:label "zeroR12" ;
    rdfs:comment "Zero sequence series resistance from terminal sequence  1 to terminal sequence 2. Used for short circuit data exchange according to IEC 60909.\nEquivalentBranch is a result of network reduction prior to the data exchange." ;
    rdfs:domain cim:EquivalentBranch ;
    rdfs:range cim:Resistance .

cim:EquivalentBranch.zeroR21 a rdf:Property ;
    rdfs:label "zeroR21" ;
    rdfs:comment "Zero sequence series resistance from terminal sequence  2 to terminal sequence 1. Used for short circuit data exchange according to IEC 60909.\nUsage : EquivalentBranch is a result of network reduction prior to the data exchange." ;
    rdfs:domain cim:EquivalentBranch ;
    rdfs:range cim:Resistance .

cim:EquivalentBranch.zeroX12 a rdf:Property ;
    rdfs:label "zeroX12" ;
    rdfs:comment "Zero sequence series reactance from terminal sequence  1 to terminal sequence 2. Used for short circuit data exchange according to IEC 60909.\nUsage : EquivalentBranch is a result of network reduction prior to the data exchange." ;
    rdfs:domain cim:EquivalentBranch ;
    rdfs:range cim:Reactance .

cim:EquivalentBranch.zeroX21 a rdf:Property ;
    rdfs:label "zeroX21" ;
    rdfs:comment "Zero sequence series reactance from terminal sequence 2 to terminal sequence 1. Used for short circuit data exchange according to IEC 60909.\nUsage : EquivalentBranch is a result of network reduction prior to the data exchange." ;
    rdfs:domain cim:EquivalentBranch ;
    rdfs:range cim:Reactance .

cim:Feeder.LvFeeder a rdf:Property ;
    rdfs:label "Feeder.LvFeeder" ;
    rdfs:comment "The HV/MV feeders that energize the LV feeder. The LV feeders that are normally energized by this feeder." ;
    rdfs:domain cim:Feeder ;
    rdfs:range cim:LvFeeder ;
    profile:sourceCardinality "0..1" ;
    profile:targetCardinality "0..*" .

cim:Feeder.LvFeeder a rdf:Property ;
    rdfs:label "Feeder.LvFeeder" ;
    rdfs:comment "The HV/MV feeders that energize the LV feeder in the current state of the network. The LV feeders that are currently energized by this feeder." ;
    rdfs:domain cim:Feeder ;
    rdfs:range cim:LvFeeder ;
    profile:sourceCardinality "0..1" ;
    profile:targetCardinality "0..*" .

cim:Feeder.Substation a rdf:Property ;
    rdfs:label "Feeder.Substation" ;
    rdfs:comment "The feeders that potentially energize  the downstream substation.  Should be consistent with the associations that describe the naming hierarchy. The substations that are normally energized by the feeder." ;
    rdfs:domain cim:Feeder ;
    rdfs:range cim:Substation ;
    profile:sourceCardinality "0..*" ;
    profile:targetCardinality "0..*" .

cim:Feeder.Terminal a rdf:Property ;
    rdfs:label "Feeder.Terminal" ;
    rdfs:comment "The normal head terminal or terminals of the feeder." ;
    rdfs:domain cim:Feeder ;
    rdfs:range cim:Terminal ;
    profile:sourceCardinality "0..1" .

cim:Frequency.value a rdf:Property ;
    rdfs:label "value" ;
    rdfs:comment "" ;
    rdfs:domain cim:Frequency ;
    rdfs:range xsd:double .

cim:Fuse.ProtectionRelayFunction a rdf:Property ;
    rdfs:label "Fuse.ProtectionRelayFunction" ;
    rdfs:comment "The function implemented by this Fuse" ;
    rdfs:domain cim:Fuse ;
    rdfs:range cim:ProtectionRelayFunction ;
    profile:targetCardinality "0..1" .

cim:GeographicalRegion.SubGeographicalRegion a rdf:Property ;
    rdfs:label "GeographicalRegion.SubGeographicalRegion" ;
    rdfs:comment "The geographical region which this sub-geographical region is within. All sub-geographical regions within this geographical region." ;
    rdfs:domain cim:GeographicalRegion ;
    rdfs:range cim:SubGeographicalRegion ;
    profile:sourceCardinality "0..1" ;
    profile:targetCardinality "0..*" .

cim:GroundingImpedance.x a rdf:Property ;
    rdfs:label "x" ;
    rdfs:comment "Reactance of device." ;
    rdfs:domain cim:GroundingImpedance ;
    rdfs:range cim:Reactance .

cim:IdentifiedObject.Name a rdf:Property ;
    rdfs:label "IdentifiedObject.Name" ;
    rdfs:comment "All names of this identified object." ;
    rdfs:domain cim:IdentifiedObject ;
    rdfs:range cim:Name ;
    profile:targetCardinality "0..*" .

cim:IdentifiedObject.description a rdf:Property ;
    rdfs:label "description" ;
    rdfs:comment "The description is a free human readable text describing or naming the object. It may be non unique and may not correlate to a naming hierarchy." ;
    rdfs:domain cim:IdentifiedObject ;
    rdfs:range xsd:string .

cim:IdentifiedObject.mRID a rdf:Property ;
    rdfs:label "mRID" ;
    rdfs:comment "Master resource identifier issued by a model authority. The mRID is unique within an exchange context. Global uniqueness is easily achieved by using a UUID, as specified in RFC 4122, for the mRID. The use of UUID is strongly recommended.\nFor CIMXML data files in RDF syntax conforming to IEC 61970-552, the mRID is mapped to rdf:ID or rdf:about attributes that identify CIM object elements." ;
    rdfs:domain cim:IdentifiedObject ;
    rdfs:range xsd:string .

cim:IdentifiedObject.name a rdf:Property ;
    rdfs:label "name" ;
    rdfs:comment "The name is any free human readable and possibly non unique text naming the object." ;
    rdfs:domain cim:IdentifiedObject ;
    rdfs:range xsd:string .

cim:IdentifiedObject.numDiagramObjects a rdf:Property ;
    rdfs:label "numDiagramObjects" ;
    rdfs:comment "Count of the DiagramObject's that are associated with this IdentifiedObject" ;
    rdfs:domain cim:IdentifiedObject ;
    rdfs:range xsd:int .

cim:Impedance.value a rdf:Property ;
    rdfs:label "value" ;
    rdfs:comment "ohms (ohm)" ;
    rdfs:domain cim:Impedance ;
    rdfs:range xsd:double .

cim:Length.value a rdf:Property ;
    rdfs:label "value" ;
    rdfs:comment "metres (m)" ;
    rdfs:domain cim:Length ;
    rdfs:range xsd:double .

cim:LinearShuntCompensator.b0PerSection a rdf:Property ;
    rdfs:label "b0PerSection" ;
    rdfs:comment "Zero sequence shunt (charging) susceptance per section." ;
    rdfs:domain cim:LinearShuntCompensator ;
    rdfs:range cim:Susceptance .

cim:LinearShuntCompensator.bPerSection a rdf:Property ;
    rdfs:label "bPerSection" ;
    rdfs:comment "Positive sequence shunt (charging) susceptance per section." ;
    rdfs:domain cim:LinearShuntCompensator ;
    rdfs:range cim:Susceptance .

cim:LinearShuntCompensator.g0PerSection a rdf:Property ;
    rdfs:label "g0PerSection" ;
    rdfs:comment "Zero sequence shunt (charging) conductance per section." ;
    rdfs:domain cim:LinearShuntCompensator ;
    rdfs:range cim:Conductance .

cim:LinearShuntCompensator.gPerSection a rdf:Property ;
    rdfs:label "gPerSection" ;
    rdfs:comment "Positive sequence shunt (charging) conductance per section." ;
    rdfs:domain cim:LinearShuntCompensator ;
    rdfs:range cim:Conductance .

cim:Location.PositionPoint a rdf:Property ;
    rdfs:label "Location.PositionPoint" ;
    rdfs:comment "Sequence of position points describing this location, expressed in coordinate system 'Location.CoordinateSystem'." ;
    rdfs:domain cim:Location ;
    rdfs:range cim:PositionPoint ;
    profile:targetCardinality "0..*" .

cim:Location.mainAddress a rdf:Property ;
    rdfs:label "mainAddress" ;
    rdfs:comment "Main address of the location." ;
    rdfs:domain cim:Location ;
    rdfs:range cim:StreetAddress .

cim:Loop.Circuit a rdf:Property ;
    rdfs:label "Loop.Circuit" ;
    rdfs:comment "\\[ZBEX\\] The loop containing this circuit. \\[ZBEX\\] Sub-transmission circuits that form part of this loop." ;
    rdfs:domain cim:Loop ;
    rdfs:range cim:Circuit ;
    profile:sourceCardinality "0..1" ;
    profile:targetCardinality "0..*" .

cim:Loop.Substation a rdf:Property ;
    rdfs:label "Loop.Substation" ;
    rdfs:comment "\\[ZBEX\\] The loops that are energizing this substation. \\[ZBEX\\] Substations that are energized by this loop." ;
    rdfs:domain cim:Loop ;
    rdfs:range cim:Substation ;
    profile:sourceCardinality "0..*" ;
    profile:targetCardinality "0..*" .

cim:Loop.Substation a rdf:Property ;
    rdfs:label "Loop.Substation" ;
    rdfs:comment "\\[ZBEX\\] The substations that normally energize this loop." ;
    rdfs:domain cim:Loop ;
    rdfs:range cim:Substation ;
    profile:sourceCardinality "0..*" ;
    profile:targetCardinality "0..*" .

cim:LvFeeder.Equipment a rdf:Property ;
    rdfs:label "LvFeeder.Equipment" ;
    rdfs:comment "\\[ZBEX\\] The LV feeders that are normally energized by the feeder. \\[ZBEX\\] Contained equipment using the current state of the network." ;
    rdfs:domain cim:LvFeeder ;
    rdfs:range cim:Equipment ;
    profile:sourceCardinality "0..*" ;
    profile:targetCardinality "0..*" .

cim:LvFeeder.Feeder a rdf:Property ;
    rdfs:label "LvFeeder.Feeder" ;
    rdfs:comment "\\[ZBEX\\] The LV feeders that are normally energized by the feeder. \\[ZBEX\\] The HV/MV feeders that energize this LV feeder." ;
    rdfs:domain cim:LvFeeder ;
    rdfs:range cim:Feeder ;
    profile:sourceCardinality "0..*" ;
    profile:targetCardinality "0..*" .

cim:LvFeeder.Feeder a rdf:Property ;
    rdfs:label "LvFeeder.Feeder" ;
    rdfs:comment "\\[ZBEX\\] The LV feeders that are currently energized by the feeder. \\[ZBEX\\] The HV/MV feeders that energize this LV feeder in the current state of the network." ;
    rdfs:domain cim:LvFeeder ;
    rdfs:range cim:Feeder ;
    profile:sourceCardinality "0..*" ;
    profile:targetCardinality "0..*" .

cim:LvFeeder.Terminal a rdf:Property ;
    rdfs:label "LvFeeder.Terminal" ;
    rdfs:comment "\\[ZBEX\\] The normal head terminal of this LV feeder, typically the LV terminal of a distribution substation." ;
    rdfs:domain cim:LvFeeder ;
    rdfs:range cim:Terminal ;
    profile:targetCardinality "0..1" .

cim:Measurement.ACDCTerminal a rdf:Property ;
    rdfs:label "Measurement.ACDCTerminal" ;
    rdfs:comment "Measurements associated with this terminal defining  where the measurement is placed in the network topology.  It may be used, for instance, to capture the sensor position, such as a voltage transformer (PT) at a busbar or a current transformer (CT) at the bar between a breaker and an isolator. One or more measurements may be associated with a terminal in the network." ;
    rdfs:domain cim:Measurement ;
    rdfs:range cim:ACDCTerminal ;
    profile:sourceCardinality "0..*" ;
    profile:targetCardinality "0..1" .

cim:Measurement.PowerSystemResource a rdf:Property ;
    rdfs:label "Measurement.PowerSystemResource" ;
    rdfs:comment "The measurements associated with this power system resource. The power system resource that contains the measurement." ;
    rdfs:domain cim:Measurement ;
    rdfs:range cim:PowerSystemResource ;
    profile:sourceCardinality "0..*" ;
    profile:targetCardinality "0..1" .

cim:Measurement.RemoteSource a rdf:Property ;
    rdfs:label "Measurement.RemoteSource" ;
    rdfs:comment "The measurements associated with this remote source The remote point taking the measurement." ;
    rdfs:domain cim:Measurement ;
    rdfs:range cim:RemoteSource ;
    profile:sourceCardinality "0..1" ;
    profile:targetCardinality "0..1" .

cim:Measurement.phases a rdf:Property ;
    rdfs:label "phases" ;
    rdfs:comment "Indicates to which phases the measurement applies and avoids the need to use 'measurementType' to also encode phase information (which would explode the types). The phase information in Measurement, along with 'measurementType' and 'phases' uniquely defines a Measurement for a device, based on normal network phase. Their meaning will not change when the computed energizing phasing is changed due to jumpers or other reasons.\nIf the attribute is missing three phases (ABC) shall be assumed." ;
    rdfs:domain cim:Measurement ;
    rdfs:range cim:PhaseCode .

cim:Measurement.unitSymbol a rdf:Property ;
    rdfs:label "unitSymbol" ;
    rdfs:comment "The unit of measure of the measured quantity." ;
    rdfs:domain cim:Measurement ;
    rdfs:range cim:UnitSymbol .

cim:MeasurementValue.timeStamp a rdf:Property ;
    rdfs:label "timeStamp" ;
    rdfs:comment "The time when the value was last updated." ;
    rdfs:domain cim:MeasurementValue ;
    rdfs:range cim:DateTime .

cim:Meter.companyMeterId a rdf:Property ;
    rdfs:label "companyMeterId" ;
    rdfs:comment "" ;
    rdfs:domain cim:Meter ;
    rdfs:range xsd:string .

cim:Name.IdentifiedObject a rdf:Property ;
    rdfs:label "Name.IdentifiedObject" ;
    rdfs:comment "All names of this identified object. Identified object that this name designates." ;
    rdfs:domain cim:Name ;
    rdfs:range cim:IdentifiedObject ;
    profile:sourceCardinality "0..*" ;
    profile:targetCardinality "0..1" .

cim:Name.name a rdf:Property ;
    rdfs:label "name" ;
    rdfs:comment "Any free text that name the object." ;
    rdfs:domain cim:Name ;
    rdfs:range xsd:string .

cim:Name.type a rdf:Property ;
    rdfs:label "type" ;
    rdfs:comment "Type of this name." ;
    rdfs:domain cim:Name ;
    rdfs:range cim:NameType .

cim:NameType.Name a rdf:Property ;
    rdfs:label "NameType.Name" ;
    rdfs:comment "All names of this type." ;
    rdfs:domain cim:NameType ;
    rdfs:range cim:Name ;
    profile:targetCardinality "0..*" .

cim:NameType.description a rdf:Property ;
    rdfs:label "description" ;
    rdfs:comment "Description of the name type." ;
    rdfs:domain cim:NameType ;
    rdfs:range xsd:string .

cim:NameType.name a rdf:Property ;
    rdfs:label "name" ;
    rdfs:comment "Name of the name type." ;
    rdfs:domain cim:NameType ;
    rdfs:range xsd:string .

cim:NoLoadTest.energisedEndVoltage a rdf:Property ;
    rdfs:label "energisedEndVoltage" ;
    rdfs:comment "Voltage applied to the winding (end) during test." ;
    rdfs:domain cim:NoLoadTest ;
    rdfs:range cim:Voltage .

cim:NoLoadTest.excitingCurrent a rdf:Property ;
    rdfs:label "excitingCurrent" ;
    rdfs:comment "Exciting current measured from a positive-sequence or single-phase excitation test." ;
    rdfs:domain cim:NoLoadTest ;
    rdfs:range cim:PerCent .

cim:NoLoadTest.excitingCurrentZero a rdf:Property ;
    rdfs:label "excitingCurrentZero" ;
    rdfs:comment "Exciting current measured from a zero-sequence open-circuit excitation test." ;
    rdfs:domain cim:NoLoadTest ;
    rdfs:range cim:PerCent .

cim:NoLoadTest.loss a rdf:Property ;
    rdfs:label "loss" ;
    rdfs:comment "Losses measured from a positive-sequence or single-phase excitation test." ;
    rdfs:domain cim:NoLoadTest ;
    rdfs:range cim:ActivePower .

cim:NoLoadTest.lossZero a rdf:Property ;
    rdfs:label "lossZero" ;
    rdfs:comment "Losses measured from a zero-sequence excitation test." ;
    rdfs:domain cim:NoLoadTest ;
    rdfs:range cim:ActivePower .

cim:OpenCircuitTest.energisedEndStep a rdf:Property ;
    rdfs:label "energisedEndStep" ;
    rdfs:comment "Tap step number for the energised end of the test pair." ;
    rdfs:domain cim:OpenCircuitTest ;
    rdfs:range xsd:int .

cim:OpenCircuitTest.energisedEndVoltage a rdf:Property ;
    rdfs:label "energisedEndVoltage" ;
    rdfs:comment "Voltage applied to the winding (end) during test." ;
    rdfs:domain cim:OpenCircuitTest ;
    rdfs:range cim:Voltage .

cim:OpenCircuitTest.openEndStep a rdf:Property ;
    rdfs:label "openEndStep" ;
    rdfs:comment "Tap step number for the open end of the test pair." ;
    rdfs:domain cim:OpenCircuitTest ;
    rdfs:range xsd:int .

cim:OpenCircuitTest.openEndVoltage a rdf:Property ;
    rdfs:label "openEndVoltage" ;
    rdfs:comment "Voltage measured at the open-circuited end, with the energised end set to rated voltage and all other ends open." ;
    rdfs:domain cim:OpenCircuitTest ;
    rdfs:range cim:Voltage .

cim:OpenCircuitTest.phaseShift a rdf:Property ;
    rdfs:label "phaseShift" ;
    rdfs:comment "Phase shift measured at the open end with the energised end set to rated voltage and all other ends open." ;
    rdfs:domain cim:OpenCircuitTest ;
    rdfs:range cim:AngleDegrees .

cim:OperationalRestriction.Equipment a rdf:Property ;
    rdfs:label "OperationalRestriction.Equipment" ;
    rdfs:comment "All operational restrictions for this equipment. All equipments to which this restriction applies." ;
    rdfs:domain cim:OperationalRestriction ;
    rdfs:range cim:Equipment ;
    profile:sourceCardinality "0..*" ;
    profile:targetCardinality "0..*" .

cim:OrganisationRole.Organisation a rdf:Property ;
    rdfs:label "OrganisationRole.Organisation" ;
    rdfs:comment "Organisation having this role." ;
    rdfs:domain cim:OrganisationRole ;
    rdfs:range cim:Organisation ;
    profile:targetCardinality "0..1" .

cim:OrientationKind.NEGATIVE a rdf:Property ;
    rdfs:label "NEGATIVE" ;
    rdfs:comment "For 2D diagrams, a negative orientation gives the left-hand orientation (favoured by computer graphics displays) with X values increasing from left to right and Y values increasing from top to bottom.   This is also known as a left hand orientation." ;
    rdfs:domain cim:OrientationKind ;
    rdfs:range xsd:string .

cim:OrientationKind.POSITIVE a rdf:Property ;
    rdfs:label "POSITIVE" ;
    rdfs:comment "For 2D diagrams, a positive orientation will result in X values increasing from left to right and Y values increasing from bottom to top.  This is also known as a right hand orientation." ;
    rdfs:domain cim:OrientationKind ;
    rdfs:range xsd:string .

cim:PanDemandResponseFunction.appliance a rdf:Property ;
    rdfs:label "appliance" ;
    rdfs:comment "\\[ZBEX\\] Appliance being controlled." ;
    rdfs:domain cim:PanDemandResponseFunction ;
    rdfs:range cim:ControlledAppliance .

cim:PanDemandResponseFunction.kind a rdf:Property ;
    rdfs:label "kind" ;
    rdfs:comment "\\[ZBEX\\] Kind of this function." ;
    rdfs:domain cim:PanDemandResponseFunction ;
    rdfs:range cim:EndDeviceFunctionKind .

cim:PerCent.value a rdf:Property ;
    rdfs:label "value" ;
    rdfs:comment "Normally 0 to 100 on a defined base." ;
    rdfs:domain cim:PerCent ;
    rdfs:range xsd:double .

cim:PerLengthPhaseImpedance.PhaseImpedanceData a rdf:Property ;
    rdfs:label "PerLengthPhaseImpedance.PhaseImpedanceData" ;
    rdfs:comment "Conductor phase impedance to which this data belongs. All data that belong to this conductor phase impedance." ;
    rdfs:domain cim:PerLengthPhaseImpedance ;
    rdfs:range cim:PhaseImpedanceData ;
    profile:sourceCardinality "0..1" ;
    profile:targetCardinality "0..*" .

cim:PerLengthSequenceImpedance.b0ch a rdf:Property ;
    rdfs:label "b0ch" ;
    rdfs:comment "Zero sequence shunt (charging) susceptance, per unit of length." ;
    rdfs:domain cim:PerLengthSequenceImpedance ;
    rdfs:range cim:SusceptancePerLength .

cim:PerLengthSequenceImpedance.bch a rdf:Property ;
    rdfs:label "bch" ;
    rdfs:comment "Positive sequence shunt (charging) susceptance, per unit of length." ;
    rdfs:domain cim:PerLengthSequenceImpedance ;
    rdfs:range cim:SusceptancePerLength .

cim:PerLengthSequenceImpedance.g0ch a rdf:Property ;
    rdfs:label "g0ch" ;
    rdfs:comment "Zero sequence shunt (charging) conductance, per unit of length." ;
    rdfs:domain cim:PerLengthSequenceImpedance ;
    rdfs:range cim:ConductancePerLength .

cim:PerLengthSequenceImpedance.gch a rdf:Property ;
    rdfs:label "gch" ;
    rdfs:comment "Positive sequence shunt (charging) conductance, per unit of length." ;
    rdfs:domain cim:PerLengthSequenceImpedance ;
    rdfs:range cim:ConductancePerLength .

cim:PerLengthSequenceImpedance.r a rdf:Property ;
    rdfs:label "r" ;
    rdfs:comment "Positive sequence series resistance, per unit of length." ;
    rdfs:domain cim:PerLengthSequenceImpedance ;
    rdfs:range cim:ResistancePerLength .

cim:PerLengthSequenceImpedance.r0 a rdf:Property ;
    rdfs:label "r0" ;
    rdfs:comment "Zero sequence series resistance, per unit of length." ;
    rdfs:domain cim:PerLengthSequenceImpedance ;
    rdfs:range cim:ResistancePerLength .

cim:PerLengthSequenceImpedance.x a rdf:Property ;
    rdfs:label "x" ;
    rdfs:comment "Positive sequence series reactance, per unit of length." ;
    rdfs:domain cim:PerLengthSequenceImpedance ;
    rdfs:range cim:ReactancePerLength .

cim:PerLengthSequenceImpedance.x0 a rdf:Property ;
    rdfs:label "x0" ;
    rdfs:comment "Zero sequence series reactance, per unit of length." ;
    rdfs:domain cim:PerLengthSequenceImpedance ;
    rdfs:range cim:ReactancePerLength .

cim:PetersenCoil.xGroundNominal a rdf:Property ;
    rdfs:label "xGroundNominal" ;
    rdfs:comment "The nominal reactance in ohms. This is the operating point (normally over compensation) that is defined based on the resonance point in the healthy network condition. The impedance is calculated based on nominal voltage divided by position current." ;
    rdfs:domain cim:PetersenCoil ;
    rdfs:range cim:Reactance .

cim:PhaseCode.A a rdf:Property ;
    rdfs:label "A" ;
    rdfs:comment "Phase A." ;
    rdfs:domain cim:PhaseCode ;
    rdfs:range xsd:string .

cim:PhaseCode.AB a rdf:Property ;
    rdfs:label "AB" ;
    rdfs:comment "Phases A and B." ;
    rdfs:domain cim:PhaseCode ;
    rdfs:range xsd:string .

cim:PhaseCode.ABC a rdf:Property ;
    rdfs:label "ABC" ;
    rdfs:comment "Phases A, B, and C." ;
    rdfs:domain cim:PhaseCode ;
    rdfs:range xsd:string .

cim:PhaseCode.ABCN a rdf:Property ;
    rdfs:label "ABCN" ;
    rdfs:comment "Phases A, B, C, and N." ;
    rdfs:domain cim:PhaseCode ;
    rdfs:range xsd:string .

cim:PhaseCode.ABN a rdf:Property ;
    rdfs:label "ABN" ;
    rdfs:comment "Phases A, B, and neutral." ;
    rdfs:domain cim:PhaseCode ;
    rdfs:range xsd:string .

cim:PhaseCode.AC a rdf:Property ;
    rdfs:label "AC" ;
    rdfs:comment "Phases A and C." ;
    rdfs:domain cim:PhaseCode ;
    rdfs:range xsd:string .

cim:PhaseCode.ACN a rdf:Property ;
    rdfs:label "ACN" ;
    rdfs:comment "Phases A, C and neutral." ;
    rdfs:domain cim:PhaseCode ;
    rdfs:range xsd:string .

cim:PhaseCode.AN a rdf:Property ;
    rdfs:label "AN" ;
    rdfs:comment "Phases A and neutral." ;
    rdfs:domain cim:PhaseCode ;
    rdfs:range xsd:string .

cim:PhaseCode.B a rdf:Property ;
    rdfs:label "B" ;
    rdfs:comment "Phase B." ;
    rdfs:domain cim:PhaseCode ;
    rdfs:range xsd:string .

cim:PhaseCode.BC a rdf:Property ;
    rdfs:label "BC" ;
    rdfs:comment "Phases B and C." ;
    rdfs:domain cim:PhaseCode ;
    rdfs:range xsd:string .

cim:PhaseCode.BCN a rdf:Property ;
    rdfs:label "BCN" ;
    rdfs:comment "Phases B, C, and neutral." ;
    rdfs:domain cim:PhaseCode ;
    rdfs:range xsd:string .

cim:PhaseCode.BN a rdf:Property ;
    rdfs:label "BN" ;
    rdfs:comment "Phases B and neutral." ;
    rdfs:domain cim:PhaseCode ;
    rdfs:range xsd:string .

cim:PhaseCode.C a rdf:Property ;
    rdfs:label "C" ;
    rdfs:comment "Phase C." ;
    rdfs:domain cim:PhaseCode ;
    rdfs:range xsd:string .

cim:PhaseCode.CN a rdf:Property ;
    rdfs:label "CN" ;
    rdfs:comment "Phases C and neutral." ;
    rdfs:domain cim:PhaseCode ;
    rdfs:range xsd:string .

cim:PhaseCode.N a rdf:Property ;
    rdfs:label "N" ;
    rdfs:comment "Neutral phase." ;
    rdfs:domain cim:PhaseCode ;
    rdfs:range xsd:string .

cim:PhaseCode.X a rdf:Property ;
    rdfs:label "X" ;
    rdfs:comment "Unknown non-neutral phase." ;
    rdfs:domain cim:PhaseCode ;
    rdfs:range xsd:string .

cim:PhaseCode.XN a rdf:Property ;
    rdfs:label "XN" ;
    rdfs:comment "Unknown non-neutral phase plus neutral." ;
    rdfs:domain cim:PhaseCode ;
    rdfs:range xsd:string .

cim:PhaseCode.XY a rdf:Property ;
    rdfs:label "XY" ;
    rdfs:comment "Two unknown non-neutral phases." ;
    rdfs:domain cim:PhaseCode ;
    rdfs:range xsd:string .

cim:PhaseCode.XYN a rdf:Property ;
    rdfs:label "XYN" ;
    rdfs:comment "Two unknown non-neutral phases plus neutral." ;
    rdfs:domain cim:PhaseCode ;
    rdfs:range xsd:string .

cim:PhaseCode.Y a rdf:Property ;
    rdfs:label "Y" ;
    rdfs:comment "/[ZBEX/] Unknown non-neutral phase." ;
    rdfs:domain cim:PhaseCode ;
    rdfs:range xsd:string .

cim:PhaseCode.YN a rdf:Property ;
    rdfs:label "YN" ;
    rdfs:comment "/[ZBEX/] Unknown non-neutral phase plus neutral." ;
    rdfs:domain cim:PhaseCode ;
    rdfs:range xsd:string .

cim:PhaseCode.none a rdf:Property ;
    rdfs:label "none" ;
    rdfs:comment "No phases specified." ;
    rdfs:domain cim:PhaseCode ;
    rdfs:range xsd:string .

cim:PhaseCode.s1 a rdf:Property ;
    rdfs:label "s1" ;
    rdfs:comment "Secondary phase 1." ;
    rdfs:domain cim:PhaseCode ;
    rdfs:range xsd:string .

cim:PhaseCode.s12 a rdf:Property ;
    rdfs:label "s12" ;
    rdfs:comment "Secondary phase 1 and 2." ;
    rdfs:domain cim:PhaseCode ;
    rdfs:range xsd:string .

cim:PhaseCode.s12N a rdf:Property ;
    rdfs:label "s12N" ;
    rdfs:comment "Secondary phases 1, 2, and neutral." ;
    rdfs:domain cim:PhaseCode ;
    rdfs:range xsd:string .

cim:PhaseCode.s1N a rdf:Property ;
    rdfs:label "s1N" ;
    rdfs:comment "Secondary phase 1 and neutral." ;
    rdfs:domain cim:PhaseCode ;
    rdfs:range xsd:string .

cim:PhaseCode.s2 a rdf:Property ;
    rdfs:label "s2" ;
    rdfs:comment "Secondary phase 2." ;
    rdfs:domain cim:PhaseCode ;
    rdfs:range xsd:string .

cim:PhaseCode.s2N a rdf:Property ;
    rdfs:label "s2N" ;
    rdfs:comment "Secondary phase 2 and neutral." ;
    rdfs:domain cim:PhaseCode ;
    rdfs:range xsd:string .

cim:PhaseImpedanceData.PerLengthPhaseImpedance a rdf:Property ;
    rdfs:label "PhaseImpedanceData.PerLengthPhaseImpedance" ;
    rdfs:comment "All data that belong to this conductor phase impedance. Conductor phase impedance to which this data belongs." ;
    rdfs:domain cim:PhaseImpedanceData ;
    rdfs:range cim:PerLengthPhaseImpedance ;
    profile:sourceCardinality "0..*" ;
    profile:targetCardinality "0..1" .

cim:PhaseImpedanceData.b a rdf:Property ;
    rdfs:label "b" ;
    rdfs:comment "Susceptance matrix element value, per length of unit." ;
    rdfs:domain cim:PhaseImpedanceData ;
    rdfs:range cim:SusceptancePerLength .

cim:PhaseImpedanceData.fromPhase a rdf:Property ;
    rdfs:label "fromPhase" ;
    rdfs:comment "Refer to the class description." ;
    rdfs:domain cim:PhaseImpedanceData ;
    rdfs:range cim:SinglePhaseKind .

cim:PhaseImpedanceData.g a rdf:Property ;
    rdfs:label "g" ;
    rdfs:comment "Conductance matrix element value, per length of unit." ;
    rdfs:domain cim:PhaseImpedanceData ;
    rdfs:range cim:ConductancePerLength .

cim:PhaseImpedanceData.r a rdf:Property ;
    rdfs:label "r" ;
    rdfs:comment "Resistance matrix element value, per length of unit." ;
    rdfs:domain cim:PhaseImpedanceData ;
    rdfs:range cim:ResistancePerLength .

cim:PhaseImpedanceData.toPhase a rdf:Property ;
    rdfs:label "toPhase" ;
    rdfs:comment "Refer to the class description." ;
    rdfs:domain cim:PhaseImpedanceData ;
    rdfs:range cim:SinglePhaseKind .

cim:PhaseImpedanceData.x a rdf:Property ;
    rdfs:label "x" ;
    rdfs:comment "Reactance matrix element value, per length of unit." ;
    rdfs:domain cim:PhaseImpedanceData ;
    rdfs:range cim:ReactancePerLength .

cim:PhaseShuntConnectionKind.D a rdf:Property ;
    rdfs:label "D" ;
    rdfs:comment "Delta connection." ;
    rdfs:domain cim:PhaseShuntConnectionKind ;
    rdfs:range xsd:string .

cim:PhaseShuntConnectionKind.G a rdf:Property ;
    rdfs:label "G" ;
    rdfs:comment "Ground connection; use when explicit connection to ground needs to be expressed in combination with the phase code, such as for electrical wire/cable or for meters." ;
    rdfs:domain cim:PhaseShuntConnectionKind ;
    rdfs:range xsd:string .

cim:PhaseShuntConnectionKind.I a rdf:Property ;
    rdfs:label "I" ;
    rdfs:comment "Independent winding, for single-phase connections." ;
    rdfs:domain cim:PhaseShuntConnectionKind ;
    rdfs:range xsd:string .

cim:PhaseShuntConnectionKind.UNKNOWN a rdf:Property ;
    rdfs:label "UNKNOWN" ;
    rdfs:comment "" ;
    rdfs:domain cim:PhaseShuntConnectionKind ;
    rdfs:range xsd:string .

cim:PhaseShuntConnectionKind.Y a rdf:Property ;
    rdfs:label "Y" ;
    rdfs:comment "Wye connection." ;
    rdfs:domain cim:PhaseShuntConnectionKind ;
    rdfs:range xsd:string .

cim:PhaseShuntConnectionKind.Yn a rdf:Property ;
    rdfs:label "Yn" ;
    rdfs:comment "Wye, with neutral brought out for grounding." ;
    rdfs:domain cim:PhaseShuntConnectionKind ;
    rdfs:range xsd:string .

cim:PolarizingQuantityType.NEGATIVE_SEQUENCE_VOLTAGE a rdf:Property ;
    rdfs:label "NEGATIVE_SEQUENCE_VOLTAGE" ;
    rdfs:comment "\\[ZBEX\\] Uses the negative sequence voltage (V2), derived from three phase voltages." ;
    rdfs:domain cim:PolarizingQuantityType ;
    rdfs:range xsd:string .

cim:PolarizingQuantityType.POSITIVE_SEQUENCE_VOLTAGE a rdf:Property ;
    rdfs:label "POSITIVE_SEQUENCE_VOLTAGE" ;
    rdfs:comment "\\[ZBEX\\] Uses the positive sequence voltage (V1), derived from three phase voltages." ;
    rdfs:domain cim:PolarizingQuantityType ;
    rdfs:range xsd:string .

cim:PolarizingQuantityType.QUADRATURE_VOLTAGE a rdf:Property ;
    rdfs:label "QUADRATURE_VOLTAGE" ;
    rdfs:comment "\\[ZBEX\\] Uses a quadrature voltage (e.g., Vbc for an Ia element, specific convention applies)." ;
    rdfs:domain cim:PolarizingQuantityType ;
    rdfs:range xsd:string .

cim:PolarizingQuantityType.SELF_PHASE_VOLTAGE a rdf:Property ;
    rdfs:label "SELF_PHASE_VOLTAGE" ;
    rdfs:comment "\\[ZBEX\\] Uses the voltage of the same phase as the current element (e.g., Va for an Ia element)." ;
    rdfs:domain cim:PolarizingQuantityType ;
    rdfs:range xsd:string .

cim:PolarizingQuantityType.UNKNOWN a rdf:Property ;
    rdfs:label "UNKNOWN" ;
    rdfs:comment "\\[ZBEX\\] Type is unknown." ;
    rdfs:domain cim:PolarizingQuantityType ;
    rdfs:range xsd:string .

cim:PolarizingQuantityType.ZERO_SEQUENCE_VOLTAGE a rdf:Property ;
    rdfs:label "ZERO_SEQUENCE_VOLTAGE" ;
    rdfs:comment "\\[ZBEX\\] Uses the zero sequence voltage (Vo), derived from three phase voltages." ;
    rdfs:domain cim:PolarizingQuantityType ;
    rdfs:range xsd:string .

cim:Pole.Streetlight a rdf:Property ;
    rdfs:label "Pole.Streetlight" ;
    rdfs:comment "Pole to which thiss streetlight is attached. All streetlights attached to this pole." ;
    rdfs:domain cim:Pole ;
    rdfs:range cim:Streetlight ;
    profile:sourceCardinality "0..1" ;
    profile:targetCardinality "0..*" .

cim:Pole.classification a rdf:Property ;
    rdfs:label "classification" ;
    rdfs:comment "Pole class: 1, 2, 3, 4, 5, 6, 7, H1, H2, Other, Unknown." ;
    rdfs:domain cim:Pole ;
    rdfs:range xsd:string .

cim:PositionPoint.Location a rdf:Property ;
    rdfs:label "PositionPoint.Location" ;
    rdfs:comment "Sequence of position points describing this location, expressed in coordinate system 'Location.CoordinateSystem'. Location described by this position point." ;
    rdfs:domain cim:PositionPoint ;
    rdfs:range cim:Location ;
    profile:sourceCardinality "0..*" ;
    profile:targetCardinality "1" .

cim:PositionPoint.sequenceNumber a rdf:Property ;
    rdfs:label "sequenceNumber" ;
    rdfs:comment "Order of the position point within the parent location geometry." ;
    rdfs:domain cim:PositionPoint ;
    rdfs:range xsd:int .

cim:PositionPoint.xPosition a rdf:Property ;
    rdfs:label "xPosition" ;
    rdfs:comment "X axis position." ;
    rdfs:domain cim:PositionPoint ;
    rdfs:range xsd:double .

cim:PositionPoint.yPosition a rdf:Property ;
    rdfs:label "yPosition" ;
    rdfs:comment "Y axis position." ;
    rdfs:domain cim:PositionPoint ;
    rdfs:range xsd:double .

cim:PotentialTransformer.type a rdf:Property ;
    rdfs:label "type" ;
    rdfs:comment "Potential transformer construction type." ;
    rdfs:domain cim:PotentialTransformer ;
    rdfs:range cim:PotentialTransformerKind .

cim:PotentialTransformerInfo.accuracyClass a rdf:Property ;
    rdfs:label "accuracyClass" ;
    rdfs:comment "" ;
    rdfs:domain cim:PotentialTransformerInfo ;
    rdfs:range xsd:string .

cim:PotentialTransformerInfo.nominalRatio a rdf:Property ;
    rdfs:label "nominalRatio" ;
    rdfs:comment "" ;
    rdfs:domain cim:PotentialTransformerInfo ;
    rdfs:range cim:Ratio .

cim:PotentialTransformerInfo.primaryRatio a rdf:Property ;
    rdfs:label "primaryRatio" ;
    rdfs:comment "Ratio for the primary winding tap changer (numerator)." ;
    rdfs:domain cim:PotentialTransformerInfo ;
    rdfs:range xsd:double .

cim:PotentialTransformerInfo.ptClass a rdf:Property ;
    rdfs:label "ptClass" ;
    rdfs:comment "" ;
    rdfs:domain cim:PotentialTransformerInfo ;
    rdfs:range xsd:string .

cim:PotentialTransformerInfo.ratedVoltage a rdf:Property ;
    rdfs:label "ratedVoltage" ;
    rdfs:comment "Rated voltage on the primary side." ;
    rdfs:domain cim:PotentialTransformerInfo ;
    rdfs:range cim:Voltage .

cim:PotentialTransformerInfo.secondaryRatio a rdf:Property ;
    rdfs:label "secondaryRatio" ;
    rdfs:comment "Ratio for the secondary winding tap changer (denominator)." ;
    rdfs:domain cim:PotentialTransformerInfo ;
    rdfs:range xsd:double .

cim:PotentialTransformerKind.UNKNOWN a rdf:Property ;
    rdfs:label "UNKNOWN" ;
    rdfs:comment "The construction type of the potential transformer is unknown." ;
    rdfs:domain cim:PotentialTransformerKind ;
    rdfs:range xsd:string .

cim:PotentialTransformerKind.capacitiveCoupling a rdf:Property ;
    rdfs:label "capacitiveCoupling" ;
    rdfs:comment "The potential transformer is using capacitive coupling to create secondary voltage." ;
    rdfs:domain cim:PotentialTransformerKind ;
    rdfs:range xsd:string .

cim:PotentialTransformerKind.inductive a rdf:Property ;
    rdfs:label "inductive" ;
    rdfs:comment "The potential transformer is using induction coils to create secondary voltage." ;
    rdfs:domain cim:PotentialTransformerKind ;
    rdfs:range xsd:string .

cim:PowerDirectionKind.FORWARD a rdf:Property ;
    rdfs:label "FORWARD" ;
    rdfs:comment "\\[ZBEX\\] Power direction forward flow is used." ;
    rdfs:domain cim:PowerDirectionKind ;
    rdfs:range xsd:string .

cim:PowerDirectionKind.REVERSE a rdf:Property ;
    rdfs:label "REVERSE" ;
    rdfs:comment "\\[ZBEX\\] Power direction reverse flow is used." ;
    rdfs:domain cim:PowerDirectionKind ;
    rdfs:range xsd:string .

cim:PowerDirectionKind.UNDIRECTED a rdf:Property ;
    rdfs:label "UNDIRECTED" ;
    rdfs:comment "\\[ZBEX\\] Power direction flow type is not specified." ;
    rdfs:domain cim:PowerDirectionKind ;
    rdfs:range xsd:string .

cim:PowerDirectionKind.UNKNOWN_DIRECTION a rdf:Property ;
    rdfs:label "UNKNOWN_DIRECTION" ;
    rdfs:comment "\\[ZBEX\\] Unknown power direction flow." ;
    rdfs:domain cim:PowerDirectionKind ;
    rdfs:range xsd:string .

cim:PowerElectronicsConnection.PowerElectronicsConnectionPhase a rdf:Property ;
    rdfs:label "PowerElectronicsConnection.PowerElectronicsConnectionPhase" ;
    rdfs:comment "Power electronics connection of this power electronics connection phase. The individual phases models for the power electronics connection." ;
    rdfs:domain cim:PowerElectronicsConnection ;
    rdfs:range cim:PowerElectronicsConnectionPhase ;
    profile:sourceCardinality "0..1" ;
    profile:targetCardinality "0..*" .

cim:PowerElectronicsConnection.PowerElectronicsUnit a rdf:Property ;
    rdfs:label "PowerElectronicsConnection.PowerElectronicsUnit" ;
    rdfs:comment "A power electronics unit has a connection to the AC network. An AC network connection may have several power electronics units connecting through it." ;
    rdfs:domain cim:PowerElectronicsConnection ;
    rdfs:range cim:PowerElectronicsUnit ;
    profile:sourceCardinality "0..1" ;
    profile:targetCardinality "0..*" .

cim:PowerElectronicsConnection.invFixReactivePower a rdf:Property ;
    rdfs:label "invFixReactivePower" ;
    rdfs:comment "\\[ZBEX\\] Static Reactive Power, specified in a percentage output of the system. Permitted range is between -1.0 and 1.0 (inclusive), with a negative sign referring to sink." ;
    rdfs:domain cim:PowerElectronicsConnection ;
    rdfs:range cim:PU .

cim:PowerElectronicsConnection.invReactivePowerMode a rdf:Property ;
    rdfs:label "invReactivePowerMode" ;
    rdfs:comment "\\[ZBEX\\] If true, enables Static Reactive Power mode on the inverter." ;
    rdfs:domain cim:PowerElectronicsConnection ;
    rdfs:range xsd:boolean .

cim:PowerElectronicsConnection.invVarRespQAtV1 a rdf:Property ;
    rdfs:label "invVarRespQAtV1" ;
    rdfs:comment "\\[ZBEX\\] Power output set point 1 as a percentage of rated output for inverter Volt-VAr response mode. Permitted range is between -0.6 and 0 (inclusive) with a negative number referring to a sink." ;
    rdfs:domain cim:PowerElectronicsConnection ;
    rdfs:range cim:PU .

cim:PowerElectronicsConnection.invVarRespQAtV2 a rdf:Property ;
    rdfs:label "invVarRespQAtV2" ;
    rdfs:comment "\\[ZBEX\\] Power output set point 2 as a percentage of rated output for inverter Volt-VAr response mode. Permitted range is between -0.6 and 0 (inclusive) with a negative number referring to a sink." ;
    rdfs:domain cim:PowerElectronicsConnection ;
    rdfs:range cim:PU .

cim:PowerElectronicsConnection.invVarRespQAtV3 a rdf:Property ;
    rdfs:label "invVarRespQAtV3" ;
    rdfs:comment "\\[ZBEX\\] Power output set point 3 as a percentage of rated output for inverter Volt-VAr response mode. Permitted range is between -0.6 and 0 (inclusive) with a negative number referring to a sink." ;
    rdfs:domain cim:PowerElectronicsConnection ;
    rdfs:range cim:PU .

cim:PowerElectronicsConnection.invVarRespQAtV4 a rdf:Property ;
    rdfs:label "invVarRespQAtV4" ;
    rdfs:comment "\\[ZBEX\\] Power output set point 4 as a percentage of rated output for inverter Volt-VAr response mode. Permitted range is between -0.6 and 0 (inclusive) with a negative number referring to a sink." ;
    rdfs:domain cim:PowerElectronicsConnection ;
    rdfs:range cim:PU .

cim:PowerElectronicsConnection.invVarRespV1 a rdf:Property ;
    rdfs:label "invVarRespV1" ;
    rdfs:comment "\\[ZBEX\\] Set point 1 in volts for inverter Volt-VAr response mode. Permitted range is between 200 and 300 (inclusive)." ;
    rdfs:domain cim:PowerElectronicsConnection ;
    rdfs:range cim:Voltage .

cim:PowerElectronicsConnection.invVarRespV2 a rdf:Property ;
    rdfs:label "invVarRespV2" ;
    rdfs:comment "\\[ZBEX\\] Set point 2 in volts for inverter Volt-VAr response mode. Permitted range is between 200 and 300 (inclusive)." ;
    rdfs:domain cim:PowerElectronicsConnection ;
    rdfs:range cim:Voltage .

cim:PowerElectronicsConnection.invVarRespV3 a rdf:Property ;
    rdfs:label "invVarRespV3" ;
    rdfs:comment "\\[ZBEX\\] Set point 3 in volts for inverter Volt-VAr response mode. Permitted range is between 200 and 300 (inclusive)." ;
    rdfs:domain cim:PowerElectronicsConnection ;
    rdfs:range cim:Voltage .

cim:PowerElectronicsConnection.invVarRespV4 a rdf:Property ;
    rdfs:label "invVarRespV4" ;
    rdfs:comment "\\[ZBEX\\] Set point 4 in volts for inverter Volt-VAr response mode. Permitted range is between 200 and 300 (inclusive)." ;
    rdfs:domain cim:PowerElectronicsConnection ;
    rdfs:range cim:Voltage .

cim:PowerElectronicsConnection.invVoltVarRespMode a rdf:Property ;
    rdfs:label "invVoltVarRespMode" ;
    rdfs:comment "\\[ZBEX\\] Volt-VAr response mode allows an inverter to consume (sink) or produce (source) reactive power depending on the measured voltage. This mode is further described in AS4777.2:2015, section 6.3.2.3. True implies the mode is enabled." ;
    rdfs:domain cim:PowerElectronicsConnection ;
    rdfs:range xsd:boolean .

cim:PowerElectronicsConnection.invVoltWattRespMode a rdf:Property ;
    rdfs:label "invVoltWattRespMode" ;
    rdfs:comment "\\[ZBEX\\] Volt-Watt response mode allows an inverter to reduce is real power output depending on the measured voltage. This mode is further described in AS4777.2:2015, section 6.3.2.2. True implies the mode is enabled." ;
    rdfs:domain cim:PowerElectronicsConnection ;
    rdfs:range xsd:boolean .

cim:PowerElectronicsConnection.invWattRespPAtV1 a rdf:Property ;
    rdfs:label "invWattRespPAtV1" ;
    rdfs:comment "\\[ZBEX\\] Power output set point 1 as a percentage of rated output for inverter Volt-Watt response mode. Permitted range is between 0 and 0.2 (inclusive)." ;
    rdfs:domain cim:PowerElectronicsConnection ;
    rdfs:range cim:PU .

cim:PowerElectronicsConnection.invWattRespPAtV2 a rdf:Property ;
    rdfs:label "invWattRespPAtV2" ;
    rdfs:comment "\\[ZBEX\\] Power output set point 2 as a percentage of rated output for inverter Volt-Watt response mode. Permitted range is between 0 and 0.2 (inclusive)." ;
    rdfs:domain cim:PowerElectronicsConnection ;
    rdfs:range cim:PU .

cim:PowerElectronicsConnection.invWattRespPAtV3 a rdf:Property ;
    rdfs:label "invWattRespPAtV3" ;
    rdfs:comment "\\[ZBEX\\] Power output set point 3 as a percentage of rated output for inverter Volt-Watt response mode. Permitted range is between 0 and 0.2 (inclusive)." ;
    rdfs:domain cim:PowerElectronicsConnection ;
    rdfs:range cim:PU .

cim:PowerElectronicsConnection.invWattRespPAtV4 a rdf:Property ;
    rdfs:label "invWattRespPAtV4" ;
    rdfs:comment "\\[ZBEX\\] Power output set point 4 as a percentage of rated output for inverter Volt-Watt response mode. Permitted range is between 0 and 0.2 (inclusive)." ;
    rdfs:domain cim:PowerElectronicsConnection ;
    rdfs:range cim:PU .

cim:PowerElectronicsConnection.invWattRespV1 a rdf:Property ;
    rdfs:label "invWattRespV1" ;
    rdfs:comment "\\[ZBEX\\] Set point 1 in volts for inverter Volt-Watt response mode. Permitted range is between 244 and 265 (inclusive)." ;
    rdfs:domain cim:PowerElectronicsConnection ;
    rdfs:range cim:Voltage .

cim:PowerElectronicsConnection.invWattRespV2 a rdf:Property ;
    rdfs:label "invWattRespV2" ;
    rdfs:comment "\\[ZBEX\\] Set point 2 in volts for inverter Volt-Watt response mode. Permitted range is between 244 and 265 (inclusive)." ;
    rdfs:domain cim:PowerElectronicsConnection ;
    rdfs:range cim:Voltage .

cim:PowerElectronicsConnection.invWattRespV3 a rdf:Property ;
    rdfs:label "invWattRespV3" ;
    rdfs:comment "\\[ZBEX\\] Set point 3 in volts for inverter Volt-Watt response mode. Permitted range is between 244 and 265 (inclusive)." ;
    rdfs:domain cim:PowerElectronicsConnection ;
    rdfs:range cim:Voltage .

cim:PowerElectronicsConnection.invWattRespV4 a rdf:Property ;
    rdfs:label "invWattRespV4" ;
    rdfs:comment "\\[ZBEX\\] Set point 4 in volts for inverter Volt-Watt response mode. Permitted range is between 244 and 265 (inclusive)." ;
    rdfs:domain cim:PowerElectronicsConnection ;
    rdfs:range cim:Voltage .

cim:PowerElectronicsConnection.inverterStandard a rdf:Property ;
    rdfs:label "inverterStandard" ;
    rdfs:comment "\\[ZBEX\\] The standard this inverter follows, such as AS4777.2:2020" ;
    rdfs:domain cim:PowerElectronicsConnection ;
    rdfs:range xsd:string .

cim:PowerElectronicsConnection.maxIFault a rdf:Property ;
    rdfs:label "maxIFault" ;
    rdfs:comment "Maximum fault current this device will contribute, in per-unit of rated current, before the converter protection will trip or bypass." ;
    rdfs:domain cim:PowerElectronicsConnection ;
    rdfs:range cim:PU .

cim:PowerElectronicsConnection.maxQ a rdf:Property ;
    rdfs:label "maxQ" ;
    rdfs:comment "Maximum reactive power limit. This is the maximum (nameplate) limit for the unit." ;
    rdfs:domain cim:PowerElectronicsConnection ;
    rdfs:range cim:ReactivePower .

cim:PowerElectronicsConnection.minQ a rdf:Property ;
    rdfs:label "minQ" ;
    rdfs:comment "Minimum reactive power limit for the unit. This is the minimum (nameplate) limit for the unit." ;
    rdfs:domain cim:PowerElectronicsConnection ;
    rdfs:range cim:ReactivePower .

cim:PowerElectronicsConnection.p a rdf:Property ;
    rdfs:label "p" ;
    rdfs:comment "Active power injection. Load sign convention is used, i.e. positive sign means flow out from a node.\nStarting value for a steady state solution." ;
    rdfs:domain cim:PowerElectronicsConnection ;
    rdfs:range cim:ActivePower .

cim:PowerElectronicsConnection.q a rdf:Property ;
    rdfs:label "q" ;
    rdfs:comment "Reactive power injection. Load sign convention is used, i.e. positive sign means flow out from a node.\nStarting value for a steady state solution." ;
    rdfs:domain cim:PowerElectronicsConnection ;
    rdfs:range cim:ReactivePower .

cim:PowerElectronicsConnection.ratedS a rdf:Property ;
    rdfs:label "ratedS" ;
    rdfs:comment "Nameplate apparent power rating for the unit.\nThe attribute shall have a positive value." ;
    rdfs:domain cim:PowerElectronicsConnection ;
    rdfs:range cim:ApparentPower .

cim:PowerElectronicsConnection.ratedU a rdf:Property ;
    rdfs:label "ratedU" ;
    rdfs:comment "Rated voltage (nameplate data, Ur in IEC 60909-0). It is primarily used for short circuit data exchange according to IEC 60909.\nThe attribute shall be a positive value." ;
    rdfs:domain cim:PowerElectronicsConnection ;
    rdfs:range cim:Voltage .

cim:PowerElectronicsConnection.stopAtOverFreq a rdf:Property ;
    rdfs:label "stopAtOverFreq" ;
    rdfs:comment "\\[ZBEX\\] Over frequency (stop) in Hz. Permitted range is between 51 and 52 (inclusive)" ;
    rdfs:domain cim:PowerElectronicsConnection ;
    rdfs:range cim:Frequency .

cim:PowerElectronicsConnection.stopAtUnderFreq a rdf:Property ;
    rdfs:label "stopAtUnderFreq" ;
    rdfs:comment "\\[ZBEX\\] Under frequency (stop) in Hz Permitted range is between 47 and 49 (inclusive)" ;
    rdfs:domain cim:PowerElectronicsConnection ;
    rdfs:range cim:Frequency .

cim:PowerElectronicsConnection.sustainOpOvervoltLimit a rdf:Property ;
    rdfs:label "sustainOpOvervoltLimit" ;
    rdfs:comment "\\[ZBEX\\] Indicates the sustained operation overvoltage limit in volts, when the average voltage for a 10-minute period exceeds the Vnom-max." ;
    rdfs:domain cim:PowerElectronicsConnection ;
    rdfs:range cim:Voltage .

cim:PowerElectronicsConnectionPhase.PowerElectronicsConnection a rdf:Property ;
    rdfs:label "PowerElectronicsConnectionPhase.PowerElectronicsConnection" ;
    rdfs:comment "The individual phases models for the power electronics connection. Power electronics connection of this power electronics connection phase." ;
    rdfs:domain cim:PowerElectronicsConnectionPhase ;
    rdfs:range cim:PowerElectronicsConnection ;
    profile:sourceCardinality "0..*" ;
    profile:targetCardinality "0..1" .

cim:PowerElectronicsConnectionPhase.p a rdf:Property ;
    rdfs:label "p" ;
    rdfs:comment "Active power injection. Load sign convention is used, i.e. positive sign means flow into the equipment from the network." ;
    rdfs:domain cim:PowerElectronicsConnectionPhase ;
    rdfs:range cim:ActivePower .

cim:PowerElectronicsConnectionPhase.phase a rdf:Property ;
    rdfs:label "phase" ;
    rdfs:comment "Phase of this energy producer component.   If the energy producer is wye connected, the connection is from the indicated phase to the central ground or neutral point.  If the energy producer is delta connected, the phase indicates an energy producer connected from the indicated phase to the next logical non-neutral phase." ;
    rdfs:domain cim:PowerElectronicsConnectionPhase ;
    rdfs:range cim:SinglePhaseKind .

cim:PowerElectronicsConnectionPhase.q a rdf:Property ;
    rdfs:label "q" ;
    rdfs:comment "Reactive power injection. Load sign convention is used, i.e. positive sign means flow into the equipment from the network." ;
    rdfs:domain cim:PowerElectronicsConnectionPhase ;
    rdfs:range cim:ReactivePower .

cim:PowerElectronicsUnit.PowerElectronicsConnection a rdf:Property ;
    rdfs:label "PowerElectronicsUnit.PowerElectronicsConnection" ;
    rdfs:comment "An AC network connection may have several power electronics units connecting through it. A power electronics unit has a connection to the AC network." ;
    rdfs:domain cim:PowerElectronicsUnit ;
    rdfs:range cim:PowerElectronicsConnection ;
    profile:sourceCardinality "0..*" ;
    profile:targetCardinality "0..1" .

cim:PowerElectronicsUnit.maxP a rdf:Property ;
    rdfs:label "maxP" ;
    rdfs:comment "Maximum active power limit. This is the maximum (nameplate) limit for the unit." ;
    rdfs:domain cim:PowerElectronicsUnit ;
    rdfs:range cim:ActivePower .

cim:PowerElectronicsUnit.minP a rdf:Property ;
    rdfs:label "minP" ;
    rdfs:comment "Minimum active power limit. This is the minimum (nameplate) limit for the unit." ;
    rdfs:domain cim:PowerElectronicsUnit ;
    rdfs:range cim:ActivePower .

cim:PowerSystemResource.Asset a rdf:Property ;
    rdfs:label "PowerSystemResource.Asset" ;
    rdfs:comment "All assets represented by this power system resource. For example, multiple conductor assets are electrically modelled as a single AC line segment." ;
    rdfs:domain cim:PowerSystemResource ;
    rdfs:range cim:Asset ;
    profile:targetCardinality "0..*" .

cim:PowerSystemResource.AssetInfo a rdf:Property ;
    rdfs:label "PowerSystemResource.AssetInfo" ;
    rdfs:comment "Datasheet information for this power system resource." ;
    rdfs:domain cim:PowerSystemResource ;
    rdfs:range cim:AssetInfo ;
    profile:targetCardinality "0..1" .

cim:PowerSystemResource.Location a rdf:Property ;
    rdfs:label "PowerSystemResource.Location" ;
    rdfs:comment "Location of this power system resource." ;
    rdfs:domain cim:PowerSystemResource ;
    rdfs:range cim:Location ;
    profile:targetCardinality "0..1" .

cim:PowerSystemResource.numControls a rdf:Property ;
    rdfs:label "numControls" ;
    rdfs:comment "The controller outputs used to actually govern a regulating device, e.g. the magnetization of a synchronous machine or capacitor bank breaker actuator." ;
    rdfs:domain cim:PowerSystemResource ;
    rdfs:range xsd:int .

cim:PowerTransformer.PowerTransformerEnd a rdf:Property ;
    rdfs:label "PowerTransformer.PowerTransformerEnd" ;
    rdfs:comment "The power transformer of this power transformer end. The ends of this power transformer." ;
    rdfs:domain cim:PowerTransformer ;
    rdfs:range cim:PowerTransformerEnd ;
    profile:sourceCardinality "0..1" ;
    profile:targetCardinality "0..*" .

cim:PowerTransformer.constructionKind a rdf:Property ;
    rdfs:label "constructionKind" ;
    rdfs:comment "The construction kind of this transformer" ;
    rdfs:domain cim:PowerTransformer ;
    rdfs:range cim:TransformerConstructionKind .

cim:PowerTransformer.function a rdf:Property ;
    rdfs:label "function" ;
    rdfs:comment "The function of this transformer" ;
    rdfs:domain cim:PowerTransformer ;
    rdfs:range cim:TransformerFunctionKind .

cim:PowerTransformer.transformerUtilisation a rdf:Property ;
    rdfs:label "transformerUtilisation" ;
    rdfs:comment "The fraction of the transformers normal capacity (nameplate rating) that is in use. It may be expressed as the result of the calculation S/Sn, where S = Load on Transformer (in VA), Sn = Transformer Nameplate Rating (in VA)." ;
    rdfs:domain cim:PowerTransformer ;
    rdfs:range cim:PU .

cim:PowerTransformer.vectorGroup a rdf:Property ;
    rdfs:label "vectorGroup" ;
    rdfs:comment "Vector group of the transformer for protective relaying, e.g., Dyn1. For unbalanced transformers, this may not be simply determined from the constituent winding connections and phase angle displacements.\n\nThe vectorGroup string consists of the following components in the order listed: high voltage winding connection, mid voltage winding connection (for three winding transformers), phase displacement clock number from 0 to 11,  low voltage winding connection \nphase displacement clock number from 0 to 11.   The winding connections are D (delta), Y (wye), YN (wye with neutral), Z (zigzag), ZN (zigzag with neutral), A (auto transformer). Upper case means the high voltage, lower case mid or low. The high voltage winding always has clock position 0 and is not included in the vector group string.  Some examples: YNy0 (two winding wye to wye with no phase displacement), YNd11 (two winding wye to delta with 330 degrees phase displacement), YNyn0d5 (three winding transformer wye with neutral high voltage, wye with neutral mid voltage and no phase displacement, delta low voltage with 150 degrees displacement).\n\nPhase displacement is defined as the angular difference between the phasors representing the voltages between the neutral point (real or imaginary) and the corresponding terminals of two windings, a positive sequence voltage system being applied to the high-voltage terminals, following each other in alphabetical sequence if they are lettered, or in numerical sequence if they are numbered: the phasors are assumed to rotate in a counter-clockwise sense." ;
    rdfs:domain cim:PowerTransformer ;
    rdfs:range xsd:string .

cim:PowerTransformerEnd.PowerTransformer a rdf:Property ;
    rdfs:label "PowerTransformerEnd.PowerTransformer" ;
    rdfs:comment "The ends of this power transformer. The power transformer of this power transformer end." ;
    rdfs:domain cim:PowerTransformerEnd ;
    rdfs:range cim:PowerTransformer ;
    profile:sourceCardinality "0..*" ;
    profile:targetCardinality "0..1" .

cim:PowerTransformerEnd.TransformerEndRatedS a rdf:Property ;
    rdfs:label "PowerTransformerEnd.TransformerEndRatedS" ;
    rdfs:comment "\\[ZBEX\\] The normal apparent power ratings for this PowerTransformerEnd." ;
    rdfs:domain cim:PowerTransformerEnd ;
    rdfs:range cim:TransformerEndRatedS ;
    profile:targetCardinality "0..*" .

cim:PowerTransformerEnd.b a rdf:Property ;
    rdfs:label "b" ;
    rdfs:comment "Magnetizing branch susceptance (B mag).  The value can be positive or negative." ;
    rdfs:domain cim:PowerTransformerEnd ;
    rdfs:range cim:Susceptance .

cim:PowerTransformerEnd.b0 a rdf:Property ;
    rdfs:label "b0" ;
    rdfs:comment "Zero sequence magnetizing branch susceptance." ;
    rdfs:domain cim:PowerTransformerEnd ;
    rdfs:range cim:Susceptance .

cim:PowerTransformerEnd.connectionKind a rdf:Property ;
    rdfs:label "connectionKind" ;
    rdfs:comment "Kind of connection." ;
    rdfs:domain cim:PowerTransformerEnd ;
    rdfs:range cim:WindingConnection .

cim:PowerTransformerEnd.g a rdf:Property ;
    rdfs:label "g" ;
    rdfs:comment "Magnetizing branch conductance." ;
    rdfs:domain cim:PowerTransformerEnd ;
    rdfs:range cim:Conductance .

cim:PowerTransformerEnd.g0 a rdf:Property ;
    rdfs:label "g0" ;
    rdfs:comment "Zero sequence magnetizing branch conductance (star-model)." ;
    rdfs:domain cim:PowerTransformerEnd ;
    rdfs:range cim:Conductance .

cim:PowerTransformerEnd.phaseAngleClock a rdf:Property ;
    rdfs:label "phaseAngleClock" ;
    rdfs:comment "Terminal voltage phase angle displacement where 360 degrees are represented with clock hours. The valid values are 0 to 11. For example, for the secondary side end of a transformer with vector group code of 'Dyn11', specify the connection kind as wye with neutral and specify the phase angle of the clock as 11.  The clock value of the transformer end number specified as 1, is assumed to be zero.  Note the transformer end number is not assumed to be the same as the terminal sequence number." ;
    rdfs:domain cim:PowerTransformerEnd ;
    rdfs:range xsd:int .

cim:PowerTransformerEnd.r a rdf:Property ;
    rdfs:label "r" ;
    rdfs:comment "Resistance (star-model) of the transformer end.\nThe attribute shall be equal to or greater than zero for non-equivalent transformers." ;
    rdfs:domain cim:PowerTransformerEnd ;
    rdfs:range cim:Resistance .

cim:PowerTransformerEnd.r0 a rdf:Property ;
    rdfs:label "r0" ;
    rdfs:comment "Zero sequence series resistance (star-model) of the transformer end." ;
    rdfs:domain cim:PowerTransformerEnd ;
    rdfs:range cim:Resistance .

cim:PowerTransformerEnd.ratedS a rdf:Property ;
    rdfs:label "ratedS" ;
    rdfs:comment "Normal apparent power rating.\nThe attribute shall be a positive value. For a two-winding transformer the values for the high and low voltage sides shall be identical." ;
    rdfs:domain cim:PowerTransformerEnd ;
    rdfs:range cim:ApparentPower .

cim:PowerTransformerEnd.ratedU a rdf:Property ;
    rdfs:label "ratedU" ;
    rdfs:comment "Rated voltage: phase-phase for three-phase windings, and either phase-phase or phase-neutral for single-phase windings.\nA high voltage side, as given by TransformerEnd.endNumber, shall have a ratedU that is greater than or equal to ratedU for the lower voltage sides.\nThe attribute shall be a positive value." ;
    rdfs:domain cim:PowerTransformerEnd ;
    rdfs:range cim:Voltage .

cim:PowerTransformerEnd.x a rdf:Property ;
    rdfs:label "x" ;
    rdfs:comment "Positive sequence series reactance (star-model) of the transformer end." ;
    rdfs:domain cim:PowerTransformerEnd ;
    rdfs:range cim:Reactance .

cim:PowerTransformerEnd.x0 a rdf:Property ;
    rdfs:label "x0" ;
    rdfs:comment "Zero sequence series reactance of the transformer end." ;
    rdfs:domain cim:PowerTransformerEnd ;
    rdfs:range cim:Reactance .

cim:PowerTransformerInfo.TransformerTankInfo a rdf:Property ;
    rdfs:label "PowerTransformerInfo.TransformerTankInfo" ;
    rdfs:comment "Power transformer data that this tank description is part of. Data for all the tanks described by this power transformer data." ;
    rdfs:domain cim:PowerTransformerInfo ;
    rdfs:range cim:TransformerTankInfo ;
    profile:sourceCardinality "0..1" ;
    profile:targetCardinality "0..*" .

cim:PricingStructure.Tariff a rdf:Property ;
    rdfs:label "PricingStructure.Tariff" ;
    rdfs:comment "All tariffs used by this pricing structure." ;
    rdfs:domain cim:PricingStructure ;
    rdfs:range cim:Tariff ;
    profile:targetCardinality "0..*" .

cim:ProtectedSwitch.ProtectionRelayFunction a rdf:Property ;
    rdfs:label "ProtectedSwitch.ProtectionRelayFunction" ;
    rdfs:comment "\\[ZBEX\\] The ProtectedSwitches operated by this ProtectionRelayFunction. \\[ZBEX\\] The ProtectionRelayFunctions operating this ProtectedSwitch." ;
    rdfs:domain cim:ProtectedSwitch ;
    rdfs:range cim:ProtectionRelayFunction ;
    profile:sourceCardinality "0..*" ;
    profile:targetCardinality "0..*" .

cim:ProtectedSwitch.breakingCapacity a rdf:Property ;
    rdfs:label "breakingCapacity" ;
    rdfs:comment "The maximum fault current in amps a breaking device can break safely under prescribed conditions of use." ;
    rdfs:domain cim:ProtectedSwitch ;
    rdfs:range cim:CurrentFlow .

cim:ProtectionKind.AUTO_TRANSFORMER a rdf:Property ;
    rdfs:label "AUTO_TRANSFORMER" ;
    rdfs:comment "\\[ZBEX\\] A device used to regulate the voltage of transmission lines and can also be used to transform voltages." ;
    rdfs:domain cim:ProtectionKind ;
    rdfs:range xsd:string .

cim:ProtectionKind.DISTANCE a rdf:Property ;
    rdfs:label "DISTANCE" ;
    rdfs:comment "\\[ZBEX\\] A device used to detect faults on long-distance lines, pinpointing not only the fault condition but also measuring the distance between the current sensing mechanism and the fault location in the wire." ;
    rdfs:domain cim:ProtectionKind ;
    rdfs:range xsd:string .

cim:ProtectionKind.FREQ a rdf:Property ;
    rdfs:label "FREQ" ;
    rdfs:comment "\\[ZBEX\\] Under frequency" ;
    rdfs:domain cim:ProtectionKind ;
    rdfs:range xsd:string .

cim:ProtectionKind.FREQG a rdf:Property ;
    rdfs:label "FREQG" ;
    rdfs:comment "\\[ZBEX\\] Over frequency" ;
    rdfs:domain cim:ProtectionKind ;
    rdfs:range xsd:string .

cim:ProtectionKind.GROUND_CURRENT a rdf:Property ;
    rdfs:label "GROUND_CURRENT" ;
    rdfs:comment "\\[ZBEX\\] A device used to monitor and protect electrical equipment from damage caused by ground faults" ;
    rdfs:domain cim:ProtectionKind ;
    rdfs:range xsd:string .

cim:ProtectionKind.GROUND_VOLTAGE a rdf:Property ;
    rdfs:label "GROUND_VOLTAGE" ;
    rdfs:comment "\\[ZBEX\\] A device used to detect contact accidents between an electric path and ground caused by arc ground faults" ;
    rdfs:domain cim:ProtectionKind ;
    rdfs:range xsd:string .

cim:ProtectionKind.J0 a rdf:Property ;
    rdfs:label "J0" ;
    rdfs:comment "\\[ZBEX\\] Ground overcurrent" ;
    rdfs:domain cim:ProtectionKind ;
    rdfs:range xsd:string .

cim:ProtectionKind.J0GG a rdf:Property ;
    rdfs:label "J0GG" ;
    rdfs:comment "\\[ZBEX\\] Instantaneous ground overcurrent" ;
    rdfs:domain cim:ProtectionKind ;
    rdfs:range xsd:string .

cim:ProtectionKind.J2G a rdf:Property ;
    rdfs:label "J2G" ;
    rdfs:comment "\\[ZBEX\\] Negative-sequence overcurrent" ;
    rdfs:domain cim:ProtectionKind ;
    rdfs:range xsd:string .

cim:ProtectionKind.JDIFF a rdf:Property ;
    rdfs:label "JDIFF" ;
    rdfs:comment "\\[ZBEX\\] Differential Current" ;
    rdfs:domain cim:ProtectionKind ;
    rdfs:range xsd:string .

cim:ProtectionKind.JG a rdf:Property ;
    rdfs:label "JG" ;
    rdfs:comment "\\[ZBEX\\] Overcurrent" ;
    rdfs:domain cim:ProtectionKind ;
    rdfs:range xsd:string .

cim:ProtectionKind.JGG a rdf:Property ;
    rdfs:label "JGG" ;
    rdfs:comment "\\[ZBEX\\] Instantaneous" ;
    rdfs:domain cim:ProtectionKind ;
    rdfs:range xsd:string .

cim:ProtectionKind.JGGG a rdf:Property ;
    rdfs:label "JGGG" ;
    rdfs:comment "\\[ZBEX\\] Instantaneous" ;
    rdfs:domain cim:ProtectionKind ;
    rdfs:range xsd:string .

cim:ProtectionKind.JT a rdf:Property ;
    rdfs:label "JT" ;
    rdfs:comment "\\[ZBEX\\] Thermal overload" ;
    rdfs:domain cim:ProtectionKind ;
    rdfs:range xsd:string .

cim:ProtectionKind.LE a rdf:Property ;
    rdfs:label "LE" ;
    rdfs:comment "\\[ZBEX\\] Load encroachment" ;
    rdfs:domain cim:ProtectionKind ;
    rdfs:range xsd:string .

cim:ProtectionKind.MULTI_FUNCTION a rdf:Property ;
    rdfs:label "MULTI_FUNCTION" ;
    rdfs:comment "\\[ZBEX\\] A multifunctional relay for universal usages" ;
    rdfs:domain cim:ProtectionKind ;
    rdfs:range xsd:string .

cim:ProtectionKind.NEGATIVE_OVERCURRENT a rdf:Property ;
    rdfs:label "NEGATIVE_OVERCURRENT" ;
    rdfs:comment "\\[ZBEX\\] A device used to protect generators from the unbalanced load by detecting negative sequence current." ;
    rdfs:domain cim:ProtectionKind ;
    rdfs:range xsd:string .

cim:ProtectionKind.NETWORK_PROTECTOR a rdf:Property ;
    rdfs:label "NETWORK_PROTECTOR" ;
    rdfs:comment "\\[ZBEX\\] Is a special self-contained air breaker or switching unit having a full complement of current, potential and control transformers, as well as relay functionality." ;
    rdfs:domain cim:ProtectionKind ;
    rdfs:range xsd:string .

cim:ProtectionKind.POWER a rdf:Property ;
    rdfs:label "POWER" ;
    rdfs:comment "\\[ZBEX\\] A device that uses an electromagnet to open or close a circuit when the input (coil) is correctly excited" ;
    rdfs:domain cim:ProtectionKind ;
    rdfs:range xsd:string .

cim:ProtectionKind.SECTIONALIZER a rdf:Property ;
    rdfs:label "SECTIONALIZER" ;
    rdfs:comment "\\[ZBEX\\] A device that automatically isolates a faulted section of line from the rest of the distribution system" ;
    rdfs:domain cim:ProtectionKind ;
    rdfs:range xsd:string .

cim:ProtectionKind.SEF a rdf:Property ;
    rdfs:label "SEF" ;
    rdfs:comment "\\[ZBEX\\] Sensitive earth fault" ;
    rdfs:domain cim:ProtectionKind ;
    rdfs:range xsd:string .

cim:ProtectionKind.UNKNOWN a rdf:Property ;
    rdfs:label "UNKNOWN" ;
    rdfs:comment "\\[ZBEX\\] Unknown" ;
    rdfs:domain cim:ProtectionKind ;
    rdfs:range xsd:string .

cim:ProtectionKind.V0G a rdf:Property ;
    rdfs:label "V0G" ;
    rdfs:comment "\\[ZBEX\\] Zero-sequence overvoltage" ;
    rdfs:domain cim:ProtectionKind ;
    rdfs:range xsd:string .

cim:ProtectionKind.V0GG a rdf:Property ;
    rdfs:label "V0GG" ;
    rdfs:comment "\\[ZBEX\\] Instantaneous zero-sequence overvoltage" ;
    rdfs:domain cim:ProtectionKind ;
    rdfs:range xsd:string .

cim:ProtectionKind.VG a rdf:Property ;
    rdfs:label "VG" ;
    rdfs:comment "\\[ZBEX\\] Overvoltage" ;
    rdfs:domain cim:ProtectionKind ;
    rdfs:range xsd:string .

cim:ProtectionKind.VGG a rdf:Property ;
    rdfs:label "VGG" ;
    rdfs:comment "\\[ZBEX\\] Instantaneous overvoltage" ;
    rdfs:domain cim:ProtectionKind ;
    rdfs:range xsd:string .

cim:ProtectionKind.VL a rdf:Property ;
    rdfs:label "VL" ;
    rdfs:comment "\\[ZBEX\\] Undervoltage" ;
    rdfs:domain cim:ProtectionKind ;
    rdfs:range xsd:string .

cim:ProtectionKind.VLL a rdf:Property ;
    rdfs:label "VLL" ;
    rdfs:comment "\\[ZBEX\\] Instantaneous" ;
    rdfs:domain cim:ProtectionKind ;
    rdfs:range xsd:string .

cim:ProtectionKind.Z0L a rdf:Property ;
    rdfs:label "Z0L" ;
    rdfs:comment "\\[ZBEX\\] Ground distance" ;
    rdfs:domain cim:ProtectionKind ;
    rdfs:range xsd:string .

cim:ProtectionKind.ZL a rdf:Property ;
    rdfs:label "ZL" ;
    rdfs:comment "\\[ZBEX\\] Phase distance" ;
    rdfs:domain cim:ProtectionKind ;
    rdfs:range xsd:string .

cim:ProtectionRelayFunction.ProtectedSwitch a rdf:Property ;
    rdfs:label "ProtectionRelayFunction.ProtectedSwitch" ;
    rdfs:comment "\\[ZBEX\\] The ProtectionRelayFunctions operating this ProtectedSwitch. \\[ZBEX\\] The ProtectedSwitches operated by this ProtectionRelayFunction." ;
    rdfs:domain cim:ProtectionRelayFunction ;
    rdfs:range cim:ProtectedSwitch ;
    profile:sourceCardinality "0..*" ;
    profile:targetCardinality "0..*" .

cim:ProtectionRelayFunction.ProtectionRelayScheme a rdf:Property ;
    rdfs:label "ProtectionRelayFunction.ProtectionRelayScheme" ;
    rdfs:comment "\\[ZBEX\\] The functions operated as part of this protection scheme. \\[ZBEX\\] The schemes this function operates under." ;
    rdfs:domain cim:ProtectionRelayFunction ;
    rdfs:range cim:ProtectionRelayScheme ;
    profile:sourceCardinality "0..*" ;
    profile:targetCardinality "0..*" .

cim:ProtectionRelayFunction.RelaySetting a rdf:Property ;
    rdfs:label "ProtectionRelayFunction.RelaySetting" ;
    rdfs:comment "\\[ZBEX\\] The thresholds for this relay function. The order of thresholds corresponds to the order of time limits." ;
    rdfs:domain cim:ProtectionRelayFunction ;
    rdfs:range cim:RelaySetting ;
    profile:targetCardinality "0..*" .

cim:ProtectionRelayFunction.Sensor a rdf:Property ;
    rdfs:label "ProtectionRelayFunction.Sensor" ;
    rdfs:comment "\\[ZBEX\\] The relay functions influenced by this Sensor \\[ZBEX\\] The Sensors for this relay function." ;
    rdfs:domain cim:ProtectionRelayFunction ;
    rdfs:range cim:Sensor ;
    profile:sourceCardinality "0..*" ;
    profile:targetCardinality "0..*" .

cim:ProtectionRelayFunction.directable a rdf:Property ;
    rdfs:label "directable" ;
    rdfs:comment "\\[ZBEX\\] Whether this ProtectionRelayFunction responds to power flow in a given direction." ;
    rdfs:domain cim:ProtectionRelayFunction ;
    rdfs:range xsd:boolean .

cim:ProtectionRelayFunction.model a rdf:Property ;
    rdfs:label "model" ;
    rdfs:comment "\\[ZBEX\\] The protection equipment type name (manufacturer information)" ;
    rdfs:domain cim:ProtectionRelayFunction ;
    rdfs:range xsd:string .

cim:ProtectionRelayFunction.powerDirection a rdf:Property ;
    rdfs:label "powerDirection" ;
    rdfs:comment "\\[ZBEX\\] The flow of power direction used by this ProtectionRelayFunction." ;
    rdfs:domain cim:ProtectionRelayFunction ;
    rdfs:range cim:PowerDirectionKind .

cim:ProtectionRelayFunction.protectionKind a rdf:Property ;
    rdfs:label "protectionKind" ;
    rdfs:comment "\\[ZBEX\\] The kind of protection being provided by this ProtectionRelayFunction." ;
    rdfs:domain cim:ProtectionRelayFunction ;
    rdfs:range cim:ProtectionKind .

cim:ProtectionRelayFunction.reclosing a rdf:Property ;
    rdfs:label "reclosing" ;
    rdfs:comment "\\[ZBEX\\] True if the protection equipment is reclosing or False otherwise." ;
    rdfs:domain cim:ProtectionRelayFunction ;
    rdfs:range xsd:boolean .

cim:ProtectionRelayFunction.relayDelayTime a rdf:Property ;
    rdfs:label "relayDelayTime" ;
    rdfs:comment "\\[ZBEX\\] The time delay from detection of abnormal conditions to relay operation in seconds." ;
    rdfs:domain cim:ProtectionRelayFunction ;
    rdfs:range cim:Secondsyaml .

cim:ProtectionRelayFunction.timeLimits a rdf:Property ;
    rdfs:label "timeLimits" ;
    rdfs:comment "\\[ZBEX\\] The time limits (in seconds) for this relay function. Order of entries corresponds to the order of entries in thresholds." ;
    rdfs:domain cim:ProtectionRelayFunction ;
    rdfs:range cim:SecondsyamlList .

cim:ProtectionRelayScheme.ProtectionRelayFunction a rdf:Property ;
    rdfs:label "ProtectionRelayScheme.ProtectionRelayFunction" ;
    rdfs:comment "\\[ZBEX\\] The schemes this function operates under. \\[ZBEX\\] The functions operated as part of this protection scheme." ;
    rdfs:domain cim:ProtectionRelayScheme ;
    rdfs:range cim:ProtectionRelayFunction ;
    profile:sourceCardinality "0..*" ;
    profile:targetCardinality "0..*" .

cim:ProtectionRelayScheme.ProtectionRelaySystem a rdf:Property ;
    rdfs:label "ProtectionRelayScheme.ProtectionRelaySystem" ;
    rdfs:comment "\\[ZBEX\\] The schemes implemented by this ProtectionRelaySystem. \\[ZBEX\\] The system this scheme belongs to." ;
    rdfs:domain cim:ProtectionRelayScheme ;
    rdfs:range cim:ProtectionRelaySystem ;
    profile:sourceCardinality "0..*" ;
    profile:targetCardinality "0..1" .

cim:ProtectionRelaySystem.ProtectionRelayScheme a rdf:Property ;
    rdfs:label "ProtectionRelaySystem.ProtectionRelayScheme" ;
    rdfs:comment "\\[ZBEX\\] The system this scheme belongs to. \\[ZBEX\\] The schemes implemented by this ProtectionRelaySystem." ;
    rdfs:domain cim:ProtectionRelaySystem ;
    rdfs:range cim:ProtectionRelayScheme ;
    profile:sourceCardinality "0..1" ;
    profile:targetCardinality "0..*" .

cim:ProtectionRelaySystem.protectionKind a rdf:Property ;
    rdfs:label "protectionKind" ;
    rdfs:comment "\\[ZBEX\\] The kind of protection being provided by this protection equipment." ;
    rdfs:domain cim:ProtectionRelaySystem ;
    rdfs:range cim:ProtectionKind .

cim:Ratio.denominator a rdf:Property ;
    rdfs:label "denominator" ;
    rdfs:comment "The part of a fraction that is below the line and that functions as the divisor of the numerator." ;
    rdfs:domain cim:Ratio ;
    rdfs:range xsd:double .

cim:Ratio.numerator a rdf:Property ;
    rdfs:label "numerator" ;
    rdfs:comment "The part of a fraction that is above the line and signifies the number to be divided by the denominator." ;
    rdfs:domain cim:Ratio ;
    rdfs:range xsd:double .

cim:RatioTapChanger.TransformerEnd a rdf:Property ;
    rdfs:label "RatioTapChanger.TransformerEnd" ;
    rdfs:comment "Transformer end to which this ratio tap changer belongs." ;
    rdfs:domain cim:RatioTapChanger ;
    rdfs:range cim:TransformerEnd ;
    profile:targetCardinality "0..1" .

cim:RatioTapChanger.stepVoltageIncrement a rdf:Property ;
    rdfs:label "stepVoltageIncrement" ;
    rdfs:comment "Tap step increment, in per cent of rated voltage of the power transformer end, per step position.\nWhen the increment is negative, the voltage decreases when the tap step increases." ;
    rdfs:domain cim:RatioTapChanger ;
    rdfs:range cim:PerCent .

cim:Reactance.value a rdf:Property ;
    rdfs:label "value" ;
    rdfs:comment "ohms (ohm)" ;
    rdfs:domain cim:Reactance ;
    rdfs:range xsd:double .

cim:ReactancePerLength.value a rdf:Property ;
    rdfs:label "value" ;
    rdfs:comment "ohms per metre (ohmPerm)" ;
    rdfs:domain cim:ReactancePerLength ;
    rdfs:range xsd:double .

cim:ReactivePower.value a rdf:Property ;
    rdfs:label "value" ;
    rdfs:comment "volt amperes reactive (VAr)" ;
    rdfs:domain cim:ReactivePower ;
    rdfs:range xsd:double .

cim:RegulatingCondEq.RegulatingControl a rdf:Property ;
    rdfs:label "RegulatingCondEq.RegulatingControl" ;
    rdfs:comment "The equipment that participates in this regulating control scheme. The regulating control scheme in which this equipment participates." ;
    rdfs:domain cim:RegulatingCondEq ;
    rdfs:range cim:RegulatingControl ;
    profile:sourceCardinality "0..*" ;
    profile:targetCardinality "0..1" .

cim:RegulatingCondEq.controlEnabled a rdf:Property ;
    rdfs:label "controlEnabled" ;
    rdfs:comment "Specifies the regulation status of the equipment.  True is regulating, false is not regulating." ;
    rdfs:domain cim:RegulatingCondEq ;
    rdfs:range xsd:boolean .

cim:RegulatingControl.RegulatingCondEq a rdf:Property ;
    rdfs:label "RegulatingControl.RegulatingCondEq" ;
    rdfs:comment "The regulating control scheme in which this equipment participates. The equipment that participates in this regulating control scheme." ;
    rdfs:domain cim:RegulatingControl ;
    rdfs:range cim:RegulatingCondEq ;
    profile:sourceCardinality "0..1" ;
    profile:targetCardinality "0..*" .

cim:RegulatingControl.Terminal a rdf:Property ;
    rdfs:label "RegulatingControl.Terminal" ;
    rdfs:comment "The terminal associated with this regulating control.  The terminal is associated instead of a node, since the terminal could connect into either a topological node or a connectivity node.  Sometimes it is useful to model regulation at a terminal of a bus bar object." ;
    rdfs:domain cim:RegulatingControl ;
    rdfs:range cim:Terminal ;
    profile:targetCardinality "0..1" .

cim:RegulatingControl.ctPrimary a rdf:Property ;
    rdfs:label "ctPrimary" ;
    rdfs:comment "\\[ZBEX\\] Current rating of the CT, expressed in terms of the current (in Amperes) that flows in the Primary where the 'Primary' is the conductor being monitored. It ensures proper operation of the regulating equipment by providing the necessary current references for control actions. An important side effect of this current value is that it also defines the current value at which the full LDC R and X voltages are applied by the controller, where enabled." ;
    rdfs:domain cim:RegulatingControl ;
    rdfs:range cim:CurrentFlow .

cim:RegulatingControl.discrete a rdf:Property ;
    rdfs:label "discrete" ;
    rdfs:comment "The regulation is performed in a discrete mode. This applies to equipment with discrete controls, e.g. tap changers and shunt compensators." ;
    rdfs:domain cim:RegulatingControl ;
    rdfs:range xsd:boolean .

cim:RegulatingControl.enabled a rdf:Property ;
    rdfs:label "enabled" ;
    rdfs:comment "The flag tells if regulation is enabled." ;
    rdfs:domain cim:RegulatingControl ;
    rdfs:range xsd:boolean .

cim:RegulatingControl.maxAllowedTargetValue a rdf:Property ;
    rdfs:label "maxAllowedTargetValue" ;
    rdfs:comment "Maximum allowed target value (RegulatingControl.targetValue)." ;
    rdfs:domain cim:RegulatingControl ;
    rdfs:range xsd:double .

cim:RegulatingControl.minAllowedTargetValue a rdf:Property ;
    rdfs:label "minAllowedTargetValue" ;
    rdfs:comment "Minimum allowed target value (RegulatingControl.targetValue)." ;
    rdfs:domain cim:RegulatingControl ;
    rdfs:range xsd:double .

cim:RegulatingControl.minTargetDeadband a rdf:Property ;
    rdfs:label "minTargetDeadband" ;
    rdfs:comment "\\[ZBEX\\] This is the minimum allowable range for discrete control in regulating devices, used to prevent frequent control actions and promote operational stability. This attribute sets a baseline range within which no adjustments are made, applicable across various devices like voltage regulators, shunt compensators, or battery units." ;
    rdfs:domain cim:RegulatingControl ;
    rdfs:range xsd:double .

cim:RegulatingControl.mode a rdf:Property ;
    rdfs:label "mode" ;
    rdfs:comment "The regulating control mode presently available.  This specification allows for determining the kind of regulation without need for obtaining the units from a schedule." ;
    rdfs:domain cim:RegulatingControl ;
    rdfs:range cim:RegulatingControlModeKind .

cim:RegulatingControl.monitoredPhase a rdf:Property ;
    rdfs:label "monitoredPhase" ;
    rdfs:comment "Phase voltage controlling this regulator, measured at regulator location." ;
    rdfs:domain cim:RegulatingControl ;
    rdfs:range cim:PhaseCode .

cim:RegulatingControl.ratedCurrent a rdf:Property ;
    rdfs:label "ratedCurrent" ;
    rdfs:comment "\\[ZBEX\\] The rated current of associated CT in amps for this RegulatingControl. Forms the base used to convert Line Drop Compensation settings from ohms to voltage." ;
    rdfs:domain cim:RegulatingControl ;
    rdfs:range cim:CurrentFlow .

cim:RegulatingControl.targetDeadband a rdf:Property ;
    rdfs:label "targetDeadband" ;
    rdfs:comment "This is a deadband used with discrete control to avoid excessive update of controls like tap changers and shunt compensator banks while regulating.  The units of those appropriate for the mode. The attribute shall be a positive value or zero. If RegulatingControl.discrete is set to \"false\", the RegulatingControl.targetDeadband is to be ignored.\nNote that for instance, if the targetValue is 100 kV and the targetDeadband is 2 kV the range is from 99 to 101 kV." ;
    rdfs:domain cim:RegulatingControl ;
    rdfs:range xsd:double .

cim:RegulatingControl.targetValue a rdf:Property ;
    rdfs:label "targetValue" ;
    rdfs:comment "The target value specified for case input.   This value can be used for the target value without the use of schedules. The value has the units appropriate to the mode attribute." ;
    rdfs:domain cim:RegulatingControl ;
    rdfs:range xsd:double .

cim:RegulatingControlModeKind.UNKNOWN_CONTROL_MODE a rdf:Property ;
    rdfs:label "UNKNOWN_CONTROL_MODE" ;
    rdfs:comment "" ;
    rdfs:domain cim:RegulatingControlModeKind ;
    rdfs:range xsd:string .

cim:RegulatingControlModeKind.activePower a rdf:Property ;
    rdfs:label "activePower" ;
    rdfs:comment "Active power is specified." ;
    rdfs:domain cim:RegulatingControlModeKind ;
    rdfs:range xsd:string .

cim:RegulatingControlModeKind.admittance a rdf:Property ;
    rdfs:label "admittance" ;
    rdfs:comment "Admittance is specified." ;
    rdfs:domain cim:RegulatingControlModeKind ;
    rdfs:range xsd:string .

cim:RegulatingControlModeKind.currentFlow a rdf:Property ;
    rdfs:label "currentFlow" ;
    rdfs:comment "Current flow is specified." ;
    rdfs:domain cim:RegulatingControlModeKind ;
    rdfs:range xsd:string .

cim:RegulatingControlModeKind.powerFactor a rdf:Property ;
    rdfs:label "powerFactor" ;
    rdfs:comment "Power factor is specified." ;
    rdfs:domain cim:RegulatingControlModeKind ;
    rdfs:range xsd:string .

cim:RegulatingControlModeKind.reactivePower a rdf:Property ;
    rdfs:label "reactivePower" ;
    rdfs:comment "Reactive power is specified." ;
    rdfs:domain cim:RegulatingControlModeKind ;
    rdfs:range xsd:string .

cim:RegulatingControlModeKind.temperature a rdf:Property ;
    rdfs:label "temperature" ;
    rdfs:comment "Control switches on/off based on the local temperature (i.e., a thermostat)." ;
    rdfs:domain cim:RegulatingControlModeKind ;
    rdfs:range xsd:string .

cim:RegulatingControlModeKind.timeScheduled a rdf:Property ;
    rdfs:label "timeScheduled" ;
    rdfs:comment "Control switches on/off by time of day. The times may change on the weekend, or in different seasons." ;
    rdfs:domain cim:RegulatingControlModeKind ;
    rdfs:range xsd:string .

cim:RegulatingControlModeKind.voltage a rdf:Property ;
    rdfs:label "voltage" ;
    rdfs:comment "Voltage is specified." ;
    rdfs:domain cim:RegulatingControlModeKind ;
    rdfs:range xsd:string .

cim:RelayInfo.curveSetting a rdf:Property ;
    rdfs:label "curveSetting" ;
    rdfs:comment "\\[ZBEX\\] The type of curve used for the Relay." ;
    rdfs:domain cim:RelayInfo ;
    rdfs:range xsd:string .

cim:RelayInfo.recloseDelays a rdf:Property ;
    rdfs:label "recloseDelays" ;
    rdfs:comment "\\[ZBEX\\] The reclose delays for this curve and relay type (in seconds). The index of the list is the reclose step, and the value is the overall delay time." ;
    rdfs:domain cim:RelayInfo ;
    rdfs:range cim:SecondsList .

cim:RelayInfo.recloseFast a rdf:Property ;
    rdfs:label "recloseFast" ;
    rdfs:comment "\\[ZBEX\\] True if recloseDelays are associated with a fast Curve, False otherwise." ;
    rdfs:domain cim:RelayInfo ;
    rdfs:range xsd:boolean .

cim:RelaySetting.name a rdf:Property ;
    rdfs:label "name" ;
    rdfs:comment "\\[ZBEX\\] The name of the setting." ;
    rdfs:domain cim:RelaySetting ;
    rdfs:range xsd:string .

cim:RelaySetting.unitSymbol a rdf:Property ;
    rdfs:label "unitSymbol" ;
    rdfs:comment "\\[ZBEX\\] The unit of the value." ;
    rdfs:domain cim:RelaySetting ;
    rdfs:range cim:UnitSymbol .

cim:RelaySetting.value a rdf:Property ;
    rdfs:label "value" ;
    rdfs:comment "\\[ZBEX\\] The value of the setting, e.g voltage, current, etc." ;
    rdfs:domain cim:RelaySetting ;
    rdfs:range xsd:double .

cim:RemoteControl.Control a rdf:Property ;
    rdfs:label "RemoteControl.Control" ;
    rdfs:comment "The remote point controlling the physical actuator. The Control for the RemoteControl point." ;
    rdfs:domain cim:RemoteControl ;
    rdfs:range cim:Control ;
    profile:sourceCardinality "0..1" ;
    profile:targetCardinality "0..1" .

cim:RemoteSource.Measurement a rdf:Property ;
    rdfs:label "RemoteSource.Measurement" ;
    rdfs:comment "The remote point taking the measurement. The Measurement for the RemoteSource point." ;
    rdfs:domain cim:RemoteSource ;
    rdfs:range cim:Measurement ;
    profile:sourceCardinality "0..1" ;
    profile:targetCardinality "0..1" .

cim:Resistance.value a rdf:Property ;
    rdfs:label "value" ;
    rdfs:comment "ohms (ohm)" ;
    rdfs:domain cim:Resistance ;
    rdfs:range xsd:double .

cim:ResistancePerLength.value a rdf:Property ;
    rdfs:label "value" ;
    rdfs:comment "ohms per metre (ohmPerm)" ;
    rdfs:domain cim:ResistancePerLength ;
    rdfs:range xsd:double .

cim:RotatingMachine.p a rdf:Property ;
    rdfs:label "p" ;
    rdfs:comment "Active power injection in watts. Load sign convention is used, i.e. positive sign means flow out from a node. Starting value for a steady state solution." ;
    rdfs:domain cim:RotatingMachine ;
    rdfs:range cim:ActivePower .

cim:RotatingMachine.q a rdf:Property ;
    rdfs:label "q" ;
    rdfs:comment "Reactive power injection in VAr. Load sign convention is used, i.e. positive sign means flow out from a node. Starting value for a steady state solution." ;
    rdfs:domain cim:RotatingMachine ;
    rdfs:range cim:ReactivePower .

cim:RotatingMachine.ratedPowerFactor a rdf:Property ;
    rdfs:label "ratedPowerFactor" ;
    rdfs:comment "Power factor (nameplate data). It is primarily used for short circuit data exchange according to IEC 60909. The attribute cannot be a negative value." ;
    rdfs:domain cim:RotatingMachine ;
    rdfs:range xsd:double .

cim:RotatingMachine.ratedS a rdf:Property ;
    rdfs:label "ratedS" ;
    rdfs:comment "Nameplate apparent power rating for the unit in volt-amperes (VA). The attribute shall have a positive value." ;
    rdfs:domain cim:RotatingMachine ;
    rdfs:range cim:ApparentPower .

cim:RotatingMachine.ratedU a rdf:Property ;
    rdfs:label "ratedU" ;
    rdfs:comment "Rated voltage in volts (nameplate data, Ur in IEC 60909-0). It is primarily used for short circuit data exchange according to IEC 60909. The attribute shall be a positive value." ;
    rdfs:domain cim:RotatingMachine ;
    rdfs:range cim:Voltage .

cim:SVCControlMode.reactivePower a rdf:Property ;
    rdfs:label "reactivePower" ;
    rdfs:comment "Reactive power control." ;
    rdfs:domain cim:SVCControlMode ;
    rdfs:range xsd:string .

cim:SVCControlMode.unknown a rdf:Property ;
    rdfs:label "unknown" ;
    rdfs:comment "unknown control." ;
    rdfs:domain cim:SVCControlMode ;
    rdfs:range xsd:string .

cim:SVCControlMode.voltage a rdf:Property ;
    rdfs:label "voltage" ;
    rdfs:comment "Voltage control." ;
    rdfs:domain cim:SVCControlMode ;
    rdfs:range xsd:string .

cim:Seconds.value a rdf:Property ;
    rdfs:label "value" ;
    rdfs:comment "Time, in seconds" ;
    rdfs:domain cim:Seconds ;
    rdfs:range xsd:double .

cim:Sensor.RelayFunction a rdf:Property ;
    rdfs:label "Sensor.RelayFunction" ;
    rdfs:comment "\\[ZBEX\\] The relay functions influenced by this Sensor." ;
    rdfs:domain cim:Sensor ;
    rdfs:range cim:RelayFunction ;
    profile:targetCardinality "0..*" .

cim:SeriesCompensator.r a rdf:Property ;
    rdfs:label "r" ;
    rdfs:comment "Positive sequence resistance." ;
    rdfs:domain cim:SeriesCompensator ;
    rdfs:range cim:Resistance .

cim:SeriesCompensator.r0 a rdf:Property ;
    rdfs:label "r0" ;
    rdfs:comment "Zero sequence resistance." ;
    rdfs:domain cim:SeriesCompensator ;
    rdfs:range cim:Resistance .

cim:SeriesCompensator.varistorRatedCurrent a rdf:Property ;
    rdfs:label "varistorRatedCurrent" ;
    rdfs:comment "The maximum current the varistor is designed to handle at specified duration. It is used for short circuit calculations and exchanged only if SeriesCompensator.varistorPresent is true.\nThe attribute shall be a positive value." ;
    rdfs:domain cim:SeriesCompensator ;
    rdfs:range cim:CurrentFlow .

cim:SeriesCompensator.varistorVoltageThreshold a rdf:Property ;
    rdfs:label "varistorVoltageThreshold" ;
    rdfs:comment "The dc voltage at which the varistor starts conducting. It is used for short circuit calculations and exchanged only if SeriesCompensator.varistorPresent is true." ;
    rdfs:domain cim:SeriesCompensator ;
    rdfs:range cim:Voltage .

cim:SeriesCompensator.x a rdf:Property ;
    rdfs:label "x" ;
    rdfs:comment "Positive sequence reactance." ;
    rdfs:domain cim:SeriesCompensator ;
    rdfs:range cim:Reactance .

cim:SeriesCompensator.x0 a rdf:Property ;
    rdfs:label "x0" ;
    rdfs:comment "Zero sequence reactance." ;
    rdfs:domain cim:SeriesCompensator ;
    rdfs:range cim:Reactance .

cim:ShortCircuitTest.current a rdf:Property ;
    rdfs:label "current" ;
    rdfs:comment "Short circuit current.." ;
    rdfs:domain cim:ShortCircuitTest ;
    rdfs:range cim:CurrentFlow .

cim:ShortCircuitTest.energisedEndStep a rdf:Property ;
    rdfs:label "energisedEndStep" ;
    rdfs:comment "Tap step number for the energised end of the test pair." ;
    rdfs:domain cim:ShortCircuitTest ;
    rdfs:range xsd:int .

cim:ShortCircuitTest.groundedEndStep a rdf:Property ;
    rdfs:label "groundedEndStep" ;
    rdfs:comment "Tap step number for the grounded end of the test pair." ;
    rdfs:domain cim:ShortCircuitTest ;
    rdfs:range xsd:int .

cim:ShortCircuitTest.leakageImpedance a rdf:Property ;
    rdfs:label "leakageImpedance" ;
    rdfs:comment "Leakage impedance measured from a positive-sequence or single-phase short-circuit test." ;
    rdfs:domain cim:ShortCircuitTest ;
    rdfs:range cim:Impedance .

cim:ShortCircuitTest.leakageImpedanceZero a rdf:Property ;
    rdfs:label "leakageImpedanceZero" ;
    rdfs:comment "Leakage impedance measured from a zero-sequence short-circuit test." ;
    rdfs:domain cim:ShortCircuitTest ;
    rdfs:range cim:Impedance .

cim:ShortCircuitTest.loss a rdf:Property ;
    rdfs:label "loss" ;
    rdfs:comment "Load losses from a positive-sequence or single-phase short-circuit test." ;
    rdfs:domain cim:ShortCircuitTest ;
    rdfs:range cim:ActivePower .

cim:ShortCircuitTest.lossZero a rdf:Property ;
    rdfs:label "lossZero" ;
    rdfs:comment "Load losses from a zero-sequence short-circuit test." ;
    rdfs:domain cim:ShortCircuitTest ;
    rdfs:range cim:ActivePower .

cim:ShortCircuitTest.power a rdf:Property ;
    rdfs:label "power" ;
    rdfs:comment "Short circuit apparent power." ;
    rdfs:domain cim:ShortCircuitTest ;
    rdfs:range cim:ApparentPower .

cim:ShortCircuitTest.voltage a rdf:Property ;
    rdfs:label "voltage" ;
    rdfs:comment "Short circuit voltage.." ;
    rdfs:domain cim:ShortCircuitTest ;
    rdfs:range cim:PerCent .

cim:ShortCircuitTest.voltageOhmicPart a rdf:Property ;
    rdfs:label "voltageOhmicPart" ;
    rdfs:comment "Short Circuit Voltage  Ohmic Part." ;
    rdfs:domain cim:ShortCircuitTest ;
    rdfs:range cim:PerCent .

cim:ShuntCompensator.grounded a rdf:Property ;
    rdfs:label "grounded" ;
    rdfs:comment "Used for Yn and Zn connections. True if the neutral is solidly grounded." ;
    rdfs:domain cim:ShuntCompensator ;
    rdfs:range xsd:boolean .

cim:ShuntCompensator.nomU a rdf:Property ;
    rdfs:label "nomU" ;
    rdfs:comment "The voltage at which the nominal reactive power may be calculated. This should normally be within 10% of the voltage at which the capacitor is connected to the network." ;
    rdfs:domain cim:ShuntCompensator ;
    rdfs:range cim:Voltage .

cim:ShuntCompensator.phaseConnection a rdf:Property ;
    rdfs:label "phaseConnection" ;
    rdfs:comment "The type of phase connection, such as wye or delta." ;
    rdfs:domain cim:ShuntCompensator ;
    rdfs:range cim:PhaseShuntConnectionKind .

cim:ShuntCompensator.sections a rdf:Property ;
    rdfs:label "sections" ;
    rdfs:comment "Shunt compensator sections in use. Starting value for steady state solution. The attribute shall be a positive value or zero. Non integer values are allowed to support continuous variables. The reasons for continuous value are to support study cases where no discrete shunt compensators has yet been designed, a solutions where a narrow voltage band force the sections to oscillate or accommodate for a continuous solution as input. \nFor LinearShuntConpensator the value shall be between zero and ShuntCompensator.maximumSections. At value zero the shunt compensator conductance and admittance is zero. Linear interpolation of conductance and admittance between the previous and next integer section is applied in case of non-integer values.\nFor NonlinearShuntCompensator-s shall only be set to one of the NonlinearShuntCompenstorPoint.sectionNumber. There is no interpolation between NonlinearShuntCompenstorPoint-s." ;
    rdfs:domain cim:ShuntCompensator ;
    rdfs:range xsd:double .

cim:ShuntCompensatorInfo.maxPowerLoss a rdf:Property ;
    rdfs:label "maxPowerLoss" ;
    rdfs:comment "Maximum allowed apparent power loss." ;
    rdfs:domain cim:ShuntCompensatorInfo ;
    rdfs:range cim:ApparentPower .

cim:ShuntCompensatorInfo.ratedCurrent a rdf:Property ;
    rdfs:label "ratedCurrent" ;
    rdfs:comment "Rated current." ;
    rdfs:domain cim:ShuntCompensatorInfo ;
    rdfs:range cim:CurrentFlow .

cim:ShuntCompensatorInfo.ratedReactivePower a rdf:Property ;
    rdfs:label "ratedReactivePower" ;
    rdfs:comment "Rated reactive power." ;
    rdfs:domain cim:ShuntCompensatorInfo ;
    rdfs:range cim:ReactivePower .

cim:ShuntCompensatorInfo.ratedVoltage a rdf:Property ;
    rdfs:label "ratedVoltage" ;
    rdfs:comment "Rated voltage." ;
    rdfs:domain cim:ShuntCompensatorInfo ;
    rdfs:range cim:Voltage .

cim:SinglePhaseKind.A a rdf:Property ;
    rdfs:label "A" ;
    rdfs:comment "Phase A." ;
    rdfs:domain cim:SinglePhaseKind ;
    rdfs:range xsd:string .

cim:SinglePhaseKind.B a rdf:Property ;
    rdfs:label "B" ;
    rdfs:comment "Phase B." ;
    rdfs:domain cim:SinglePhaseKind ;
    rdfs:range xsd:string .

cim:SinglePhaseKind.C a rdf:Property ;
    rdfs:label "C" ;
    rdfs:comment "Phase C." ;
    rdfs:domain cim:SinglePhaseKind ;
    rdfs:range xsd:string .

cim:SinglePhaseKind.N a rdf:Property ;
    rdfs:label "N" ;
    rdfs:comment "Neutral." ;
    rdfs:domain cim:SinglePhaseKind ;
    rdfs:range xsd:string .

cim:SinglePhaseKind.NONE a rdf:Property ;
    rdfs:label "NONE" ;
    rdfs:comment "no phase specified." ;
    rdfs:domain cim:SinglePhaseKind ;
    rdfs:range xsd:string .

cim:SinglePhaseKind.X a rdf:Property ;
    rdfs:label "X" ;
    rdfs:comment "An unknown primary phase." ;
    rdfs:domain cim:SinglePhaseKind ;
    rdfs:range xsd:string .

cim:SinglePhaseKind.Y a rdf:Property ;
    rdfs:label "Y" ;
    rdfs:comment "An unknown primary phase." ;
    rdfs:domain cim:SinglePhaseKind ;
    rdfs:range xsd:string .

cim:SinglePhaseKind.s1 a rdf:Property ;
    rdfs:label "s1" ;
    rdfs:comment "Secondary phase 1." ;
    rdfs:domain cim:SinglePhaseKind ;
    rdfs:range xsd:string .

cim:SinglePhaseKind.s2 a rdf:Property ;
    rdfs:label "s2" ;
    rdfs:comment "Secondary phase 2." ;
    rdfs:domain cim:SinglePhaseKind ;
    rdfs:range xsd:string .

cim:StaticVarCompensator.capacitiveRating a rdf:Property ;
    rdfs:label "capacitiveRating" ;
    rdfs:comment "Capacitive reactance in Ohms at maximum capacitive reactive power.  Shall always be positive." ;
    rdfs:domain cim:StaticVarCompensator ;
    rdfs:range cim:Reactance .

cim:StaticVarCompensator.inductiveRating a rdf:Property ;
    rdfs:label "inductiveRating" ;
    rdfs:comment "Inductive reactance in Ohms at maximum inductive reactive power.  Shall always be negative." ;
    rdfs:domain cim:StaticVarCompensator ;
    rdfs:range cim:Reactance .

cim:StaticVarCompensator.q a rdf:Property ;
    rdfs:label "q" ;
    rdfs:comment "Reactive power injection in VAr. Load sign convention is used, i.e. positive sign means flow out from a node.\nStarting value for a steady state solution." ;
    rdfs:domain cim:StaticVarCompensator ;
    rdfs:range cim:ReactivePower .

cim:StaticVarCompensator.sVCControlMode a rdf:Property ;
    rdfs:label "sVCControlMode" ;
    rdfs:comment "SVC control mode." ;
    rdfs:domain cim:StaticVarCompensator ;
    rdfs:range cim:SVCControlMode .

cim:StaticVarCompensator.voltageSetPoint a rdf:Property ;
    rdfs:label "voltageSetPoint" ;
    rdfs:comment "The reactive power output of the SVC is proportional to the difference between the voltage at the regulated bus and the voltage set-point.  When the regulated bus voltage is equal to the voltage set-point, the reactive power output is zero. Must be in volts." ;
    rdfs:domain cim:StaticVarCompensator ;
    rdfs:range cim:Voltage .

cim:StreetAddress.Location a rdf:Property ;
    rdfs:label "StreetAddress.Location" ;
    rdfs:comment "Street address associated with this location. Location for this street address." ;
    rdfs:domain cim:StreetAddress ;
    rdfs:range cim:Location ;
    profile:sourceCardinality "0..1" ;
    profile:targetCardinality "0..1" .

cim:StreetAddress.poBox a rdf:Property ;
    rdfs:label "poBox" ;
    rdfs:comment "Post office box." ;
    rdfs:domain cim:StreetAddress ;
    rdfs:range xsd:string .

cim:StreetAddress.postalCode a rdf:Property ;
    rdfs:label "postalCode" ;
    rdfs:comment "Postal code for the address." ;
    rdfs:domain cim:StreetAddress ;
    rdfs:range xsd:string .

cim:StreetAddress.streetDetail a rdf:Property ;
    rdfs:label "streetDetail" ;
    rdfs:comment "Street detail." ;
    rdfs:domain cim:StreetAddress ;
    rdfs:range cim:StreetDetail .

cim:StreetAddress.townDetail a rdf:Property ;
    rdfs:label "townDetail" ;
    rdfs:comment "Town detail." ;
    rdfs:domain cim:StreetAddress ;
    rdfs:range cim:TownDetail .

cim:StreetDetail.StreetAddress a rdf:Property ;
    rdfs:label "StreetDetail.StreetAddress" ;
    rdfs:comment "Street details that belong to this street address. Street address that owns this street detail." ;
    rdfs:domain cim:StreetDetail ;
    rdfs:range cim:StreetAddress ;
    profile:sourceCardinality "0..*" ;
    profile:targetCardinality "0..1" .

cim:StreetDetail.buildingName a rdf:Property ;
    rdfs:label "buildingName" ;
    rdfs:comment "(if applicable) In certain cases the physical location of the place of interest does not have a direct point of entry from the street, but may be located inside a larger structure such as a building, complex, office block, apartment, etc." ;
    rdfs:domain cim:StreetDetail ;
    rdfs:range xsd:string .

cim:StreetDetail.buildingNumber a rdf:Property ;
    rdfs:label "buildingNumber" ;
    rdfs:comment "\\[ZBEX\\] The number of the building." ;
    rdfs:domain cim:StreetDetail ;
    rdfs:range xsd:string .

cim:StreetDetail.displayAddress a rdf:Property ;
    rdfs:label "displayAddress" ;
    rdfs:comment "The address as it should be displayed to a user." ;
    rdfs:domain cim:StreetDetail ;
    rdfs:range xsd:string .

cim:StreetDetail.floorIdentification a rdf:Property ;
    rdfs:label "floorIdentification" ;
    rdfs:comment "The identification by name or number, expressed as text, of the floor in the building as part of this address." ;
    rdfs:domain cim:StreetDetail ;
    rdfs:range xsd:string .

cim:StreetDetail.name a rdf:Property ;
    rdfs:label "name" ;
    rdfs:comment "Name of the street." ;
    rdfs:domain cim:StreetDetail ;
    rdfs:range xsd:string .

cim:StreetDetail.number a rdf:Property ;
    rdfs:label "number" ;
    rdfs:comment "Designator of the specific location on the street." ;
    rdfs:domain cim:StreetDetail ;
    rdfs:range xsd:string .

cim:StreetDetail.suiteNumber a rdf:Property ;
    rdfs:label "suiteNumber" ;
    rdfs:comment "Number of the apartment or suite." ;
    rdfs:domain cim:StreetDetail ;
    rdfs:range xsd:string .

cim:StreetDetail.type a rdf:Property ;
    rdfs:label "type" ;
    rdfs:comment "Type of street. Examples include: street, circle, boulevard, avenue, road, drive, etc." ;
    rdfs:domain cim:StreetDetail ;
    rdfs:range xsd:string .

cim:Streetlight.Pole a rdf:Property ;
    rdfs:label "Streetlight.Pole" ;
    rdfs:comment "All streetlights attached to this pole. Pole to which thiss streetlight is attached." ;
    rdfs:domain cim:Streetlight ;
    rdfs:range cim:Pole ;
    profile:sourceCardinality "0..*" ;
    profile:targetCardinality "0..1" .

cim:Streetlight.lampKind a rdf:Property ;
    rdfs:label "lampKind" ;
    rdfs:comment "Lamp kind." ;
    rdfs:domain cim:Streetlight ;
    rdfs:range cim:StreetlightLampKind .

cim:Streetlight.lightRating a rdf:Property ;
    rdfs:label "lightRating" ;
    rdfs:comment "Power rating of light." ;
    rdfs:domain cim:Streetlight ;
    rdfs:range cim:ActivePower .

cim:StreetlightLampKind.HIGH_PRESSURE_SODIUM a rdf:Property ;
    rdfs:label "HIGH_PRESSURE_SODIUM" ;
    rdfs:comment "" ;
    rdfs:domain cim:StreetlightLampKind ;
    rdfs:range xsd:string .

cim:StreetlightLampKind.MERCURY_VAPOR a rdf:Property ;
    rdfs:label "MERCURY_VAPOR" ;
    rdfs:comment "" ;
    rdfs:domain cim:StreetlightLampKind ;
    rdfs:range xsd:string .

cim:StreetlightLampKind.METAL_HALIDE a rdf:Property ;
    rdfs:label "METAL_HALIDE" ;
    rdfs:comment "" ;
    rdfs:domain cim:StreetlightLampKind ;
    rdfs:range xsd:string .

cim:StreetlightLampKind.OTHER a rdf:Property ;
    rdfs:label "OTHER" ;
    rdfs:comment "" ;
    rdfs:domain cim:StreetlightLampKind ;
    rdfs:range xsd:string .

cim:StreetlightLampKind.UNKNOWN a rdf:Property ;
    rdfs:label "UNKNOWN" ;
    rdfs:comment "" ;
    rdfs:domain cim:StreetlightLampKind ;
    rdfs:range xsd:string .

cim:SubGeographicalRegion.GeographicalRegion a rdf:Property ;
    rdfs:label "SubGeographicalRegion.GeographicalRegion" ;
    rdfs:comment "All sub-geographical regions within this geographical region. The geographical region which this sub-geographical region is within." ;
    rdfs:domain cim:SubGeographicalRegion ;
    rdfs:range cim:GeographicalRegion ;
    profile:sourceCardinality "0..*" ;
    profile:targetCardinality "0..1" .

cim:SubGeographicalRegion.Substation a rdf:Property ;
    rdfs:label "SubGeographicalRegion.Substation" ;
    rdfs:comment "The SubGeographicalRegion containing the substation. The substations in this sub-geographical region." ;
    rdfs:domain cim:SubGeographicalRegion ;
    rdfs:range cim:Substation ;
    profile:sourceCardinality "0..1" ;
    profile:targetCardinality "0..*" .

cim:Substation.Circuit a rdf:Property ;
    rdfs:label "Substation.Circuit" ;
    rdfs:comment "Simplification of the CIM association via Bay to Circuit Simplification of the CIM association via Bay to Substation" ;
    rdfs:domain cim:Substation ;
    rdfs:range cim:Circuit ;
    profile:sourceCardinality "0..*" ;
    profile:targetCardinality "0..*" .

cim:Substation.Feeder a rdf:Property ;
    rdfs:label "Substation.Feeder" ;
    rdfs:comment "The substations that are normally energized by the feeder. The feeders that potentially energize  the downstream substation.  Should be consistent with the associations that describe the naming hierarchy." ;
    rdfs:domain cim:Substation ;
    rdfs:range cim:Feeder ;
    profile:sourceCardinality "0..1" ;
    profile:targetCardinality "0..*" .

cim:Substation.Loop a rdf:Property ;
    rdfs:label "Substation.Loop" ;
    rdfs:comment "Substation.Loop" ;
    rdfs:domain cim:Substation ;
    rdfs:range cim:Loop ;
    profile:sourceCardinality "0..*" .

cim:Substation.Loop a rdf:Property ;
    rdfs:label "Substation.Loop" ;
    rdfs:comment "The substations that normally energize this loop. The loops that are energized by this substation." ;
    rdfs:domain cim:Substation ;
    rdfs:range cim:Loop ;
    profile:sourceCardinality "0..*" .

cim:Substation.SubGeographicalRegion a rdf:Property ;
    rdfs:label "Substation.SubGeographicalRegion" ;
    rdfs:comment "The substations in this sub-geographical region. The SubGeographicalRegion containing the substation." ;
    rdfs:domain cim:Substation ;
    rdfs:range cim:SubGeographicalRegion ;
    profile:sourceCardinality "0..*" ;
    profile:targetCardinality "0..1" .

cim:Susceptance.value a rdf:Property ;
    rdfs:label "value" ;
    rdfs:comment "siemens (S)" ;
    rdfs:domain cim:Susceptance ;
    rdfs:range xsd:double .

cim:SusceptancePerLength.value a rdf:Property ;
    rdfs:label "value" ;
    rdfs:comment "siemens per metre (SPerm)" ;
    rdfs:domain cim:SusceptancePerLength ;
    rdfs:range xsd:double .

cim:Switch.normalOpen a rdf:Property ;
    rdfs:label "normalOpen" ;
    rdfs:comment "The attribute is used in cases when no Measurement for the status value is present. If the Switch has a status measurement the Discrete.normalValue is expected to match with the Switch.normalOpen." ;
    rdfs:domain cim:Switch ;
    rdfs:range xsd:boolean .

cim:Switch.open a rdf:Property ;
    rdfs:label "open" ;
    rdfs:comment "The attribute tells if the switch is considered open when used as input to topology processing." ;
    rdfs:domain cim:Switch ;
    rdfs:range xsd:boolean .

cim:Switch.ratedCurrent a rdf:Property ;
    rdfs:label "ratedCurrent" ;
    rdfs:comment "The maximum continuous current carrying capacity in amps governed by the device material and construction. The attribute shall be a positive value." ;
    rdfs:domain cim:Switch ;
    rdfs:range cim:CurrentFlow .

cim:SwitchInfo.ratedInterruptingTime a rdf:Property ;
    rdfs:label "ratedInterruptingTime" ;
    rdfs:comment "Switch rated interrupting time in seconds." ;
    rdfs:domain cim:SwitchInfo ;
    rdfs:range cim:Seconds .

cim:SynchronousMachine.ReactiveCapabilityCurve a rdf:Property ;
    rdfs:label "SynchronousMachine.ReactiveCapabilityCurve" ;
    rdfs:comment "The available reactive capability curves for this synchronous machine. The first shall be the default for this SynchronousMachine. Reactive power rating envelope versus the synchronous machine's active power, in both the generating and motoring modes. For each active power value there is a corresponding high and low reactive power limit value. Typically there will be a separate curve for each coolant condition, such as hydrogen pressure. The Y1 axis values represent reactive minimum and the Y2 axis values represent reactive maximum." ;
    rdfs:domain cim:SynchronousMachine ;
    rdfs:range cim:ReactiveCapabilityCurve ;
    profile:sourceCardinality "0..1" ;
    profile:targetCardinality "0..*" .

cim:SynchronousMachine.baseQ a rdf:Property ;
    rdfs:label "baseQ" ;
    rdfs:comment "Default base reactive power value in VAr. This value represents the initial reactive power that can be used by any application function." ;
    rdfs:domain cim:SynchronousMachine ;
    rdfs:range cim:ReactivePower .

cim:SynchronousMachine.condenserP a rdf:Property ;
    rdfs:label "condenserP" ;
    rdfs:comment "Active power consumed (watts) when in condenser mode operation." ;
    rdfs:domain cim:SynchronousMachine ;
    rdfs:range cim:ActivePower .

cim:SynchronousMachine.earthing a rdf:Property ;
    rdfs:label "earthing" ;
    rdfs:comment "Indicates whether or not the generator is earthed. Used for short circuit data exchange according to IEC 60909." ;
    rdfs:domain cim:SynchronousMachine ;
    rdfs:range xsd:boolean .

cim:SynchronousMachine.earthingStarPointR a rdf:Property ;
    rdfs:label "earthingStarPointR" ;
    rdfs:comment "Generator star point earthing resistance in Ohms (Re). Used for short circuit data exchange according to IEC 60909." ;
    rdfs:domain cim:SynchronousMachine ;
    rdfs:range cim:Resistance .

cim:SynchronousMachine.earthingStarPointX a rdf:Property ;
    rdfs:label "earthingStarPointX" ;
    rdfs:comment "Generator star point earthing reactance in Ohms (Xe). Used for short circuit data exchange according to IEC 60909." ;
    rdfs:domain cim:SynchronousMachine ;
    rdfs:range cim:Reactance .

cim:SynchronousMachine.ikk a rdf:Property ;
    rdfs:label "ikk" ;
    rdfs:comment "Steady-state short-circuit current (in A for the profile) of generator with compound excitation during 3-phase short circuit. - Ikk=0: Generator with no compound excitation. - Ikk<>0: Generator with compound excitation. Ikk is used to calculate the minimum steady-state short-circuit current for generators with compound excitation. (4.6.1.2 in IEC 60909-0:2001). Used only for single fed short circuit on a generator. (4.3.4.2. in IEC 60909-0:2001)." ;
    rdfs:domain cim:SynchronousMachine ;
    rdfs:range cim:CurrentFlow .

cim:SynchronousMachine.maxQ a rdf:Property ;
    rdfs:label "maxQ" ;
    rdfs:comment "Maximum reactive power limit in VAr. This is the maximum (nameplate) limit for the unit." ;
    rdfs:domain cim:SynchronousMachine ;
    rdfs:range cim:ReactivePower .

cim:SynchronousMachine.maxU a rdf:Property ;
    rdfs:label "maxU" ;
    rdfs:comment "Maximum voltage limit for the unit in volts." ;
    rdfs:domain cim:SynchronousMachine ;
    rdfs:range cim:Voltage .

cim:SynchronousMachine.minQ a rdf:Property ;
    rdfs:label "minQ" ;
    rdfs:comment "Minimum reactive power limit for the unit in VAr." ;
    rdfs:domain cim:SynchronousMachine ;
    rdfs:range cim:ReactivePower .

cim:SynchronousMachine.minU a rdf:Property ;
    rdfs:label "minU" ;
    rdfs:comment "Minimum voltage limit for the unit in volts." ;
    rdfs:domain cim:SynchronousMachine ;
    rdfs:range cim:Voltage .

cim:SynchronousMachine.mu a rdf:Property ;
    rdfs:label "mu" ;
    rdfs:comment "Factor to calculate the breaking current (Section 4.5.2.1 in IEC 60909-0). Used only for single fed short circuit on a generator (Section 4.3.4.2. in IEC 60909-0)." ;
    rdfs:domain cim:SynchronousMachine ;
    rdfs:range xsd:double .

cim:SynchronousMachine.operatingMode a rdf:Property ;
    rdfs:label "operatingMode" ;
    rdfs:comment "Current mode of operation." ;
    rdfs:domain cim:SynchronousMachine ;
    rdfs:range cim:SynchronousMachineKind .

cim:SynchronousMachine.r a rdf:Property ;
    rdfs:label "r" ;
    rdfs:comment "Equivalent resistance (RG) of generator as a percentage. RG is considered for the calculation of all currents, except for the calculation of the peak current ip. Used for short circuit data exchange according to IEC 60909." ;
    rdfs:domain cim:SynchronousMachine ;
    rdfs:range cim:Resistance .

cim:SynchronousMachine.r0 a rdf:Property ;
    rdfs:label "r0" ;
    rdfs:comment "Zero sequence resistance of the synchronous machine as a percentage." ;
    rdfs:domain cim:SynchronousMachine ;
    rdfs:range cim:Resistance .

cim:SynchronousMachine.r2 a rdf:Property ;
    rdfs:label "r2" ;
    rdfs:comment "Negative sequence resistance as a percentage." ;
    rdfs:domain cim:SynchronousMachine ;
    rdfs:range cim:Resistance .

cim:SynchronousMachine.satDirectSubtransX a rdf:Property ;
    rdfs:label "satDirectSubtransX" ;
    rdfs:comment "Direct-axis subtransient reactance saturated as a percentage, also known as Xd\"sat." ;
    rdfs:domain cim:SynchronousMachine ;
    rdfs:range cim:PU .

cim:SynchronousMachine.satDirectSyncX a rdf:Property ;
    rdfs:label "satDirectSyncX" ;
    rdfs:comment "Direct-axes saturated synchronous reactance (xdsat); reciprocal of short-circuit ration, as a percentage. Used for short circuit data exchange, only for single fed short circuit on a generator. (4.3.4.2. in IEC 60909-0:2001)." ;
    rdfs:domain cim:SynchronousMachine ;
    rdfs:range cim:PU .

cim:SynchronousMachine.satDirectTransX a rdf:Property ;
    rdfs:label "satDirectTransX" ;
    rdfs:comment "Saturated Direct-axis transient reactance as a percentage. The attribute is primarily used for short circuit calculations according to ANSI." ;
    rdfs:domain cim:SynchronousMachine ;
    rdfs:range cim:PU .

cim:SynchronousMachine.type a rdf:Property ;
    rdfs:label "type" ;
    rdfs:comment "Modes that this synchronous machine can operate in." ;
    rdfs:domain cim:SynchronousMachine ;
    rdfs:range cim:SynchronousMachineKind .

cim:SynchronousMachine.x0 a rdf:Property ;
    rdfs:label "x0" ;
    rdfs:comment "Zero sequence reactance of the synchronous machine as a percentage." ;
    rdfs:domain cim:SynchronousMachine ;
    rdfs:range cim:Reactance .

cim:SynchronousMachine.x2 a rdf:Property ;
    rdfs:label "x2" ;
    rdfs:comment "Negative sequence reactance as a percentage." ;
    rdfs:domain cim:SynchronousMachine ;
    rdfs:range cim:Reactance .

cim:SynchronousMachineKind.UNKNOWN a rdf:Property ;
    rdfs:label "UNKNOWN" ;
    rdfs:comment "Indicates how the synchronous machine is operated is unknown." ;
    rdfs:domain cim:SynchronousMachineKind ;
    rdfs:range xsd:string .

cim:SynchronousMachineKind.condenser a rdf:Property ;
    rdfs:label "condenser" ;
    rdfs:comment "Indicates the synchronous machine can operate as a condenser." ;
    rdfs:domain cim:SynchronousMachineKind ;
    rdfs:range xsd:string .

cim:SynchronousMachineKind.generator a rdf:Property ;
    rdfs:label "generator" ;
    rdfs:comment "Indicates the synchronous machine can operate as a generator." ;
    rdfs:domain cim:SynchronousMachineKind ;
    rdfs:range xsd:string .

cim:SynchronousMachineKind.generatorOrCondenser a rdf:Property ;
    rdfs:label "generatorOrCondenser" ;
    rdfs:comment "Indicates the synchronous machine can operate as a generator or as a condenser." ;
    rdfs:domain cim:SynchronousMachineKind ;
    rdfs:range xsd:string .

cim:SynchronousMachineKind.generatorOrCondenserOrMotor a rdf:Property ;
    rdfs:label "generatorOrCondenserOrMotor" ;
    rdfs:comment "Indicates the synchronous machine can operate as a generator or as a condenser or as a motor." ;
    rdfs:domain cim:SynchronousMachineKind ;
    rdfs:range xsd:string .

cim:SynchronousMachineKind.generatorOrMotor a rdf:Property ;
    rdfs:label "generatorOrMotor" ;
    rdfs:comment "Indicates the synchronous machine can operate as a generator or as a motor." ;
    rdfs:domain cim:SynchronousMachineKind ;
    rdfs:range xsd:string .

cim:SynchronousMachineKind.motor a rdf:Property ;
    rdfs:label "motor" ;
    rdfs:comment "Indicates the synchronous machine can operate as a motor." ;
    rdfs:domain cim:SynchronousMachineKind ;
    rdfs:range xsd:string .

cim:SynchronousMachineKind.motorOrCondenser a rdf:Property ;
    rdfs:label "motorOrCondenser" ;
    rdfs:comment "Indicates the synchronous machine can operate as a motor or as a condenser." ;
    rdfs:domain cim:SynchronousMachineKind ;
    rdfs:range xsd:string .

cim:TapChanger.TapChangerControl a rdf:Property ;
    rdfs:label "TapChanger.TapChangerControl" ;
    rdfs:comment "The regulating control scheme in which this tap changer participates." ;
    rdfs:domain cim:TapChanger ;
    rdfs:range cim:TapChangerControl ;
    profile:targetCardinality "0..1" .

cim:TapChanger.controlEnabled a rdf:Property ;
    rdfs:label "controlEnabled" ;
    rdfs:comment "Specifies the regulation status of the equipment.  True is regulating, false is not regulating." ;
    rdfs:domain cim:TapChanger ;
    rdfs:range xsd:boolean .

cim:TapChanger.highStep a rdf:Property ;
    rdfs:label "highStep" ;
    rdfs:comment "Highest possible tap step position, advance from neutral.\nThe attribute shall be greater than lowStep.\nThis tap position results in the maximum voltage boost on secondary winding(s)." ;
    rdfs:domain cim:TapChanger ;
    rdfs:range xsd:int .

cim:TapChanger.lowStep a rdf:Property ;
    rdfs:label "lowStep" ;
    rdfs:comment "Lowest possible tap step position, retard from neutral.\nThis tap position results in the maximum voltage buck on secondary winding(s)." ;
    rdfs:domain cim:TapChanger ;
    rdfs:range xsd:int .

cim:TapChanger.neutralStep a rdf:Property ;
    rdfs:label "neutralStep" ;
    rdfs:comment "The neutral tap step position for this winding.\nThe attribute shall be equal to or greater than lowStep and equal or less than highStep.\nIt is the step position where the voltage is neutralU when the other terminals of the transformer are at the ratedU.  If there are other tap changers on the transformer those taps are kept constant at their neutralStep." ;
    rdfs:domain cim:TapChanger ;
    rdfs:range xsd:int .

cim:TapChanger.neutralU a rdf:Property ;
    rdfs:label "neutralU" ;
    rdfs:comment "Voltage at which the winding operates at the neutral tap setting. It is the voltage at the terminal of the PowerTransformerEnd associated with the tap changer when all tap changers on the transformer are at their neutralStep position.  Normally neutralU of the tap changer is the same as ratedU of the PowerTransformerEnd, but it can differ in special cases such as when the tapping mechanism is separate from the winding more common on lower voltage transformers.\nThis attribute is not relevant for PhaseTapChangerAsymmetrical, PhaseTapChangerSymmetrical and PhaseTapChangerLinear." ;
    rdfs:domain cim:TapChanger ;
    rdfs:range cim:Voltage .

cim:TapChanger.normalStep a rdf:Property ;
    rdfs:label "normalStep" ;
    rdfs:comment "The tap step position used in \"normal\" network operation for this winding. For a \"Fixed\" tap changer indicates the current physical tap setting.\nThe attribute shall be equal to or greater than lowStep and equal to or less than highStep." ;
    rdfs:domain cim:TapChanger ;
    rdfs:range xsd:int .

cim:TapChanger.step a rdf:Property ;
    rdfs:label "step" ;
    rdfs:comment "Tap changer position.\nStarting step for a steady state solution. Non integer values are allowed to support continuous tap variables. The reasons for continuous value are to support study cases where no discrete tap changer has yet been designed, a solution where a narrow voltage band forces the tap step to oscillate or to accommodate for a continuous solution as input.\nThe attribute shall be equal to or greater than lowStep and equal to or less than highStep." ;
    rdfs:domain cim:TapChanger ;
    rdfs:range xsd:double .

cim:TapChangerControl.coGenerationEnabled a rdf:Property ;
    rdfs:label "coGenerationEnabled" ;
    rdfs:comment "True implies cogeneration mode is enabled and that the control will regulate to the new source bushing (downline bushing), keeping locations downline from experiencing overvoltage situations." ;
    rdfs:domain cim:TapChangerControl ;
    rdfs:range xsd:boolean .

cim:TapChangerControl.forwardLDCBlocking a rdf:Property ;
    rdfs:label "forwardLDCBlocking" ;
    rdfs:comment "True implies this tap changer turns off/ignores reverse current flows for line drop compensation when power flow is reversed and no reverse line drop is set." ;
    rdfs:domain cim:TapChangerControl ;
    rdfs:range xsd:boolean .

cim:TapChangerControl.limitVoltage a rdf:Property ;
    rdfs:label "limitVoltage" ;
    rdfs:comment "Maximum allowed regulated voltage on the PT secondary, regardless of line drop compensation. Sometimes referred to as first-house protection." ;
    rdfs:domain cim:TapChangerControl ;
    rdfs:range cim:Voltage .

cim:TapChangerControl.lineDropCompensation a rdf:Property ;
    rdfs:label "lineDropCompensation" ;
    rdfs:comment "If true, the line drop compensation is to be applied." ;
    rdfs:domain cim:TapChangerControl ;
    rdfs:range xsd:boolean .

cim:TapChangerControl.lineDropR a rdf:Property ;
    rdfs:label "lineDropR" ;
    rdfs:comment "Line drop compensator resistance setting for normal (forward) power flow." ;
    rdfs:domain cim:TapChangerControl ;
    rdfs:range cim:Resistance .

cim:TapChangerControl.lineDropX a rdf:Property ;
    rdfs:label "lineDropX" ;
    rdfs:comment "Line drop compensator reactance setting for normal (forward) power flow." ;
    rdfs:domain cim:TapChangerControl ;
    rdfs:range cim:Reactance .

cim:TapChangerControl.reverseLineDropR a rdf:Property ;
    rdfs:label "reverseLineDropR" ;
    rdfs:comment "Line drop compensator resistance setting for reverse power flow." ;
    rdfs:domain cim:TapChangerControl ;
    rdfs:range cim:Resistance .

cim:TapChangerControl.reverseLineDropX a rdf:Property ;
    rdfs:label "reverseLineDropX" ;
    rdfs:comment "Line drop compensator reactance setting for reverse power flow." ;
    rdfs:domain cim:TapChangerControl ;
    rdfs:range cim:Reactance .

cim:TapChangerControl.timeDelay a rdf:Property ;
    rdfs:label "timeDelay" ;
    rdfs:comment "The time delay for the tap changer in seconds." ;
    rdfs:domain cim:TapChangerControl ;
    rdfs:range cim:Reactance .

cim:TelephoneNumber.areaCode a rdf:Property ;
    rdfs:label "areaCode" ;
    rdfs:comment "(if applicable) Area or region code." ;
    rdfs:domain cim:TelephoneNumber ;
    rdfs:range xsd:string .

cim:TelephoneNumber.cityCode a rdf:Property ;
    rdfs:label "cityCode" ;
    rdfs:comment "City code." ;
    rdfs:domain cim:TelephoneNumber ;
    rdfs:range xsd:string .

cim:TelephoneNumber.countryCode a rdf:Property ;
    rdfs:label "countryCode" ;
    rdfs:comment "Country code." ;
    rdfs:domain cim:TelephoneNumber ;
    rdfs:range xsd:string .

cim:TelephoneNumber.description a rdf:Property ;
    rdfs:label "description" ;
    rdfs:comment "[ZBEX] Description for phone number, e.g: home, work, mobile." ;
    rdfs:domain cim:TelephoneNumber ;
    rdfs:range xsd:string .

cim:TelephoneNumber.dialOut a rdf:Property ;
    rdfs:label "dialOut" ;
    rdfs:comment "(if applicable) Dial out code, for instance to call outside an enterprise." ;
    rdfs:domain cim:TelephoneNumber ;
    rdfs:range xsd:string .

cim:TelephoneNumber.extension a rdf:Property ;
    rdfs:label "extension" ;
    rdfs:comment "(if applicable) Extension for this telephone number." ;
    rdfs:domain cim:TelephoneNumber ;
    rdfs:range xsd:string .

cim:TelephoneNumber.internationalPrefix a rdf:Property ;
    rdfs:label "internationalPrefix" ;
    rdfs:comment "(if applicable) Prefix used when calling an international number." ;
    rdfs:domain cim:TelephoneNumber ;
    rdfs:range xsd:string .

cim:TelephoneNumber.isPrimary a rdf:Property ;
    rdfs:label "isPrimary" ;
    rdfs:comment "\\[ZBEX\\] Is this phone number the primary number for the contact?" ;
    rdfs:domain cim:TelephoneNumber ;
    rdfs:range xsd:boolean .

cim:TelephoneNumber.ituPhone a rdf:Property ;
    rdfs:label "ituPhone" ;
    rdfs:comment "Phone number according to ITU E.164." ;
    rdfs:domain cim:TelephoneNumber ;
    rdfs:range xsd:string .

cim:TelephoneNumber.localNumber a rdf:Property ;
    rdfs:label "localNumber" ;
    rdfs:comment "Main (local) part of this telephone number." ;
    rdfs:domain cim:TelephoneNumber ;
    rdfs:range xsd:string .

cim:Temperature.value a rdf:Property ;
    rdfs:label "value" ;
    rdfs:comment "degrees Celsius (degC)" ;
    rdfs:domain cim:Temperature ;
    rdfs:range xsd:double .

cim:Terminal.ConductingEquipment a rdf:Property ;
    rdfs:label "Terminal.ConductingEquipment" ;
    rdfs:comment "Conducting equipment have terminals that may be connected to other conducting equipment terminals via connectivity nodes or topological nodes. The conducting equipment of the terminal.  Conducting equipment have  terminals that may be connected to other conducting equipment terminals via connectivity nodes or topological nodes." ;
    rdfs:domain cim:Terminal ;
    rdfs:range cim:ConductingEquipment ;
    profile:sourceCardinality "0..*" ;
    profile:targetCardinality "0..1" .

cim:Terminal.ConnectivityNode a rdf:Property ;
    rdfs:label "Terminal.ConnectivityNode" ;
    rdfs:comment "Terminals interconnected with zero impedance at a this connectivity node. The connectivity node to which this terminal connects with zero impedance." ;
    rdfs:domain cim:Terminal ;
    rdfs:range cim:ConnectivityNode ;
    profile:sourceCardinality "0..*" ;
    profile:targetCardinality "0..1" .

cim:Terminal.currentFeederDirection a rdf:Property ;
    rdfs:label "currentFeederDirection" ;
    rdfs:comment "Stores the direction of the feeder head relative to this terminal in the current state of the network." ;
    rdfs:domain cim:Terminal ;
    rdfs:range xsd:int .

cim:Terminal.currentPhases a rdf:Property ;
    rdfs:label "currentPhases" ;
    rdfs:comment "Represents the current network phasing condition. Mirrors the exported Terminal.currentPhases values." ;
    rdfs:domain cim:Terminal ;
    rdfs:range cim:PhaseCode .

cim:Terminal.normalFeederDirection a rdf:Property ;
    rdfs:label "normalFeederDirection" ;
    rdfs:comment "Stores the direction of the feeder head relative to this terminal in the normal state of the network." ;
    rdfs:domain cim:Terminal ;
    rdfs:range xsd:int .

cim:Terminal.normalPhases a rdf:Property ;
    rdfs:label "normalPhases" ;
    rdfs:comment "Represents the normal network phasing condition. Mirrors the exported Terminal.normalPhases values." ;
    rdfs:domain cim:Terminal ;
    rdfs:range cim:PhaseCode .

cim:Terminal.phases a rdf:Property ;
    rdfs:label "phases" ;
    rdfs:comment "Represents the normal network phasing condition." ;
    rdfs:domain cim:Terminal ;
    rdfs:range cim:PhaseCode .

cim:Terminal.sequenceNumber a rdf:Property ;
    rdfs:label "sequenceNumber" ;
    rdfs:comment "This Terminal's sequence number." ;
    rdfs:domain cim:Terminal ;
    rdfs:range xsd:int .

cim:Terminal.tracedPhases a rdf:Property ;
    rdfs:label "tracedPhases" ;
    rdfs:comment "The traced phase status:\n                |      uint32      |\n                | 16 bits |16 bits |\nNetwork status: | current | normal |\nNetwork state phase status:\n               |              16 bits              |\n               | 4 bits | 4 bits | 4 bits | 4 bits |\nNominal phase: |   N    |    C   | B/Y/s2 | A/X/s1 |\nEach nominal phase (actual phase):\n              |                 4 bits                |\n              |  1 bit  |  1 bit  |  1 bit  |  1 bit  |\nActual Phase: |    N    |    C    |    B    |    A    |\n" ;
    rdfs:domain cim:Terminal ;
    rdfs:range xsd:int .

cim:TownDetail.StreetAddress a rdf:Property ;
    rdfs:label "TownDetail.StreetAddress" ;
    rdfs:comment "Town details that belong to this street address. Street address that owns this town detail." ;
    rdfs:domain cim:TownDetail ;
    rdfs:range cim:StreetAddress ;
    profile:sourceCardinality "0..*" ;
    profile:targetCardinality "0..1" .

cim:TownDetail.country a rdf:Property ;
    rdfs:label "country" ;
    rdfs:comment "Name of the country." ;
    rdfs:domain cim:TownDetail ;
    rdfs:range xsd:string .

cim:TownDetail.name a rdf:Property ;
    rdfs:label "name" ;
    rdfs:comment "Town name." ;
    rdfs:domain cim:TownDetail ;
    rdfs:range xsd:string .

cim:TownDetail.stateOrProvince a rdf:Property ;
    rdfs:label "stateOrProvince" ;
    rdfs:comment "Name of the state or province." ;
    rdfs:domain cim:TownDetail ;
    rdfs:range xsd:string .

cim:TransformerConstructionKind.aerial a rdf:Property ;
    rdfs:label "aerial" ;
    rdfs:comment "" ;
    rdfs:domain cim:TransformerConstructionKind ;
    rdfs:range xsd:string .

cim:TransformerConstructionKind.dryType a rdf:Property ;
    rdfs:label "dryType" ;
    rdfs:comment "" ;
    rdfs:domain cim:TransformerConstructionKind ;
    rdfs:range xsd:string .

cim:TransformerConstructionKind.network a rdf:Property ;
    rdfs:label "network" ;
    rdfs:comment "" ;
    rdfs:domain cim:TransformerConstructionKind ;
    rdfs:range xsd:string .

cim:TransformerConstructionKind.onePhase a rdf:Property ;
    rdfs:label "onePhase" ;
    rdfs:comment "" ;
    rdfs:domain cim:TransformerConstructionKind ;
    rdfs:range xsd:string .

cim:TransformerConstructionKind.overhead a rdf:Property ;
    rdfs:label "overhead" ;
    rdfs:comment "" ;
    rdfs:domain cim:TransformerConstructionKind ;
    rdfs:range xsd:string .

cim:TransformerConstructionKind.padmountDeadFront a rdf:Property ;
    rdfs:label "padmountDeadFront" ;
    rdfs:comment "" ;
    rdfs:domain cim:TransformerConstructionKind ;
    rdfs:range xsd:string .

cim:TransformerConstructionKind.padmountFeedThrough a rdf:Property ;
    rdfs:label "padmountFeedThrough" ;
    rdfs:comment "" ;
    rdfs:domain cim:TransformerConstructionKind ;
    rdfs:range xsd:string .

cim:TransformerConstructionKind.padmountLiveFront a rdf:Property ;
    rdfs:label "padmountLiveFront" ;
    rdfs:comment "" ;
    rdfs:domain cim:TransformerConstructionKind ;
    rdfs:range xsd:string .

cim:TransformerConstructionKind.padmountLoopThrough a rdf:Property ;
    rdfs:label "padmountLoopThrough" ;
    rdfs:comment "" ;
    rdfs:domain cim:TransformerConstructionKind ;
    rdfs:range xsd:string .

cim:TransformerConstructionKind.padmounted a rdf:Property ;
    rdfs:label "padmounted" ;
    rdfs:comment "" ;
    rdfs:domain cim:TransformerConstructionKind ;
    rdfs:range xsd:string .

cim:TransformerConstructionKind.subway a rdf:Property ;
    rdfs:label "subway" ;
    rdfs:comment "" ;
    rdfs:domain cim:TransformerConstructionKind ;
    rdfs:range xsd:string .

cim:TransformerConstructionKind.threePhase a rdf:Property ;
    rdfs:label "threePhase" ;
    rdfs:comment "" ;
    rdfs:domain cim:TransformerConstructionKind ;
    rdfs:range xsd:string .

cim:TransformerConstructionKind.underground a rdf:Property ;
    rdfs:label "underground" ;
    rdfs:comment "" ;
    rdfs:domain cim:TransformerConstructionKind ;
    rdfs:range xsd:string .

cim:TransformerConstructionKind.unknown a rdf:Property ;
    rdfs:label "unknown" ;
    rdfs:comment "" ;
    rdfs:domain cim:TransformerConstructionKind ;
    rdfs:range xsd:string .

cim:TransformerConstructionKind.vault a rdf:Property ;
    rdfs:label "vault" ;
    rdfs:comment "" ;
    rdfs:domain cim:TransformerConstructionKind ;
    rdfs:range xsd:string .

cim:TransformerConstructionKind.vaultThreePhase a rdf:Property ;
    rdfs:label "vaultThreePhase" ;
    rdfs:comment "" ;
    rdfs:domain cim:TransformerConstructionKind ;
    rdfs:range xsd:string .

cim:TransformerCoolingType.KDAF a rdf:Property ;
    rdfs:label "KDAF" ;
    rdfs:comment "\\[ZBEX\\] Non-mineral oil directed, air forced" ;
    rdfs:domain cim:TransformerCoolingType ;
    rdfs:range xsd:string .

cim:TransformerCoolingType.KFAF a rdf:Property ;
    rdfs:label "KFAF" ;
    rdfs:comment "\\[ZBEX\\] Non-mineral oil forced, air forced" ;
    rdfs:domain cim:TransformerCoolingType ;
    rdfs:range xsd:string .

cim:TransformerCoolingType.KFWF a rdf:Property ;
    rdfs:label "KFWF" ;
    rdfs:comment "\\[ZBEX\\] Non-mineral oil forced, water forced" ;
    rdfs:domain cim:TransformerCoolingType ;
    rdfs:range xsd:string .

cim:TransformerCoolingType.KNAF a rdf:Property ;
    rdfs:label "KNAF" ;
    rdfs:comment "\\[ZBEX\\] Non-mineral oil natural, air forced" ;
    rdfs:domain cim:TransformerCoolingType ;
    rdfs:range xsd:string .

cim:TransformerCoolingType.KNAN a rdf:Property ;
    rdfs:label "KNAN" ;
    rdfs:comment "\\[ZBEX\\] Non-mineral oil natural, air natural" ;
    rdfs:domain cim:TransformerCoolingType ;
    rdfs:range xsd:string .

cim:TransformerCoolingType.ODAF a rdf:Property ;
    rdfs:label "ODAF" ;
    rdfs:comment "\\[ZBEX\\] Oil directed, air forced" ;
    rdfs:domain cim:TransformerCoolingType ;
    rdfs:range xsd:string .

cim:TransformerCoolingType.OFAF a rdf:Property ;
    rdfs:label "OFAF" ;
    rdfs:comment "\\[ZBEX\\] Oil forced, air forced" ;
    rdfs:domain cim:TransformerCoolingType ;
    rdfs:range xsd:string .

cim:TransformerCoolingType.OFWF a rdf:Property ;
    rdfs:label "OFWF" ;
    rdfs:comment "\\[ZBEX\\] Oil forced, water forced" ;
    rdfs:domain cim:TransformerCoolingType ;
    rdfs:range xsd:string .

cim:TransformerCoolingType.ONAF a rdf:Property ;
    rdfs:label "ONAF" ;
    rdfs:comment "\\[ZBEX\\] Oil natural, air forced" ;
    rdfs:domain cim:TransformerCoolingType ;
    rdfs:range xsd:string .

cim:TransformerCoolingType.ONAN a rdf:Property ;
    rdfs:label "ONAN" ;
    rdfs:comment "\\[ZBEX\\] Oil natural, air natural" ;
    rdfs:domain cim:TransformerCoolingType ;
    rdfs:range xsd:string .

cim:TransformerCoolingType.UNKNOWN_COOLING_TYPE a rdf:Property ;
    rdfs:label "UNKNOWN_COOLING_TYPE" ;
    rdfs:comment "\\[ZBEX\\] Default" ;
    rdfs:domain cim:TransformerCoolingType ;
    rdfs:range xsd:string .

cim:TransformerEnd.BaseVoltage a rdf:Property ;
    rdfs:label "TransformerEnd.BaseVoltage" ;
    rdfs:comment "Base voltage of the transformer end.  This is essential for PU calculation." ;
    rdfs:domain cim:TransformerEnd ;
    rdfs:range cim:BaseVoltage ;
    profile:targetCardinality "0..1" .

cim:TransformerEnd.RatioTapChanger a rdf:Property ;
    rdfs:label "TransformerEnd.RatioTapChanger" ;
    rdfs:comment "Transformer end to which this ratio tap changer belongs. Ratio tap changer associated with this transformer end." ;
    rdfs:domain cim:TransformerEnd ;
    rdfs:range cim:RatioTapChanger ;
    profile:sourceCardinality "0..1" ;
    profile:targetCardinality "0..1" .

cim:TransformerEnd.Terminal a rdf:Property ;
    rdfs:label "TransformerEnd.Terminal" ;
    rdfs:comment "Terminal of the power transformer to which this transformer end belongs." ;
    rdfs:domain cim:TransformerEnd ;
    rdfs:range cim:Terminal ;
    profile:targetCardinality "0..1" .

cim:TransformerEnd.TransformerStarImpedance a rdf:Property ;
    rdfs:label "TransformerEnd.TransformerStarImpedance" ;
    rdfs:comment "(accurate for 2- or 3-winding transformers only) Pi-model impedances of this transformer end. By convention, for a two winding transformer, the full values of the transformer should be entered on the high voltage end (endNumber=1)." ;
    rdfs:domain cim:TransformerEnd ;
    rdfs:range cim:TransformerStarImpedance ;
    profile:targetCardinality "0..1" .

cim:TransformerEnd.endNumber a rdf:Property ;
    rdfs:label "endNumber" ;
    rdfs:comment "Number for this transformer end, corresponding to the end's order in the power transformer vector group or phase angle clock number.  Highest voltage winding should be 1.  Each end within a power transformer should have a unique subsequent end number.   Note the transformer end number need not match the terminal sequence number." ;
    rdfs:domain cim:TransformerEnd ;
    rdfs:range xsd:int .

cim:TransformerEnd.grounded a rdf:Property ;
    rdfs:label "grounded" ;
    rdfs:comment "(for Yn and Zn connections) True if the neutral is solidly grounded." ;
    rdfs:domain cim:TransformerEnd ;
    rdfs:range xsd:boolean .

cim:TransformerEnd.rground a rdf:Property ;
    rdfs:label "rground" ;
    rdfs:comment "(for Yn and Zn connections) Resistance part of neutral impedance where 'grounded' is true." ;
    rdfs:domain cim:TransformerEnd ;
    rdfs:range cim:Resistance .

cim:TransformerEnd.xground a rdf:Property ;
    rdfs:label "xground" ;
    rdfs:comment "(for Yn and Zn connections) Reactive part of neutral impedance where 'grounded' is true." ;
    rdfs:domain cim:TransformerEnd ;
    rdfs:range cim:Reactance .

cim:TransformerEndInfo.NoLoadTest a rdf:Property ;
    rdfs:label "TransformerEndInfo.NoLoadTest" ;
    rdfs:comment "All no-load test measurements in which this transformer end was energised." ;
    rdfs:domain cim:TransformerEndInfo ;
    rdfs:range cim:NoLoadTest ;
    profile:targetCardinality "0..1" .

cim:TransformerEndInfo.OpenCircuitTest a rdf:Property ;
    rdfs:label "TransformerEndInfo.OpenCircuitTest" ;
    rdfs:comment "Transformer end measured for induced voltage and angle in this open-circuit test. All open-circuit test measurements in which this transformer end was not excited." ;
    rdfs:domain cim:TransformerEndInfo ;
    rdfs:range cim:OpenCircuitTest ;
    profile:sourceCardinality "0..1" ;
    profile:targetCardinality "0..1" .

cim:TransformerEndInfo.OpenCircuitTest a rdf:Property ;
    rdfs:label "TransformerEndInfo.OpenCircuitTest" ;
    rdfs:comment "All open-circuit test measurements in which this transformer end was excited." ;
    rdfs:domain cim:TransformerEndInfo ;
    rdfs:range cim:OpenCircuitTest ;
    profile:targetCardinality "0..1" .

cim:TransformerEndInfo.ShortCircuitTest a rdf:Property ;
    rdfs:label "TransformerEndInfo.ShortCircuitTest" ;
    rdfs:comment "All short-circuit test measurements in which this transformer end was short-circuited." ;
    rdfs:domain cim:TransformerEndInfo ;
    rdfs:range cim:ShortCircuitTest ;
    profile:targetCardinality "0..1" .

cim:TransformerEndInfo.ShortCircuitTest a rdf:Property ;
    rdfs:label "TransformerEndInfo.ShortCircuitTest" ;
    rdfs:comment "All short-circuit test measurements in which this transformer end was energised." ;
    rdfs:domain cim:TransformerEndInfo ;
    rdfs:range cim:ShortCircuitTest ;
    profile:targetCardinality "0..1" .

cim:TransformerEndInfo.TransformerStarImpedance a rdf:Property ;
    rdfs:label "TransformerEndInfo.TransformerStarImpedance" ;
    rdfs:comment "Transformer end datasheet used to calculate this transformer star impedance. Transformer star impedance calculated from this transformer end datasheet." ;
    rdfs:domain cim:TransformerEndInfo ;
    rdfs:range cim:TransformerStarImpedance ;
    profile:sourceCardinality "0..1" ;
    profile:targetCardinality "0..1" .

cim:TransformerEndInfo.TransformerTankInfo a rdf:Property ;
    rdfs:label "TransformerEndInfo.TransformerTankInfo" ;
    rdfs:comment "Transformer tank data that this end description is part of." ;
    rdfs:domain cim:TransformerEndInfo ;
    rdfs:range cim:TransformerTankInfo ;
    profile:targetCardinality "0..1" .

cim:TransformerEndInfo.connectionKind a rdf:Property ;
    rdfs:label "connectionKind" ;
    rdfs:comment "Kind of connection." ;
    rdfs:domain cim:TransformerEndInfo ;
    rdfs:range cim:WindingConnection .

cim:TransformerEndInfo.emergencyS a rdf:Property ;
    rdfs:label "emergencyS" ;
    rdfs:comment "Apparent power that the winding can carry under emergency conditions (also called long-term emergency power)." ;
    rdfs:domain cim:TransformerEndInfo ;
    rdfs:range cim:ApparentPower .

cim:TransformerEndInfo.endNumber a rdf:Property ;
    rdfs:label "endNumber" ;
    rdfs:comment "Number for this transformer end, corresponding to the end's order in the PowerTransformer.vectorGroup attribute. Highest voltage winding should be 1." ;
    rdfs:domain cim:TransformerEndInfo ;
    rdfs:range xsd:int .

cim:TransformerEndInfo.insulationU a rdf:Property ;
    rdfs:label "insulationU" ;
    rdfs:comment "Basic insulation level voltage rating." ;
    rdfs:domain cim:TransformerEndInfo ;
    rdfs:range cim:Voltage .

cim:TransformerEndInfo.phaseAngleClock a rdf:Property ;
    rdfs:label "phaseAngleClock" ;
    rdfs:comment "Winding phase angle where 360 degrees are represented with clock hours, so the valid values are {0, ..., 11}. For example, to express the second winding in code 'Dyn11', set attributes as follows: 'endNumber'=2, 'connectionKind' = Yn and 'phaseAngleClock' = 11." ;
    rdfs:domain cim:TransformerEndInfo ;
    rdfs:range xsd:int .

cim:TransformerEndInfo.r a rdf:Property ;
    rdfs:label "r" ;
    rdfs:comment "DC resistance." ;
    rdfs:domain cim:TransformerEndInfo ;
    rdfs:range cim:Resistance .

cim:TransformerEndInfo.ratedS a rdf:Property ;
    rdfs:label "ratedS" ;
    rdfs:comment "Normal apparent power rating." ;
    rdfs:domain cim:TransformerEndInfo ;
    rdfs:range cim:ApparentPower .

cim:TransformerEndInfo.ratedU a rdf:Property ;
    rdfs:label "ratedU" ;
    rdfs:comment "Rated voltage: phase-phase for three-phase windings, and either phase-phase or phase-neutral for single-phase windings." ;
    rdfs:domain cim:TransformerEndInfo ;
    rdfs:range cim:Voltage .

cim:TransformerEndInfo.shortTermS a rdf:Property ;
    rdfs:label "shortTermS" ;
    rdfs:comment "Apparent power that this winding can carry for a short period of time (in emergency)." ;
    rdfs:domain cim:TransformerEndInfo ;
    rdfs:range cim:ApparentPower .

cim:TransformerEndRatedS.coolingType a rdf:Property ;
    rdfs:label "coolingType" ;
    rdfs:comment "\\[ZBEX\\] The cooling type for this rating." ;
    rdfs:domain cim:TransformerEndRatedS ;
    rdfs:range cim:TransformerCoolingType .

cim:TransformerEndRatedS.ratedS a rdf:Property ;
    rdfs:label "ratedS" ;
    rdfs:comment "\\[ZBEX\\] The normal apparent power rating for this cooling type." ;
    rdfs:domain cim:TransformerEndRatedS ;
    rdfs:range cim:ApparentPower .

cim:TransformerFunctionKind.autotransformer a rdf:Property ;
    rdfs:label "autotransformer" ;
    rdfs:comment "A transformer with a special winding divided into several sections enabling the voltage to be varied at will. (IEC ref 811-26-04). (No available CIM definition, Zepben proposed definition)." ;
    rdfs:domain cim:TransformerFunctionKind ;
    rdfs:range xsd:string .

cim:TransformerFunctionKind.distributionTransformer a rdf:Property ;
    rdfs:label "distributionTransformer" ;
    rdfs:comment "A transformer that provides the final voltage transformation in the electric power distribution system. (No available CIM definition, Zepben proposed definition)." ;
    rdfs:domain cim:TransformerFunctionKind ;
    rdfs:range xsd:string .

cim:TransformerFunctionKind.isolationTransformer a rdf:Property ;
    rdfs:label "isolationTransformer" ;
    rdfs:comment "A transformer whose primary purpose is to isolate circuits. (No available CIM definition, Zepben proposed definition)." ;
    rdfs:domain cim:TransformerFunctionKind ;
    rdfs:range xsd:string .

cim:TransformerFunctionKind.other a rdf:Property ;
    rdfs:label "other" ;
    rdfs:comment "Another type of transformer. (No available CIM definition, Zepben proposed definition)." ;
    rdfs:domain cim:TransformerFunctionKind ;
    rdfs:range xsd:string .

cim:TransformerFunctionKind.powerTransformer a rdf:Property ;
    rdfs:label "powerTransformer" ;
    rdfs:comment "No available CIM definition" ;
    rdfs:domain cim:TransformerFunctionKind ;
    rdfs:range xsd:string .

cim:TransformerFunctionKind.secondaryTransformer a rdf:Property ;
    rdfs:label "secondaryTransformer" ;
    rdfs:comment "No available CIM definition" ;
    rdfs:domain cim:TransformerFunctionKind ;
    rdfs:range xsd:string .

cim:TransformerFunctionKind.voltageRegulator a rdf:Property ;
    rdfs:label "voltageRegulator" ;
    rdfs:comment "A transformer that changes the voltage magnitude at a certain point in the power system (No available CIM definition, Zepben proposed definition)." ;
    rdfs:domain cim:TransformerFunctionKind ;
    rdfs:range xsd:string .

cim:TransformerStarImpedance.TransformerEndInfo a rdf:Property ;
    rdfs:label "TransformerStarImpedance.TransformerEndInfo" ;
    rdfs:comment "Transformer star impedance calculated from this transformer end datasheet. Transformer end datasheet used to calculate this transformer star impedance." ;
    rdfs:domain cim:TransformerStarImpedance ;
    rdfs:range cim:TransformerEndInfo ;
    profile:sourceCardinality "0..1" ;
    profile:targetCardinality "0..1" .

cim:TransformerStarImpedance.r a rdf:Property ;
    rdfs:label "r" ;
    rdfs:comment "Resistance of the transformer end." ;
    rdfs:domain cim:TransformerStarImpedance ;
    rdfs:range cim:Resistance .

cim:TransformerStarImpedance.r0 a rdf:Property ;
    rdfs:label "r0" ;
    rdfs:comment "Zero sequence series resistance of the transformer end." ;
    rdfs:domain cim:TransformerStarImpedance ;
    rdfs:range cim:Resistance .

cim:TransformerStarImpedance.x a rdf:Property ;
    rdfs:label "x" ;
    rdfs:comment "Positive sequence series reactance of the transformer end." ;
    rdfs:domain cim:TransformerStarImpedance ;
    rdfs:range cim:Reactance .

cim:TransformerStarImpedance.x0 a rdf:Property ;
    rdfs:label "x0" ;
    rdfs:comment "Zero sequence series reactance of the transformer end." ;
    rdfs:domain cim:TransformerStarImpedance ;
    rdfs:range cim:Reactance .

cim:TransformerTankInfo.PowerTransformerInfo a rdf:Property ;
    rdfs:label "TransformerTankInfo.PowerTransformerInfo" ;
    rdfs:comment "Data for all the tanks described by this power transformer data. Power transformer data that this tank description is part of." ;
    rdfs:domain cim:TransformerTankInfo ;
    rdfs:range cim:PowerTransformerInfo ;
    profile:sourceCardinality "0..*" ;
    profile:targetCardinality "0..1" .

cim:TransformerTankInfo.TransformerEndInfo a rdf:Property ;
    rdfs:label "TransformerTankInfo.TransformerEndInfo" ;
    rdfs:comment "Transformer tank data that this end description is part of. Data for all the ends described by this transformer tank data." ;
    rdfs:domain cim:TransformerTankInfo ;
    rdfs:range cim:TransformerEndInfo ;
    profile:sourceCardinality "0..1" ;
    profile:targetCardinality "0..*" .

cim:TransformerTest.basePower a rdf:Property ;
    rdfs:label "basePower" ;
    rdfs:comment "Base power at which the tests are conducted, usually equal to the rateds of one of the involved transformer ends." ;
    rdfs:domain cim:TransformerTest ;
    rdfs:range cim:ApparentPower .

cim:TransformerTest.temperature a rdf:Property ;
    rdfs:label "temperature" ;
    rdfs:comment "Temperature at which the test is conducted." ;
    rdfs:domain cim:TransformerTest ;
    rdfs:range cim:Temperature .

cim:UnitSymbol.A a rdf:Property ;
    rdfs:label "A" ;
    rdfs:comment "Current in amperes." ;
    rdfs:domain cim:UnitSymbol ;
    rdfs:range xsd:string .

cim:UnitSymbol.A2 a rdf:Property ;
    rdfs:label "A2" ;
    rdfs:comment "Amperes squared (A)." ;
    rdfs:domain cim:UnitSymbol ;
    rdfs:range xsd:string .

cim:UnitSymbol.A2h a rdf:Property ;
    rdfs:label "A2h" ;
    rdfs:comment "Ampere-squared hour, ampere-squared hour." ;
    rdfs:domain cim:UnitSymbol ;
    rdfs:range xsd:string .

cim:UnitSymbol.A2s a rdf:Property ;
    rdfs:label "A2s" ;
    rdfs:comment "Ampere squared time in square amperes (As)." ;
    rdfs:domain cim:UnitSymbol ;
    rdfs:range xsd:string .

cim:UnitSymbol.APerA a rdf:Property ;
    rdfs:label "APerA" ;
    rdfs:comment "Current, ratio of amperages.   Note: Users may need to supply a prefix such as m to show rates such as mA/A." ;
    rdfs:domain cim:UnitSymbol ;
    rdfs:range xsd:string .

cim:UnitSymbol.APerm a rdf:Property ;
    rdfs:label "APerm" ;
    rdfs:comment "A/m, magnetic field strength, amperes per metre." ;
    rdfs:domain cim:UnitSymbol ;
    rdfs:range xsd:string .

cim:UnitSymbol.Ah a rdf:Property ;
    rdfs:label "Ah" ;
    rdfs:comment "Ampere-hours, ampere-hours." ;
    rdfs:domain cim:UnitSymbol ;
    rdfs:range xsd:string .

cim:UnitSymbol.As a rdf:Property ;
    rdfs:label "As" ;
    rdfs:comment "Ampere seconds (As)." ;
    rdfs:domain cim:UnitSymbol ;
    rdfs:range xsd:string .

cim:UnitSymbol.Bq a rdf:Property ;
    rdfs:label "Bq" ;
    rdfs:comment "Radioactivity in becquerels (1/s)." ;
    rdfs:domain cim:UnitSymbol ;
    rdfs:range xsd:string .

cim:UnitSymbol.Btu a rdf:Property ;
    rdfs:label "Btu" ;
    rdfs:comment "Energy, British Thermal Units." ;
    rdfs:domain cim:UnitSymbol ;
    rdfs:range xsd:string .

cim:UnitSymbol.C a rdf:Property ;
    rdfs:label "C" ;
    rdfs:comment "Electric charge in coulombs (As)." ;
    rdfs:domain cim:UnitSymbol ;
    rdfs:range xsd:string .

cim:UnitSymbol.CPerkg a rdf:Property ;
    rdfs:label "CPerkg" ;
    rdfs:comment "Exposure (x rays), coulombs per kilogram." ;
    rdfs:domain cim:UnitSymbol ;
    rdfs:range xsd:string .

cim:UnitSymbol.CPerm2 a rdf:Property ;
    rdfs:label "CPerm2" ;
    rdfs:comment "Surface charge density, coulombs per square metre." ;
    rdfs:domain cim:UnitSymbol ;
    rdfs:range xsd:string .

cim:UnitSymbol.CPerm3 a rdf:Property ;
    rdfs:label "CPerm3" ;
    rdfs:comment "Electric charge density, coulombs per cubic metre." ;
    rdfs:domain cim:UnitSymbol ;
    rdfs:range xsd:string .

cim:UnitSymbol.F a rdf:Property ;
    rdfs:label "F" ;
    rdfs:comment "Electric capacitance in farads (C/V)." ;
    rdfs:domain cim:UnitSymbol ;
    rdfs:range xsd:string .

cim:UnitSymbol.FPerm a rdf:Property ;
    rdfs:label "FPerm" ;
    rdfs:comment "Permittivity, farads per metre." ;
    rdfs:domain cim:UnitSymbol ;
    rdfs:range xsd:string .

cim:UnitSymbol.G a rdf:Property ;
    rdfs:label "G" ;
    rdfs:comment "Magnetic flux density, gausses (1 G = 10-4 T)." ;
    rdfs:domain cim:UnitSymbol ;
    rdfs:range xsd:string .

cim:UnitSymbol.Gy a rdf:Property ;
    rdfs:label "Gy" ;
    rdfs:comment "Absorbed dose in grays (J/kg)." ;
    rdfs:domain cim:UnitSymbol ;
    rdfs:range xsd:string .

cim:UnitSymbol.GyPers a rdf:Property ;
    rdfs:label "GyPers" ;
    rdfs:comment "Absorbed dose rate, grays per second." ;
    rdfs:domain cim:UnitSymbol ;
    rdfs:range xsd:string .

cim:UnitSymbol.H a rdf:Property ;
    rdfs:label "H" ;
    rdfs:comment "Electric inductance in henrys (Wb/A)." ;
    rdfs:domain cim:UnitSymbol ;
    rdfs:range xsd:string .

cim:UnitSymbol.HPerm a rdf:Property ;
    rdfs:label "HPerm" ;
    rdfs:comment "Permeability, henrys per metre." ;
    rdfs:domain cim:UnitSymbol ;
    rdfs:range xsd:string .

cim:UnitSymbol.Hz a rdf:Property ;
    rdfs:label "Hz" ;
    rdfs:comment "Frequency in hertz (1/s)." ;
    rdfs:domain cim:UnitSymbol ;
    rdfs:range xsd:string .

cim:UnitSymbol.HzPerHz a rdf:Property ;
    rdfs:label "HzPerHz" ;
    rdfs:comment "Frequency, rate of frequency change.   Note: Users may need to supply a prefix such as m to show rates such as mHz/Hz." ;
    rdfs:domain cim:UnitSymbol ;
    rdfs:range xsd:string .

cim:UnitSymbol.HzPers a rdf:Property ;
    rdfs:label "HzPers" ;
    rdfs:comment "Rate of change of frequency in hertz per second." ;
    rdfs:domain cim:UnitSymbol ;
    rdfs:range xsd:string .

cim:UnitSymbol.J a rdf:Property ;
    rdfs:label "J" ;
    rdfs:comment "Energy in joules (Nm = CV = Ws)." ;
    rdfs:domain cim:UnitSymbol ;
    rdfs:range xsd:string .

cim:UnitSymbol.JPerK a rdf:Property ;
    rdfs:label "JPerK" ;
    rdfs:comment "Heat capacity in joules/kelvin." ;
    rdfs:domain cim:UnitSymbol ;
    rdfs:range xsd:string .

cim:UnitSymbol.JPerkg a rdf:Property ;
    rdfs:label "JPerkg" ;
    rdfs:comment "Specific energy, Joules / kg." ;
    rdfs:domain cim:UnitSymbol ;
    rdfs:range xsd:string .

cim:UnitSymbol.JPerkgK a rdf:Property ;
    rdfs:label "JPerkgK" ;
    rdfs:comment "Specific heat capacity, specific entropy, joules per kilogram Kelvin." ;
    rdfs:domain cim:UnitSymbol ;
    rdfs:range xsd:string .

cim:UnitSymbol.JPerm2 a rdf:Property ;
    rdfs:label "JPerm2" ;
    rdfs:comment "Insulation energy density, joules per square metre or watt second per square metre." ;
    rdfs:domain cim:UnitSymbol ;
    rdfs:range xsd:string .

cim:UnitSymbol.JPerm3 a rdf:Property ;
    rdfs:label "JPerm3" ;
    rdfs:comment "Energy density, joules per cubic metre." ;
    rdfs:domain cim:UnitSymbol ;
    rdfs:range xsd:string .

cim:UnitSymbol.JPermol a rdf:Property ;
    rdfs:label "JPermol" ;
    rdfs:comment "Molar energy, joules per mole." ;
    rdfs:domain cim:UnitSymbol ;
    rdfs:range xsd:string .

cim:UnitSymbol.JPermolK a rdf:Property ;
    rdfs:label "JPermolK" ;
    rdfs:comment "Molar entropy, molar heat capacity, joules per mole kelvin." ;
    rdfs:domain cim:UnitSymbol ;
    rdfs:range xsd:string .

cim:UnitSymbol.JPers a rdf:Property ;
    rdfs:label "JPers" ;
    rdfs:comment "Energy rate in joules per second (J/s)." ;
    rdfs:domain cim:UnitSymbol ;
    rdfs:range xsd:string .

cim:UnitSymbol.K a rdf:Property ;
    rdfs:label "K" ;
    rdfs:comment "Temperature in kelvins." ;
    rdfs:domain cim:UnitSymbol ;
    rdfs:range xsd:string .

cim:UnitSymbol.KPers a rdf:Property ;
    rdfs:label "KPers" ;
    rdfs:comment "Temperature change rate in kelvins per second." ;
    rdfs:domain cim:UnitSymbol ;
    rdfs:range xsd:string .

cim:UnitSymbol.M a rdf:Property ;
    rdfs:label "M" ;
    rdfs:comment "Length, nautical miles (1 M = 1852 m)." ;
    rdfs:domain cim:UnitSymbol ;
    rdfs:range xsd:string .

cim:UnitSymbol.Mx a rdf:Property ;
    rdfs:label "Mx" ;
    rdfs:comment "Magnetic flux, maxwells (1 Mx = 10-8 Wb)." ;
    rdfs:domain cim:UnitSymbol ;
    rdfs:range xsd:string .

cim:UnitSymbol.N a rdf:Property ;
    rdfs:label "N" ;
    rdfs:comment "Force in newtons (kgm/s)." ;
    rdfs:domain cim:UnitSymbol ;
    rdfs:range xsd:string .

cim:UnitSymbol.NPerm a rdf:Property ;
    rdfs:label "NPerm" ;
    rdfs:comment "Surface tension, newton per metre." ;
    rdfs:domain cim:UnitSymbol ;
    rdfs:range xsd:string .

cim:UnitSymbol.Nm a rdf:Property ;
    rdfs:label "Nm" ;
    rdfs:comment "Moment of force, newton metres." ;
    rdfs:domain cim:UnitSymbol ;
    rdfs:range xsd:string .

cim:UnitSymbol.Oe a rdf:Property ;
    rdfs:label "Oe" ;
    rdfs:comment "Magnetic field in oersteds, (1 Oe = (103/4p) A/m)." ;
    rdfs:domain cim:UnitSymbol ;
    rdfs:range xsd:string .

cim:UnitSymbol.Pa a rdf:Property ;
    rdfs:label "Pa" ;
    rdfs:comment "Pressure in pascals (N/m). Note: the absolute or relative measurement of pressure is implied with this entry. See below for more explicit forms." ;
    rdfs:domain cim:UnitSymbol ;
    rdfs:range xsd:string .

cim:UnitSymbol.PaPers a rdf:Property ;
    rdfs:label "PaPers" ;
    rdfs:comment "Pressure change rate in pascals per second." ;
    rdfs:domain cim:UnitSymbol ;
    rdfs:range xsd:string .

cim:UnitSymbol.Pas a rdf:Property ;
    rdfs:label "Pas" ;
    rdfs:comment "Dynamic viscosity, pascal seconds." ;
    rdfs:domain cim:UnitSymbol ;
    rdfs:range xsd:string .

cim:UnitSymbol.Q a rdf:Property ;
    rdfs:label "Q" ;
    rdfs:comment "Quantity power, Q." ;
    rdfs:domain cim:UnitSymbol ;
    rdfs:range xsd:string .

cim:UnitSymbol.Qh a rdf:Property ;
    rdfs:label "Qh" ;
    rdfs:comment "Quantity energy, Qh." ;
    rdfs:domain cim:UnitSymbol ;
    rdfs:range xsd:string .

cim:UnitSymbol.S a rdf:Property ;
    rdfs:label "S" ;
    rdfs:comment "Conductance in siemens." ;
    rdfs:domain cim:UnitSymbol ;
    rdfs:range xsd:string .

cim:UnitSymbol.SPerm a rdf:Property ;
    rdfs:label "SPerm" ;
    rdfs:comment "Conductance per length (F/m)." ;
    rdfs:domain cim:UnitSymbol ;
    rdfs:range xsd:string .

cim:UnitSymbol.Sv a rdf:Property ;
    rdfs:label "Sv" ;
    rdfs:comment "Dose equivalent in sieverts (J/kg)." ;
    rdfs:domain cim:UnitSymbol ;
    rdfs:range xsd:string .

cim:UnitSymbol.T a rdf:Property ;
    rdfs:label "T" ;
    rdfs:comment "Magnetic flux density in teslas (Wb/m2)." ;
    rdfs:domain cim:UnitSymbol ;
    rdfs:range xsd:string .

cim:UnitSymbol.V a rdf:Property ;
    rdfs:label "V" ;
    rdfs:comment "Electric potential in volts (W/A)." ;
    rdfs:domain cim:UnitSymbol ;
    rdfs:range xsd:string .

cim:UnitSymbol.V2 a rdf:Property ;
    rdfs:label "V2" ;
    rdfs:comment "Volt squared (W/A)." ;
    rdfs:domain cim:UnitSymbol ;
    rdfs:range xsd:string .

cim:UnitSymbol.V2h a rdf:Property ;
    rdfs:label "V2h" ;
    rdfs:comment "Volt-squared hour, volt-squared-hours." ;
    rdfs:domain cim:UnitSymbol ;
    rdfs:range xsd:string .

cim:UnitSymbol.VA a rdf:Property ;
    rdfs:label "VA" ;
    rdfs:comment "Apparent power in volt amperes. See also real power and reactive power." ;
    rdfs:domain cim:UnitSymbol ;
    rdfs:range xsd:string .

cim:UnitSymbol.VAh a rdf:Property ;
    rdfs:label "VAh" ;
    rdfs:comment "Apparent energy in volt ampere hours." ;
    rdfs:domain cim:UnitSymbol ;
    rdfs:range xsd:string .

cim:UnitSymbol.VAr a rdf:Property ;
    rdfs:label "VAr" ;
    rdfs:comment "Reactive power in volt amperes reactive. The reactive or imaginary component of electrical power (VIsin(phi)). (See also real power and apparent power).\nNote: Different meter designs use different methods to arrive at their results. Some meters may compute reactive power as an arithmetic value, while others compute the value vectorially. The data consumer should determine the method in use and the suitability of the measurement for the intended purpose." ;
    rdfs:domain cim:UnitSymbol ;
    rdfs:range xsd:string .

cim:UnitSymbol.VArh a rdf:Property ;
    rdfs:label "VArh" ;
    rdfs:comment "Reactive energy in volt ampere reactive hours." ;
    rdfs:domain cim:UnitSymbol ;
    rdfs:range xsd:string .

cim:UnitSymbol.VPerHz a rdf:Property ;
    rdfs:label "VPerHz" ;
    rdfs:comment "Magnetic flux in volt per hertz." ;
    rdfs:domain cim:UnitSymbol ;
    rdfs:range xsd:string .

cim:UnitSymbol.VPerV a rdf:Property ;
    rdfs:label "VPerV" ;
    rdfs:comment "Voltage, ratio of voltages.  Note: Users may need to supply a prefix such as m to show rates such as mV/V." ;
    rdfs:domain cim:UnitSymbol ;
    rdfs:range xsd:string .

cim:UnitSymbol.VPerVA a rdf:Property ;
    rdfs:label "VPerVA" ;
    rdfs:comment "Power factor, PF, the ratio of the active power to the apparent power.  Note: The sign convention used for power factor will differ between IEC meters and EEI (ANSI) meters. It is assumed that the data consumers understand the type of meter being used and agree on the sign convention in use at any given utility." ;
    rdfs:domain cim:UnitSymbol ;
    rdfs:range xsd:string .

cim:UnitSymbol.VPerVAr a rdf:Property ;
    rdfs:label "VPerVAr" ;
    rdfs:comment "Power factor, PF, the ratio of the active power to the apparent power. Note: The sign convention used for power factor will differ between IEC meters and EEI (ANSI) meters. It is assumed that the data consumers understand the type of meter being used and agree on the sign convention in use at any given utility." ;
    rdfs:domain cim:UnitSymbol ;
    rdfs:range xsd:string .

cim:UnitSymbol.VPerm a rdf:Property ;
    rdfs:label "VPerm" ;
    rdfs:comment "Electric field strength, volts per metre." ;
    rdfs:domain cim:UnitSymbol ;
    rdfs:range xsd:string .

cim:UnitSymbol.Vh a rdf:Property ;
    rdfs:label "Vh" ;
    rdfs:comment "Volt-hour, Volt hours." ;
    rdfs:domain cim:UnitSymbol ;
    rdfs:range xsd:string .

cim:UnitSymbol.Vs a rdf:Property ;
    rdfs:label "Vs" ;
    rdfs:comment "Volt seconds (Ws/A)." ;
    rdfs:domain cim:UnitSymbol ;
    rdfs:range xsd:string .

cim:UnitSymbol.W a rdf:Property ;
    rdfs:label "W" ;
    rdfs:comment "Real power in watts (J/s). Electrical power may have real and reactive components. The real portion of electrical power (I&#178;R or VIcos(phi)), is expressed in Watts. See also apparent power and reactive power." ;
    rdfs:domain cim:UnitSymbol ;
    rdfs:range xsd:string .

cim:UnitSymbol.WPerA a rdf:Property ;
    rdfs:label "WPerA" ;
    rdfs:comment "Active power per current flow, watts per Ampere." ;
    rdfs:domain cim:UnitSymbol ;
    rdfs:range xsd:string .

cim:UnitSymbol.WPerW a rdf:Property ;
    rdfs:label "WPerW" ;
    rdfs:comment "Signal Strength, ratio of power.   Note: Users may need to supply a prefix such as m to show rates such as mW/W." ;
    rdfs:domain cim:UnitSymbol ;
    rdfs:range xsd:string .

cim:UnitSymbol.WPerm2 a rdf:Property ;
    rdfs:label "WPerm2" ;
    rdfs:comment "Heat flux density, irradiance, watts per square metre." ;
    rdfs:domain cim:UnitSymbol ;
    rdfs:range xsd:string .

cim:UnitSymbol.WPerm2sr a rdf:Property ;
    rdfs:label "WPerm2sr" ;
    rdfs:comment "Radiance, watts per square metre steradian." ;
    rdfs:domain cim:UnitSymbol ;
    rdfs:range xsd:string .

cim:UnitSymbol.WPermK a rdf:Property ;
    rdfs:label "WPermK" ;
    rdfs:comment "Thermal conductivity in watt/metres kelvin." ;
    rdfs:domain cim:UnitSymbol ;
    rdfs:range xsd:string .

cim:UnitSymbol.WPers a rdf:Property ;
    rdfs:label "WPers" ;
    rdfs:comment "Ramp rate in watts per second." ;
    rdfs:domain cim:UnitSymbol ;
    rdfs:range xsd:string .

cim:UnitSymbol.WPersr a rdf:Property ;
    rdfs:label "WPersr" ;
    rdfs:comment "Radiant intensity, watts per steradian." ;
    rdfs:domain cim:UnitSymbol ;
    rdfs:range xsd:string .

cim:UnitSymbol.Wb a rdf:Property ;
    rdfs:label "Wb" ;
    rdfs:comment "Magnetic flux in webers (Vs)." ;
    rdfs:domain cim:UnitSymbol ;
    rdfs:range xsd:string .

cim:UnitSymbol.Wh a rdf:Property ;
    rdfs:label "Wh" ;
    rdfs:comment "Real energy in watt hours." ;
    rdfs:domain cim:UnitSymbol ;
    rdfs:range xsd:string .

cim:UnitSymbol.anglemin a rdf:Property ;
    rdfs:label "anglemin" ;
    rdfs:comment "Plane angle, minutes." ;
    rdfs:domain cim:UnitSymbol ;
    rdfs:range xsd:string .

cim:UnitSymbol.anglesec a rdf:Property ;
    rdfs:label "anglesec" ;
    rdfs:comment "Plane angle, seconds." ;
    rdfs:domain cim:UnitSymbol ;
    rdfs:range xsd:string .

cim:UnitSymbol.bar a rdf:Property ;
    rdfs:label "bar" ;
    rdfs:comment "Pressure in bars, (1 bar = 100 kPa)." ;
    rdfs:domain cim:UnitSymbol ;
    rdfs:range xsd:string .

cim:UnitSymbol.cd a rdf:Property ;
    rdfs:label "cd" ;
    rdfs:comment "Luminous intensity in candelas." ;
    rdfs:domain cim:UnitSymbol ;
    rdfs:range xsd:string .

cim:UnitSymbol.charPers a rdf:Property ;
    rdfs:label "charPers" ;
    rdfs:comment "Data rate (baud) in characters per second." ;
    rdfs:domain cim:UnitSymbol ;
    rdfs:range xsd:string .

cim:UnitSymbol.character a rdf:Property ;
    rdfs:label "character" ;
    rdfs:comment "Number of characters." ;
    rdfs:domain cim:UnitSymbol ;
    rdfs:range xsd:string .

cim:UnitSymbol.cosPhi a rdf:Property ;
    rdfs:label "cosPhi" ;
    rdfs:comment "Power factor, dimensionless.\nNote 1: This definition of power factor only holds for balanced systems. See the alternative definition under code 153.\nNote 2: Beware of differing sign conventions in use between the IEC and EEI. It is assumed that the data consumer understands the type of meter in use and the sign convention in use by the utility." ;
    rdfs:domain cim:UnitSymbol ;
    rdfs:range xsd:string .

cim:UnitSymbol.count a rdf:Property ;
    rdfs:label "count" ;
    rdfs:comment "Amount of substance, Counter value." ;
    rdfs:domain cim:UnitSymbol ;
    rdfs:range xsd:string .

cim:UnitSymbol.d a rdf:Property ;
    rdfs:label "d" ;
    rdfs:comment "Time in days, day = 24 h = 86400 s." ;
    rdfs:domain cim:UnitSymbol ;
    rdfs:range xsd:string .

cim:UnitSymbol.dB a rdf:Property ;
    rdfs:label "dB" ;
    rdfs:comment "Sound pressure level in decibels. Note:  multiplier d is included in this unit symbol for compatibility with IEC 61850-7-3." ;
    rdfs:domain cim:UnitSymbol ;
    rdfs:range xsd:string .

cim:UnitSymbol.dBm a rdf:Property ;
    rdfs:label "dBm" ;
    rdfs:comment "Power level (logarithmic ratio of signal strength , Bel-mW), normalized to 1mW. Note:  multiplier d is included in this unit symbol for compatibility with IEC 61850-7-3." ;
    rdfs:domain cim:UnitSymbol ;
    rdfs:range xsd:string .

cim:UnitSymbol.deg a rdf:Property ;
    rdfs:label "deg" ;
    rdfs:comment "Plane angle in degrees." ;
    rdfs:domain cim:UnitSymbol ;
    rdfs:range xsd:string .

cim:UnitSymbol.degC a rdf:Property ;
    rdfs:label "degC" ;
    rdfs:comment "Relative temperature in degrees Celsius.\nIn the SI unit system the symbol is C. Electric charge is measured in coulomb that has the unit symbol C. To distinguish degree Celsius from coulomb the symbol used in the UML is degC. The reason for not using C is that the special character  is difficult to manage in software." ;
    rdfs:domain cim:UnitSymbol ;
    rdfs:range xsd:string .

cim:UnitSymbol.ft3 a rdf:Property ;
    rdfs:label "ft3" ;
    rdfs:comment "Volume, cubic feet." ;
    rdfs:domain cim:UnitSymbol ;
    rdfs:range xsd:string .

cim:UnitSymbol.gPerg a rdf:Property ;
    rdfs:label "gPerg" ;
    rdfs:comment "Concentration, The ratio of the mass of a solute divided by the mass of  the solution. Note: Users may need use a prefix such a  to express a quantity such as g/g." ;
    rdfs:domain cim:UnitSymbol ;
    rdfs:range xsd:string .

cim:UnitSymbol.gal a rdf:Property ;
    rdfs:label "gal" ;
    rdfs:comment "Volume in gallons, US gallon (1 gal = 231 in3 = 128 fl ounce)." ;
    rdfs:domain cim:UnitSymbol ;
    rdfs:range xsd:string .

cim:UnitSymbol.h a rdf:Property ;
    rdfs:label "h" ;
    rdfs:comment "Time in hours, hour = 60 min = 3600 s." ;
    rdfs:domain cim:UnitSymbol ;
    rdfs:range xsd:string .

cim:UnitSymbol.ha a rdf:Property ;
    rdfs:label "ha" ;
    rdfs:comment "Area, hectares." ;
    rdfs:domain cim:UnitSymbol ;
    rdfs:range xsd:string .

cim:UnitSymbol.kat a rdf:Property ;
    rdfs:label "kat" ;
    rdfs:comment "Catalytic activity, katal = mol / s." ;
    rdfs:domain cim:UnitSymbol ;
    rdfs:range xsd:string .

cim:UnitSymbol.katPerm3 a rdf:Property ;
    rdfs:label "katPerm3" ;
    rdfs:comment "Catalytic activity concentration, katals per cubic metre." ;
    rdfs:domain cim:UnitSymbol ;
    rdfs:range xsd:string .

cim:UnitSymbol.kg a rdf:Property ;
    rdfs:label "kg" ;
    rdfs:comment "Mass in kilograms.  Note: multiplier k is included in this unit symbol for compatibility with IEC 61850-7-3." ;
    rdfs:domain cim:UnitSymbol ;
    rdfs:range xsd:string .

cim:UnitSymbol.kgPerJ a rdf:Property ;
    rdfs:label "kgPerJ" ;
    rdfs:comment "Weight per energy in kilograms per joule (kg/J). Note: multiplier k is included in this unit symbol for compatibility with IEC 61850-7-3." ;
    rdfs:domain cim:UnitSymbol ;
    rdfs:range xsd:string .

cim:UnitSymbol.kgPerm3 a rdf:Property ;
    rdfs:label "kgPerm3" ;
    rdfs:comment "Density in kilogram/cubic metres (kg/m). Note: multiplier k is included in this unit symbol for compatibility with IEC 61850-7-3." ;
    rdfs:domain cim:UnitSymbol ;
    rdfs:range xsd:string .

cim:UnitSymbol.kgm a rdf:Property ;
    rdfs:label "kgm" ;
    rdfs:comment "Moment of mass in kilogram metres (kgm) (first moment of mass). Note: multiplier k is included in this unit symbol for compatibility with IEC 61850-7-3." ;
    rdfs:domain cim:UnitSymbol ;
    rdfs:range xsd:string .

cim:UnitSymbol.kgm2 a rdf:Property ;
    rdfs:label "kgm2" ;
    rdfs:comment "Moment of mass in kilogram square metres (kgm) (Second moment of mass, commonly called the moment of inertia). Note: multiplier k is included in this unit symbol for compatibility with IEC 61850-7-3." ;
    rdfs:domain cim:UnitSymbol ;
    rdfs:range xsd:string .

cim:UnitSymbol.kn a rdf:Property ;
    rdfs:label "kn" ;
    rdfs:comment "Speed, knots (1 kn = 1852/3600) m/s." ;
    rdfs:domain cim:UnitSymbol ;
    rdfs:range xsd:string .

cim:UnitSymbol.l a rdf:Property ;
    rdfs:label "l" ;
    rdfs:comment "Volume in litres, litre = dm3 = m3/1000." ;
    rdfs:domain cim:UnitSymbol ;
    rdfs:range xsd:string .

cim:UnitSymbol.lPerh a rdf:Property ;
    rdfs:label "lPerh" ;
    rdfs:comment "Volumetric flow rate, litres per hour." ;
    rdfs:domain cim:UnitSymbol ;
    rdfs:range xsd:string .

cim:UnitSymbol.lPerl a rdf:Property ;
    rdfs:label "lPerl" ;
    rdfs:comment "Concentration, The ratio of the volume of a solute divided by the volume of  the solution. Note: Users may need use a prefix such a  to express a quantity such as L/L." ;
    rdfs:domain cim:UnitSymbol ;
    rdfs:range xsd:string .

cim:UnitSymbol.lPers a rdf:Property ;
    rdfs:label "lPers" ;
    rdfs:comment "Volumetric flow rate in litres per second." ;
    rdfs:domain cim:UnitSymbol ;
    rdfs:range xsd:string .

cim:UnitSymbol.lm a rdf:Property ;
    rdfs:label "lm" ;
    rdfs:comment "Luminous flux in lumens (cdsr)." ;
    rdfs:domain cim:UnitSymbol ;
    rdfs:range xsd:string .

cim:UnitSymbol.lx a rdf:Property ;
    rdfs:label "lx" ;
    rdfs:comment "Illuminance in lux (lm/m)." ;
    rdfs:domain cim:UnitSymbol ;
    rdfs:range xsd:string .

cim:UnitSymbol.m a rdf:Property ;
    rdfs:label "m" ;
    rdfs:comment "Length in metres." ;
    rdfs:domain cim:UnitSymbol ;
    rdfs:range xsd:string .

cim:UnitSymbol.m2 a rdf:Property ;
    rdfs:label "m2" ;
    rdfs:comment "Area in square metres (m)." ;
    rdfs:domain cim:UnitSymbol ;
    rdfs:range xsd:string .

cim:UnitSymbol.m2Pers a rdf:Property ;
    rdfs:label "m2Pers" ;
    rdfs:comment "Viscosity in square metres / second (m/s)." ;
    rdfs:domain cim:UnitSymbol ;
    rdfs:range xsd:string .

cim:UnitSymbol.m3 a rdf:Property ;
    rdfs:label "m3" ;
    rdfs:comment "Volume in cubic metres (m)." ;
    rdfs:domain cim:UnitSymbol ;
    rdfs:range xsd:string .

cim:UnitSymbol.m3Compensated a rdf:Property ;
    rdfs:label "m3Compensated" ;
    rdfs:comment "Volume, cubic metres, with the value compensated for weather effects." ;
    rdfs:domain cim:UnitSymbol ;
    rdfs:range xsd:string .

cim:UnitSymbol.m3Perh a rdf:Property ;
    rdfs:label "m3Perh" ;
    rdfs:comment "Volumetric flow rate, cubic metres per hour." ;
    rdfs:domain cim:UnitSymbol ;
    rdfs:range xsd:string .

cim:UnitSymbol.m3Perkg a rdf:Property ;
    rdfs:label "m3Perkg" ;
    rdfs:comment "Specific volume, cubic metres per kilogram, v." ;
    rdfs:domain cim:UnitSymbol ;
    rdfs:range xsd:string .

cim:UnitSymbol.m3Pers a rdf:Property ;
    rdfs:label "m3Pers" ;
    rdfs:comment "Volumetric flow rate in cubic metres per second (m/s)." ;
    rdfs:domain cim:UnitSymbol ;
    rdfs:range xsd:string .

cim:UnitSymbol.m3Uncompensated a rdf:Property ;
    rdfs:label "m3Uncompensated" ;
    rdfs:comment "Volume, cubic metres, with the value uncompensated for weather effects." ;
    rdfs:domain cim:UnitSymbol ;
    rdfs:range xsd:string .

cim:UnitSymbol.mPerm3 a rdf:Property ;
    rdfs:label "mPerm3" ;
    rdfs:comment "Fuel efficiency in metres per cubic metres (m/m)." ;
    rdfs:domain cim:UnitSymbol ;
    rdfs:range xsd:string .

cim:UnitSymbol.mPers a rdf:Property ;
    rdfs:label "mPers" ;
    rdfs:comment "Velocity in metres per second (m/s)." ;
    rdfs:domain cim:UnitSymbol ;
    rdfs:range xsd:string .

cim:UnitSymbol.mPers2 a rdf:Property ;
    rdfs:label "mPers2" ;
    rdfs:comment "Acceleration in metres per second squared (m/s)." ;
    rdfs:domain cim:UnitSymbol ;
    rdfs:range xsd:string .

cim:UnitSymbol.min a rdf:Property ;
    rdfs:label "min" ;
    rdfs:comment "Time in minutes, minute  = 60 s." ;
    rdfs:domain cim:UnitSymbol ;
    rdfs:range xsd:string .

cim:UnitSymbol.mmHg a rdf:Property ;
    rdfs:label "mmHg" ;
    rdfs:comment "Pressure, millimetres of mercury (1 mmHg is approximately 133.3 Pa)." ;
    rdfs:domain cim:UnitSymbol ;
    rdfs:range xsd:string .

cim:UnitSymbol.mol a rdf:Property ;
    rdfs:label "mol" ;
    rdfs:comment "Amount of substance in moles." ;
    rdfs:domain cim:UnitSymbol ;
    rdfs:range xsd:string .

cim:UnitSymbol.molPerkg a rdf:Property ;
    rdfs:label "molPerkg" ;
    rdfs:comment "Concentration, Molality, the amount of solute in moles and the amount of solvent in kilograms." ;
    rdfs:domain cim:UnitSymbol ;
    rdfs:range xsd:string .

cim:UnitSymbol.molPerm3 a rdf:Property ;
    rdfs:label "molPerm3" ;
    rdfs:comment "Concentration, The amount of substance concentration, (c), the amount of solvent in moles divided by the volume of solution in m." ;
    rdfs:domain cim:UnitSymbol ;
    rdfs:range xsd:string .

cim:UnitSymbol.molPermol a rdf:Property ;
    rdfs:label "molPermol" ;
    rdfs:comment "Concentration, Molar fraction, the ratio of the molar amount of a solute divided by the molar amount of the solution." ;
    rdfs:domain cim:UnitSymbol ;
    rdfs:range xsd:string .

cim:UnitSymbol.none a rdf:Property ;
    rdfs:label "none" ;
    rdfs:comment "Dimension less quantity, e.g. count, per unit, etc." ;
    rdfs:domain cim:UnitSymbol ;
    rdfs:range xsd:string .

cim:UnitSymbol.ohm a rdf:Property ;
    rdfs:label "ohm" ;
    rdfs:comment "Electric resistance in ohms (V/A)." ;
    rdfs:domain cim:UnitSymbol ;
    rdfs:range xsd:string .

cim:UnitSymbol.ohmPerm a rdf:Property ;
    rdfs:label "ohmPerm" ;
    rdfs:comment "Electric resistance per length in ohms per metre ((V/A)/m)." ;
    rdfs:domain cim:UnitSymbol ;
    rdfs:range xsd:string .

cim:UnitSymbol.ohmm a rdf:Property ;
    rdfs:label "ohmm" ;
    rdfs:comment "Resistivity, ohm metres, (rho)." ;
    rdfs:domain cim:UnitSymbol ;
    rdfs:range xsd:string .

cim:UnitSymbol.onePerHz a rdf:Property ;
    rdfs:label "onePerHz" ;
    rdfs:comment "Reciprocal of frequency (1/Hz)." ;
    rdfs:domain cim:UnitSymbol ;
    rdfs:range xsd:string .

cim:UnitSymbol.onePerm a rdf:Property ;
    rdfs:label "onePerm" ;
    rdfs:comment "Wavenumber, reciprocal metres,  (1/m)." ;
    rdfs:domain cim:UnitSymbol ;
    rdfs:range xsd:string .

cim:UnitSymbol.ppm a rdf:Property ;
    rdfs:label "ppm" ;
    rdfs:comment "Concentration in parts per million." ;
    rdfs:domain cim:UnitSymbol ;
    rdfs:range xsd:string .

cim:UnitSymbol.rad a rdf:Property ;
    rdfs:label "rad" ;
    rdfs:comment "Plane angle in radians (m/m)." ;
    rdfs:domain cim:UnitSymbol ;
    rdfs:range xsd:string .

cim:UnitSymbol.radPers a rdf:Property ;
    rdfs:label "radPers" ;
    rdfs:comment "Angular velocity in radians per second (rad/s)." ;
    rdfs:domain cim:UnitSymbol ;
    rdfs:range xsd:string .

cim:UnitSymbol.radPers2 a rdf:Property ;
    rdfs:label "radPers2" ;
    rdfs:comment "Angular acceleration, radians per second squared." ;
    rdfs:domain cim:UnitSymbol ;
    rdfs:range xsd:string .

cim:UnitSymbol.rev a rdf:Property ;
    rdfs:label "rev" ;
    rdfs:comment "Amount of rotation, revolutions." ;
    rdfs:domain cim:UnitSymbol ;
    rdfs:range xsd:string .

cim:UnitSymbol.rotPers a rdf:Property ;
    rdfs:label "rotPers" ;
    rdfs:comment "Rotations per second (1/s). See also Hz (1/s)." ;
    rdfs:domain cim:UnitSymbol ;
    rdfs:range xsd:string .

cim:UnitSymbol.s a rdf:Property ;
    rdfs:label "s" ;
    rdfs:comment "Time in seconds." ;
    rdfs:domain cim:UnitSymbol ;
    rdfs:range xsd:string .

cim:UnitSymbol.sPers a rdf:Property ;
    rdfs:label "sPers" ;
    rdfs:comment "Time, Ratio of time.  Note: Users may need to supply a prefix such as &#181; to show rates such as &#181;s/s." ;
    rdfs:domain cim:UnitSymbol ;
    rdfs:range xsd:string .

cim:UnitSymbol.sr a rdf:Property ;
    rdfs:label "sr" ;
    rdfs:comment "Solid angle in steradians (m2/m2)." ;
    rdfs:domain cim:UnitSymbol ;
    rdfs:range xsd:string .

cim:UnitSymbol.therm a rdf:Property ;
    rdfs:label "therm" ;
    rdfs:comment "Energy, therms." ;
    rdfs:domain cim:UnitSymbol ;
    rdfs:range xsd:string .

cim:UnitSymbol.tonne a rdf:Property ;
    rdfs:label "tonne" ;
    rdfs:comment "Mass in tons, tonne or metric  ton (1000 kg = 1 Mg)." ;
    rdfs:domain cim:UnitSymbol ;
    rdfs:range xsd:string .

cim:UsagePoint.ContactDetails a rdf:Property ;
    rdfs:label "UsagePoint.ContactDetails" ;
    rdfs:comment "\\[ZBEX\\] All contact details for this UsagePoint." ;
    rdfs:domain cim:UsagePoint ;
    rdfs:range cim:ContactDetails ;
    profile:targetCardinality "0..1" .

cim:UsagePoint.CustomerAgreement a rdf:Property ;
    rdfs:label "UsagePoint.CustomerAgreement" ;
    rdfs:comment "Customer agreement regulating this service delivery point." ;
    rdfs:domain cim:UsagePoint ;
    rdfs:range cim:CustomerAgreement ;
    profile:targetCardinality "0..1" .

cim:UsagePoint.EndDevice a rdf:Property ;
    rdfs:label "UsagePoint.EndDevice" ;
    rdfs:comment "Usage point to which this end device belongs. All end devices at this usage point." ;
    rdfs:domain cim:UsagePoint ;
    rdfs:range cim:EndDevice ;
    profile:sourceCardinality "0..*" ;
    profile:targetCardinality "0..*" .

cim:UsagePoint.Equipment a rdf:Property ;
    rdfs:label "UsagePoint.Equipment" ;
    rdfs:comment "All usage points connected to the electrical grid through this equipment. All equipment connecting this usage point to the electrical grid." ;
    rdfs:domain cim:UsagePoint ;
    rdfs:range cim:Equipment ;
    profile:sourceCardinality "0..*" ;
    profile:targetCardinality "0..*" .

cim:UsagePoint.Location a rdf:Property ;
    rdfs:label "UsagePoint.Location" ;
    rdfs:comment "Location of this usage point." ;
    rdfs:domain cim:UsagePoint ;
    rdfs:range cim:Location ;
    profile:targetCardinality "0..1" .

cim:UsagePoint.approvedInverterCapacity a rdf:Property ;
    rdfs:label "approvedInverterCapacity" ;
    rdfs:comment "\\[ZBEX\\] The approved inverter capacity at this UsagePoint in volt-amperes." ;
    rdfs:domain cim:UsagePoint ;
    rdfs:range cim:ApparentPower .

cim:UsagePoint.connectionCategory a rdf:Property ;
    rdfs:label "connectionCategory" ;
    rdfs:comment "A code used to specify the connection category, e.g., low voltage or low pressure, where the usage point is defined." ;
    rdfs:domain cim:UsagePoint ;
    rdfs:range xsd:string .

cim:UsagePoint.contacts a rdf:Property ;
    rdfs:label "contacts" ;
    rdfs:comment "[ZBEX] All contact details for this UsagePoint." ;
    rdfs:domain cim:UsagePoint ;
    rdfs:range cim:ListContactDetails .

cim:UsagePoint.isVirtual a rdf:Property ;
    rdfs:label "isVirtual" ;
    rdfs:comment "If true, this usage point is virtual, i.e., no physical location exists in the network where a meter could be located to collect the meter readings. For example, one may define a virtual usage point to serve as an aggregation of usage for all of a company's premises distributed widely across the distribution territory. Otherwise, the usage point is physical, i.e., there is a logical point in the network where a meter could be located to collect meter readings." ;
    rdfs:domain cim:UsagePoint ;
    rdfs:range xsd:boolean .

cim:UsagePoint.phaseCode a rdf:Property ;
    rdfs:label "phaseCode" ;
    rdfs:comment "Phase code. Number of wires and specific nominal phases can be deduced from enumeration literal values. For example, ABCN is three-phase, four-wire, s12n (splitSecondary12N) is single-phase, three-wire, and s1n and s2n are single-phase, two-wire." ;
    rdfs:domain cim:UsagePoint ;
    rdfs:range cim:PhaseCode .

cim:VectorGroup.D0 a rdf:Property ;
    rdfs:label "D0" ;
    rdfs:comment "" ;
    rdfs:domain cim:VectorGroup ;
    rdfs:range xsd:string .

cim:VectorGroup.DD0 a rdf:Property ;
    rdfs:label "DD0" ;
    rdfs:comment "" ;
    rdfs:domain cim:VectorGroup ;
    rdfs:range xsd:string .

cim:VectorGroup.DD6 a rdf:Property ;
    rdfs:label "DD6" ;
    rdfs:comment "" ;
    rdfs:domain cim:VectorGroup ;
    rdfs:range xsd:string .

cim:VectorGroup.DDN0 a rdf:Property ;
    rdfs:label "DDN0" ;
    rdfs:comment "" ;
    rdfs:domain cim:VectorGroup ;
    rdfs:range xsd:string .

cim:VectorGroup.DND0 a rdf:Property ;
    rdfs:label "DND0" ;
    rdfs:comment "" ;
    rdfs:domain cim:VectorGroup ;
    rdfs:range xsd:string .

cim:VectorGroup.DNYN1 a rdf:Property ;
    rdfs:label "DNYN1" ;
    rdfs:comment "" ;
    rdfs:domain cim:VectorGroup ;
    rdfs:range xsd:string .

cim:VectorGroup.DNYN11 a rdf:Property ;
    rdfs:label "DNYN11" ;
    rdfs:comment "" ;
    rdfs:domain cim:VectorGroup ;
    rdfs:range xsd:string .

cim:VectorGroup.DY1 a rdf:Property ;
    rdfs:label "DY1" ;
    rdfs:comment "" ;
    rdfs:domain cim:VectorGroup ;
    rdfs:range xsd:string .

cim:VectorGroup.DY11 a rdf:Property ;
    rdfs:label "DY11" ;
    rdfs:comment "" ;
    rdfs:domain cim:VectorGroup ;
    rdfs:range xsd:string .

cim:VectorGroup.DY5 a rdf:Property ;
    rdfs:label "DY5" ;
    rdfs:comment "" ;
    rdfs:domain cim:VectorGroup ;
    rdfs:range xsd:string .

cim:VectorGroup.DY7 a rdf:Property ;
    rdfs:label "DY7" ;
    rdfs:comment "" ;
    rdfs:domain cim:VectorGroup ;
    rdfs:range xsd:string .

cim:VectorGroup.DYN1 a rdf:Property ;
    rdfs:label "DYN1" ;
    rdfs:comment "" ;
    rdfs:domain cim:VectorGroup ;
    rdfs:range xsd:string .

cim:VectorGroup.DYN11 a rdf:Property ;
    rdfs:label "DYN11" ;
    rdfs:comment "" ;
    rdfs:domain cim:VectorGroup ;
    rdfs:range xsd:string .

cim:VectorGroup.DYN5 a rdf:Property ;
    rdfs:label "DYN5" ;
    rdfs:comment "" ;
    rdfs:domain cim:VectorGroup ;
    rdfs:range xsd:string .

cim:VectorGroup.DYN7 a rdf:Property ;
    rdfs:label "DYN7" ;
    rdfs:comment "" ;
    rdfs:domain cim:VectorGroup ;
    rdfs:range xsd:string .

cim:VectorGroup.DZ0 a rdf:Property ;
    rdfs:label "DZ0" ;
    rdfs:comment "" ;
    rdfs:domain cim:VectorGroup ;
    rdfs:range xsd:string .

cim:VectorGroup.DZ1 a rdf:Property ;
    rdfs:label "DZ1" ;
    rdfs:comment "" ;
    rdfs:domain cim:VectorGroup ;
    rdfs:range xsd:string .

cim:VectorGroup.DZ6 a rdf:Property ;
    rdfs:label "DZ6" ;
    rdfs:comment "" ;
    rdfs:domain cim:VectorGroup ;
    rdfs:range xsd:string .

cim:VectorGroup.DZ7 a rdf:Property ;
    rdfs:label "DZ7" ;
    rdfs:comment "" ;
    rdfs:domain cim:VectorGroup ;
    rdfs:range xsd:string .

cim:VectorGroup.DZN0 a rdf:Property ;
    rdfs:label "DZN0" ;
    rdfs:comment "" ;
    rdfs:domain cim:VectorGroup ;
    rdfs:range xsd:string .

cim:VectorGroup.DZN1 a rdf:Property ;
    rdfs:label "DZN1" ;
    rdfs:comment "" ;
    rdfs:domain cim:VectorGroup ;
    rdfs:range xsd:string .

cim:VectorGroup.DZN6 a rdf:Property ;
    rdfs:label "DZN6" ;
    rdfs:comment "" ;
    rdfs:domain cim:VectorGroup ;
    rdfs:range xsd:string .

cim:VectorGroup.DZN7 a rdf:Property ;
    rdfs:label "DZN7" ;
    rdfs:comment "" ;
    rdfs:domain cim:VectorGroup ;
    rdfs:range xsd:string .

cim:VectorGroup.TTN1 a rdf:Property ;
    rdfs:label "TTN1" ;
    rdfs:comment "" ;
    rdfs:domain cim:VectorGroup ;
    rdfs:range xsd:string .

cim:VectorGroup.UNKNOWN a rdf:Property ;
    rdfs:label "UNKNOWN" ;
    rdfs:comment "" ;
    rdfs:domain cim:VectorGroup ;
    rdfs:range xsd:string .

cim:VectorGroup.Y0 a rdf:Property ;
    rdfs:label "Y0" ;
    rdfs:comment "" ;
    rdfs:domain cim:VectorGroup ;
    rdfs:range xsd:string .

cim:VectorGroup.YD1 a rdf:Property ;
    rdfs:label "YD1" ;
    rdfs:comment "" ;
    rdfs:domain cim:VectorGroup ;
    rdfs:range xsd:string .

cim:VectorGroup.YD11 a rdf:Property ;
    rdfs:label "YD11" ;
    rdfs:comment "" ;
    rdfs:domain cim:VectorGroup ;
    rdfs:range xsd:string .

cim:VectorGroup.YD5 a rdf:Property ;
    rdfs:label "YD5" ;
    rdfs:comment "" ;
    rdfs:domain cim:VectorGroup ;
    rdfs:range xsd:string .

cim:VectorGroup.YD7 a rdf:Property ;
    rdfs:label "YD7" ;
    rdfs:comment "" ;
    rdfs:domain cim:VectorGroup ;
    rdfs:range xsd:string .

cim:VectorGroup.YN0 a rdf:Property ;
    rdfs:label "YN0" ;
    rdfs:comment "" ;
    rdfs:domain cim:VectorGroup ;
    rdfs:range xsd:string .

cim:VectorGroup.YND1 a rdf:Property ;
    rdfs:label "YND1" ;
    rdfs:comment "" ;
    rdfs:domain cim:VectorGroup ;
    rdfs:range xsd:string .

cim:VectorGroup.YND11 a rdf:Property ;
    rdfs:label "YND11" ;
    rdfs:comment "" ;
    rdfs:domain cim:VectorGroup ;
    rdfs:range xsd:string .

cim:VectorGroup.YND5 a rdf:Property ;
    rdfs:label "YND5" ;
    rdfs:comment "" ;
    rdfs:domain cim:VectorGroup ;
    rdfs:range xsd:string .

cim:VectorGroup.YND7 a rdf:Property ;
    rdfs:label "YND7" ;
    rdfs:comment "" ;
    rdfs:domain cim:VectorGroup ;
    rdfs:range xsd:string .

cim:VectorGroup.YNDN1 a rdf:Property ;
    rdfs:label "YNDN1" ;
    rdfs:comment "" ;
    rdfs:domain cim:VectorGroup ;
    rdfs:range xsd:string .

cim:VectorGroup.YNDN11 a rdf:Property ;
    rdfs:label "YNDN11" ;
    rdfs:comment "" ;
    rdfs:domain cim:VectorGroup ;
    rdfs:range xsd:string .

cim:VectorGroup.YNY0 a rdf:Property ;
    rdfs:label "YNY0" ;
    rdfs:comment "" ;
    rdfs:domain cim:VectorGroup ;
    rdfs:range xsd:string .

cim:VectorGroup.YNY6 a rdf:Property ;
    rdfs:label "YNY6" ;
    rdfs:comment "" ;
    rdfs:domain cim:VectorGroup ;
    rdfs:range xsd:string .

cim:VectorGroup.YNYN0 a rdf:Property ;
    rdfs:label "YNYN0" ;
    rdfs:comment "" ;
    rdfs:domain cim:VectorGroup ;
    rdfs:range xsd:string .

cim:VectorGroup.YNYN6 a rdf:Property ;
    rdfs:label "YNYN6" ;
    rdfs:comment "" ;
    rdfs:domain cim:VectorGroup ;
    rdfs:range xsd:string .

cim:VectorGroup.YNZ11 a rdf:Property ;
    rdfs:label "YNZ11" ;
    rdfs:comment "" ;
    rdfs:domain cim:VectorGroup ;
    rdfs:range xsd:string .

cim:VectorGroup.YNZ5 a rdf:Property ;
    rdfs:label "YNZ5" ;
    rdfs:comment "" ;
    rdfs:domain cim:VectorGroup ;
    rdfs:range xsd:string .

cim:VectorGroup.YNZN1 a rdf:Property ;
    rdfs:label "YNZN1" ;
    rdfs:comment "" ;
    rdfs:domain cim:VectorGroup ;
    rdfs:range xsd:string .

cim:VectorGroup.YNZN11 a rdf:Property ;
    rdfs:label "YNZN11" ;
    rdfs:comment "" ;
    rdfs:domain cim:VectorGroup ;
    rdfs:range xsd:string .

cim:VectorGroup.YNZN5 a rdf:Property ;
    rdfs:label "YNZN5" ;
    rdfs:comment "" ;
    rdfs:domain cim:VectorGroup ;
    rdfs:range xsd:string .

cim:VectorGroup.YNZN7 a rdf:Property ;
    rdfs:label "YNZN7" ;
    rdfs:comment "" ;
    rdfs:domain cim:VectorGroup ;
    rdfs:range xsd:string .

cim:VectorGroup.YY0 a rdf:Property ;
    rdfs:label "YY0" ;
    rdfs:comment "" ;
    rdfs:domain cim:VectorGroup ;
    rdfs:range xsd:string .

cim:VectorGroup.YY6 a rdf:Property ;
    rdfs:label "YY6" ;
    rdfs:comment "" ;
    rdfs:domain cim:VectorGroup ;
    rdfs:range xsd:string .

cim:VectorGroup.YYN0 a rdf:Property ;
    rdfs:label "YYN0" ;
    rdfs:comment "" ;
    rdfs:domain cim:VectorGroup ;
    rdfs:range xsd:string .

cim:VectorGroup.YYN6 a rdf:Property ;
    rdfs:label "YYN6" ;
    rdfs:comment "" ;
    rdfs:domain cim:VectorGroup ;
    rdfs:range xsd:string .

cim:VectorGroup.YZ1 a rdf:Property ;
    rdfs:label "YZ1" ;
    rdfs:comment "" ;
    rdfs:domain cim:VectorGroup ;
    rdfs:range xsd:string .

cim:VectorGroup.YZ11 a rdf:Property ;
    rdfs:label "YZ11" ;
    rdfs:comment "" ;
    rdfs:domain cim:VectorGroup ;
    rdfs:range xsd:string .

cim:VectorGroup.YZ5 a rdf:Property ;
    rdfs:label "YZ5" ;
    rdfs:comment "" ;
    rdfs:domain cim:VectorGroup ;
    rdfs:range xsd:string .

cim:VectorGroup.YZ7 a rdf:Property ;
    rdfs:label "YZ7" ;
    rdfs:comment "" ;
    rdfs:domain cim:VectorGroup ;
    rdfs:range xsd:string .

cim:VectorGroup.YZN1 a rdf:Property ;
    rdfs:label "YZN1" ;
    rdfs:comment "" ;
    rdfs:domain cim:VectorGroup ;
    rdfs:range xsd:string .

cim:VectorGroup.YZN11 a rdf:Property ;
    rdfs:label "YZN11" ;
    rdfs:comment "" ;
    rdfs:domain cim:VectorGroup ;
    rdfs:range xsd:string .

cim:VectorGroup.YZN5 a rdf:Property ;
    rdfs:label "YZN5" ;
    rdfs:comment "" ;
    rdfs:domain cim:VectorGroup ;
    rdfs:range xsd:string .

cim:VectorGroup.YZN7 a rdf:Property ;
    rdfs:label "YZN7" ;
    rdfs:comment "" ;
    rdfs:domain cim:VectorGroup ;
    rdfs:range xsd:string .

cim:VectorGroup.ZD0 a rdf:Property ;
    rdfs:label "ZD0" ;
    rdfs:comment "" ;
    rdfs:domain cim:VectorGroup ;
    rdfs:range xsd:string .

cim:VectorGroup.ZD1 a rdf:Property ;
    rdfs:label "ZD1" ;
    rdfs:comment "" ;
    rdfs:domain cim:VectorGroup ;
    rdfs:range xsd:string .

cim:VectorGroup.ZD6 a rdf:Property ;
    rdfs:label "ZD6" ;
    rdfs:comment "" ;
    rdfs:domain cim:VectorGroup ;
    rdfs:range xsd:string .

cim:VectorGroup.ZD7 a rdf:Property ;
    rdfs:label "ZD7" ;
    rdfs:comment "" ;
    rdfs:domain cim:VectorGroup ;
    rdfs:range xsd:string .

cim:VectorGroup.ZND0 a rdf:Property ;
    rdfs:label "ZND0" ;
    rdfs:comment "" ;
    rdfs:domain cim:VectorGroup ;
    rdfs:range xsd:string .

cim:VectorGroup.ZND1 a rdf:Property ;
    rdfs:label "ZND1" ;
    rdfs:comment "" ;
    rdfs:domain cim:VectorGroup ;
    rdfs:range xsd:string .

cim:VectorGroup.ZND6 a rdf:Property ;
    rdfs:label "ZND6" ;
    rdfs:comment "" ;
    rdfs:domain cim:VectorGroup ;
    rdfs:range xsd:string .

cim:VectorGroup.ZND7 a rdf:Property ;
    rdfs:label "ZND7" ;
    rdfs:comment "" ;
    rdfs:domain cim:VectorGroup ;
    rdfs:range xsd:string .

cim:VectorGroup.ZNY1 a rdf:Property ;
    rdfs:label "ZNY1" ;
    rdfs:comment "" ;
    rdfs:domain cim:VectorGroup ;
    rdfs:range xsd:string .

cim:VectorGroup.ZNY11 a rdf:Property ;
    rdfs:label "ZNY11" ;
    rdfs:comment "" ;
    rdfs:domain cim:VectorGroup ;
    rdfs:range xsd:string .

cim:VectorGroup.ZNY5 a rdf:Property ;
    rdfs:label "ZNY5" ;
    rdfs:comment "" ;
    rdfs:domain cim:VectorGroup ;
    rdfs:range xsd:string .

cim:VectorGroup.ZNY7 a rdf:Property ;
    rdfs:label "ZNY7" ;
    rdfs:comment "" ;
    rdfs:domain cim:VectorGroup ;
    rdfs:range xsd:string .

cim:VectorGroup.ZNYN1 a rdf:Property ;
    rdfs:label "ZNYN1" ;
    rdfs:comment "" ;
    rdfs:domain cim:VectorGroup ;
    rdfs:range xsd:string .

cim:VectorGroup.ZNYN11 a rdf:Property ;
    rdfs:label "ZNYN11" ;
    rdfs:comment "" ;
    rdfs:domain cim:VectorGroup ;
    rdfs:range xsd:string .

cim:VectorGroup.ZNYN5 a rdf:Property ;
    rdfs:label "ZNYN5" ;
    rdfs:comment "" ;
    rdfs:domain cim:VectorGroup ;
    rdfs:range xsd:string .

cim:VectorGroup.ZNYN7 a rdf:Property ;
    rdfs:label "ZNYN7" ;
    rdfs:comment "" ;
    rdfs:domain cim:VectorGroup ;
    rdfs:range xsd:string .

cim:VectorGroup.ZY1 a rdf:Property ;
    rdfs:label "ZY1" ;
    rdfs:comment "" ;
    rdfs:domain cim:VectorGroup ;
    rdfs:range xsd:string .

cim:VectorGroup.ZY11 a rdf:Property ;
    rdfs:label "ZY11" ;
    rdfs:comment "" ;
    rdfs:domain cim:VectorGroup ;
    rdfs:range xsd:string .

cim:VectorGroup.ZY5 a rdf:Property ;
    rdfs:label "ZY5" ;
    rdfs:comment "" ;
    rdfs:domain cim:VectorGroup ;
    rdfs:range xsd:string .

cim:VectorGroup.ZY7 a rdf:Property ;
    rdfs:label "ZY7" ;
    rdfs:comment "" ;
    rdfs:domain cim:VectorGroup ;
    rdfs:range xsd:string .

cim:VectorGroup.ZYN1 a rdf:Property ;
    rdfs:label "ZYN1" ;
    rdfs:comment "" ;
    rdfs:domain cim:VectorGroup ;
    rdfs:range xsd:string .

cim:VectorGroup.ZYN11 a rdf:Property ;
    rdfs:label "ZYN11" ;
    rdfs:comment "" ;
    rdfs:domain cim:VectorGroup ;
    rdfs:range xsd:string .

cim:VectorGroup.ZYN5 a rdf:Property ;
    rdfs:label "ZYN5" ;
    rdfs:comment "" ;
    rdfs:domain cim:VectorGroup ;
    rdfs:range xsd:string .

cim:VectorGroup.ZYN7 a rdf:Property ;
    rdfs:label "ZYN7" ;
    rdfs:comment "" ;
    rdfs:domain cim:VectorGroup ;
    rdfs:range xsd:string .

cim:Voltage.value a rdf:Property ;
    rdfs:label "value" ;
    rdfs:comment "volts (V)" ;
    rdfs:domain cim:Voltage ;
    rdfs:range xsd:int .

cim:WindingConnection.A a rdf:Property ;
    rdfs:label "A" ;
    rdfs:comment "Autotransformer common winding." ;
    rdfs:domain cim:WindingConnection ;
    rdfs:range xsd:string .

cim:WindingConnection.D a rdf:Property ;
    rdfs:label "D" ;
    rdfs:comment "Delta." ;
    rdfs:domain cim:WindingConnection ;
    rdfs:range xsd:string .

cim:WindingConnection.I a rdf:Property ;
    rdfs:label "I" ;
    rdfs:comment "Independent winding, for single-phase connections." ;
    rdfs:domain cim:WindingConnection ;
    rdfs:range xsd:string .

cim:WindingConnection.UNKNOWN_WINDING a rdf:Property ;
    rdfs:label "UNKNOWN_WINDING" ;
    rdfs:comment "" ;
    rdfs:domain cim:WindingConnection ;
    rdfs:range xsd:string .

cim:WindingConnection.Y a rdf:Property ;
    rdfs:label "Y" ;
    rdfs:comment "Wye." ;
    rdfs:domain cim:WindingConnection ;
    rdfs:range xsd:string .

cim:WindingConnection.Yn a rdf:Property ;
    rdfs:label "Yn" ;
    rdfs:comment "Wye, with neutral brought out for grounding." ;
    rdfs:domain cim:WindingConnection ;
    rdfs:range xsd:string .

cim:WindingConnection.Z a rdf:Property ;
    rdfs:label "Z" ;
    rdfs:comment "ZigZag." ;
    rdfs:domain cim:WindingConnection ;
    rdfs:range xsd:string .

cim:WindingConnection.Zn a rdf:Property ;
    rdfs:label "Zn" ;
    rdfs:comment "ZigZag, with neutral brought out for grounding." ;
    rdfs:domain cim:WindingConnection ;
    rdfs:range xsd:string .

cim:WireInfo.material a rdf:Property ;
    rdfs:label "material" ;
    rdfs:comment "Conductor material." ;
    rdfs:domain cim:WireInfo ;
    rdfs:range cim:WireMaterialKind .

cim:WireInfo.ratedCurrent a rdf:Property ;
    rdfs:label "ratedCurrent" ;
    rdfs:comment "Current carrying capacity of the wire under stated thermal conditions." ;
    rdfs:domain cim:WireInfo ;
    rdfs:range cim:CurrentFlow .

cim:WireMaterialKind.UNKNOWN a rdf:Property ;
    rdfs:label "UNKNOWN" ;
    rdfs:comment "Default. EWB extension." ;
    rdfs:domain cim:WireMaterialKind ;
    rdfs:range xsd:string .

cim:WireMaterialKind.aaac a rdf:Property ;
    rdfs:label "aaac" ;
    rdfs:comment "Aluminum-alloy conductor steel reinforced." ;
    rdfs:domain cim:WireMaterialKind ;
    rdfs:range xsd:string .

cim:WireMaterialKind.acsr a rdf:Property ;
    rdfs:label "acsr" ;
    rdfs:comment "Aluminum conductor steel reinforced." ;
    rdfs:domain cim:WireMaterialKind ;
    rdfs:range xsd:string .

cim:WireMaterialKind.acsrAz a rdf:Property ;
    rdfs:label "acsrAz" ;
    rdfs:comment "Aluminum conductor steel reinforced, aluminumized steel core. EWB extension." ;
    rdfs:domain cim:WireMaterialKind ;
    rdfs:range xsd:string .

cim:WireMaterialKind.aluminum a rdf:Property ;
    rdfs:label "aluminum" ;
    rdfs:comment "Aluminum wire." ;
    rdfs:domain cim:WireMaterialKind ;
    rdfs:range xsd:string .

cim:WireMaterialKind.aluminumAlloy a rdf:Property ;
    rdfs:label "aluminumAlloy" ;
    rdfs:comment "Aluminum-alloy wire." ;
    rdfs:domain cim:WireMaterialKind ;
    rdfs:range xsd:string .

cim:WireMaterialKind.aluminumAlloySteel a rdf:Property ;
    rdfs:label "aluminumAlloySteel" ;
    rdfs:comment "Aluminum-alloy-steel wire." ;
    rdfs:domain cim:WireMaterialKind ;
    rdfs:range xsd:string .

cim:WireMaterialKind.aluminumSteel a rdf:Property ;
    rdfs:label "aluminumSteel" ;
    rdfs:comment "Aluminum-steel wire." ;
    rdfs:domain cim:WireMaterialKind ;
    rdfs:range xsd:string .

cim:WireMaterialKind.copper a rdf:Property ;
    rdfs:label "copper" ;
    rdfs:comment "Copper wire." ;
    rdfs:domain cim:WireMaterialKind ;
    rdfs:range xsd:string .

cim:WireMaterialKind.copperCadmium a rdf:Property ;
    rdfs:label "copperCadmium" ;
    rdfs:comment "Copper cadmium wire. EWB extension." ;
    rdfs:domain cim:WireMaterialKind ;
    rdfs:range xsd:string .

cim:WireMaterialKind.other a rdf:Property ;
    rdfs:label "other" ;
    rdfs:comment "Other wire material." ;
    rdfs:domain cim:WireMaterialKind ;
    rdfs:range xsd:string .

cim:WireMaterialKind.steel a rdf:Property ;
    rdfs:label "steel" ;
    rdfs:comment "Steel wire." ;
    rdfs:domain cim:WireMaterialKind ;
    rdfs:range xsd:string .
